<?xml version="1.0" encoding="UTF-8"?>
<rdf:RDF xmlns:owl="http://www.w3.org/2002/07/owl#" xmlns:rdf="http://www.w3.org/1999/02/22-rdf-syntax-ns#" xmlns:rdfs="http://www.w3.org/2000/01/rdf-schema#"
	xmlns:av7="https://github.com/SPSCommerce/semantic-network/blob/master/Semantic%20Assortment/av7.rdf#" xmlns:dc="http://dublincore.org/2012/06/14/dcelements.rdf#"
	xmlns:dct="http://purl.org/dc/terms#" xmlns:foaf="http://xmlns.com/foaf/spec/index.rdf#" xmlns:sorg="http://schema.org" xmlns:sbml="http://www.sbml.org/sbml/level1"
	xmlns:wmlo="https://github.com/SPSCommerce/semantic-network/blob/master/Other%20Ontologies/WeightsMeasureOnto.xml" xmlns:skos="http://www.w3.org/2004/02/skos/core#"
	xmlns:spsis="https://github.com/SPSCommerce/semantic-network/blob/master/Other%20Ontologies/spsItemNetwork.rdf" xmlns:xsd="http://www.w3.org/2001/XMLSchema#"
	xmlns:xs="http://www.w3.org/2001/XMLSchema" xmlns:av7cb="https://github.com/SPSCommerce/semantic-network/blob/master/Semantic%20RSX/Semantic-Assortment/av7cBlank.rdf#"
	xml:base="https://github.com/SPSCommerce/semantic-network/blob/master/Semantic%20Assortment/av7.rdf#">
	<rdf:Description rdf:about="https://github.com/SPSCommerce/semantic-network/blob/master/Semantic%20Assortment/av7.rdf#">
		<dc:title rdf:value="Assortment Version 7"/>
		<dc:creator foaf:givenName="Mara" foaf:familyName="Inglezakis"/>
		<dc:description>Assortment Version 7 (AV7) represents SPS Commerce's Assortment Version 7 (also known as 'Catalog')
			as an ontology. It reproduces Assortment Version 7 exactly as it existed in Octobe 2016 in all save the following ways:
			1) some definitions have been updated for clarity; 2) ranges built to the specifications of particular retailers have been deprecated;
			3) the system which classified the Assortment attribute spreadsheet (also known as 'tabs') has been deprecated.</dc:description>
		<rdfs:comment>AV7 is a subset of AV7C.</rdfs:comment>
	</rdf:Description>
	<!-- Ontology Properties -->
	<owl:Class rdf:ID="TranslationProp">
		<rdfs:label>Legacy Container Property</rdfs:label>
		<rdfs:comment>The class of properties that enable concept translation into OWL ontologies from XML and other legacy models.</rdfs:comment>
	</owl:Class>
	<!-- Assortment Product Properties -->
	<owl:Class rdf:ID="CompositeWoodCertificationCode"/>
	<owl:Class rdf:ID="CountryOfOriginComponents"/>
	<owl:Class rdf:ID="CoverageAreaUOM" rdfs:subClassOf="wmlo#AreaMeasure"/>
	<owl:Class rdf:ID="ESRBRating">
		<rdfs:subClassOf rdf:resource="spsis#Marker"/>
	</owl:Class>
	<owl:Class rdf:ID="gDate">
		<owl:unionOf rdf:parseType="Collection">
			<rdf:Description rdf:about="xsd#gMonthDay"/>
			<rdf:Description rdf:about="xsd#gYear"/>
		</owl:unionOf>
	</owl:Class>
	<owl:Class rdf:ID="HazardousMaterialQualifier"/>
	<owl:Class rdf:ID="LoadOrderingFactorUOM">
		<owl:equivalentClass>
			<owl:unionOf>
				<owl:Class rdf:resource="wmlo#VolumeUOM"/>
				<owl:Class rdf:resource="wmlo#PackType"/>
				<owl:Class rdf:resource="wmlo#WeightUOM"/>
			</owl:unionOf>
		</owl:equivalentClass>
	</owl:Class>
	<owl:Class rdf:ID="MPAARating"/>
	<owl:Class rdf:ID="OpenTimeUOM" rdfs:subClassOf="wmlo#TimeMeasure"/>
	<owl:Class rdf:ID="OrderLeadTimeCode"/>
	<owl:Class rdf:ID="PackingGroup"/>
	<owl:Class rdf:ID="PackType" rdfs:subClassOf="wmlo#PackType"/>
	<owl:Class rdf:ID="PackVolumeUOM" rdfs:subClassOf="wmlo#VolumeUOM"/>
	<owl:Class rdf:ID="PackWeightUOM" rdfs:subClassOf="wmlo#WeightUOM"/>
	<owl:Class rdf:ID="PriceQualifier"/>
	<owl:Class rdf:ID="PriceUOM" rdfs:subClassOf="wmlo#PriceUOM"/>
	<owl:Class rdf:ID="ProcessorSpeedUOM" rdfs:subClassOf="wmlo#FrequencyMeasure"/>
	<owl:Class rdf:ID="ReturnCode"/>
	<owl:Class rdf:ID="SmallPartsWarning"/>
	<owl:Class rdf:ID="SpatialUOM" rdfs:subClassOf="wmlo#TwoDUOM"/>
	<owl:Class rdf:ID="SpecialHandlingCode"/>
	<owl:Class rdf:ID="SpecialItemCode"/>
	<owl:Class rdf:ID="SpreadRateUOM" rdfs:subClassOf="wmlo#AreaMeasure"/>
	<owl:Class rdf:ID="VariableDate">
		<owl:unionOf rdf:parseType="Collection">
			<rdf:Description rdf:about="av7#gDate"/>
			<rdf:Description rdf:about="xsd#date"/>
		</owl:unionOf>
	</owl:Class>
	<owl:Class rdf:ID="TempUOM" rdfs:subClassOf="wmlo#TemperatureUOM"/>
	<owl:Class rdf:ID="UsagePerTimeUOM"/>
	<owl:Class rdf:ID="WorkingTimeUOM" rdfs:subClassOf="wmlo#TimeMeasure"/>
	<owl:NamedIndividual rdf:ID="adultsRating" rdf:type="av7#ESRBRating" rdfs:label="Adults Only"/>
	<owl:NamedIndividual rdf:ID="ampere">
		<rdfs:type rdf:resource="av7#UsagePerTimeUOM"/>
		<rdfs:label>
			<rdf:Alt>
				<rdf:li rdf:value="A"/>
				<rdf:li rdf:value="Ampere"/>
			</rdf:Alt>
		</rdfs:label>
		<!-- <owl:sameAs rdf:resource="wmlo#ampere"/> -->
	</owl:NamedIndividual>
	<owl:NamedIndividual rdf:ID="aNotApplicable">
		<rdf:type rdf:resource="av7#SmallPartsWarning"/>
		<rdfs:label rdf:parseType="Resource">
			<rdf:li rdf:value="A"/>
			<rdf:li rdf:value="Not Applicable."/>
		</rdfs:label>
	</owl:NamedIndividual>
	<owl:NamedIndividual rdf:ID="assortment" rdf:type="av7#PackType">
		<rdfs:label rdf:parseType="Resource">
			<rdf:li rdf:value="AS"/>
			<rdf:li rdf:value="assortment"/>
		</rdfs:label>
		<!-- <owl:sameAs rdf:resource="wmlo#assortment"/> -->
	</owl:NamedIndividual><owl:NamedIndividual rdf:ID="australiaDollar">
		<rdf:type rdf:resource="av7#PriceUOM"/>
		<rdfs:label>
			<rdf:Bag>
				<rdf:li rdf:value="AUD"/>
				<rdf:li rdf:value="Australian Dollar"/>
			</rdf:Bag>
		</rdfs:label>
		<!-- <owl:sameAs rdf:resource="wmlo#AUD_AustraliaDollar"/> -->
	</owl:NamedIndividual><owl:NamedIndividual rdf:ID="bag" rdf:type="av7#PackType">
		<rdfs:label rdf:parseType="Resource">
			<rdf:li rdf:value="BG"/>
			<rdf:li rdf:value="bag"/>
		</rdfs:label>
		<!-- <owl:sameAs rdf:resource="wmlo#bag"/> -->
	</owl:NamedIndividual><owl:NamedIndividual rdf:ID="bar" rdf:type="av7#PackType">
		<rdfs:label rdf:parseType="Resource">
			<rdf:li rdf:value="BI"/>
			<rdf:li rdf:value="bar"/>
		</rdfs:label>
		<!-- <owl:sameAs rdf:resource="wmlo#bar"/> -->
	</owl:NamedIndividual><owl:NamedIndividual rdf:ID="barrel" rdf:type="av7#PackType">
		<rdfs:label rdf:parseType="Resource">
			<rdf:li rdf:value="BR"/>
			<rdf:li rdf:value="barrel"/>
		</rdfs:label>
		<!-- <owl:sameAs rdf:resource="wmlo#barrel"/> -->
	</owl:NamedIndividual><owl:NamedIndividual rdf:ID="bottle" rdf:type="av7#PackType">
		<rdfs:label rdf:parseType="Resource">
			<rdf:li rdf:value="BO"/>
			<rdf:li rdf:value="bottle"/>
		</rdfs:label>
		<!-- <owl:sameAs rdf:resource="wmlo#bottle"/> -->
	</owl:NamedIndividual>
	<owl:NamedIndividual rdf:ID="box" rdf:type="av7#PackType">
		<rdfs:label rdf:parseType="Resource">
			<rdf:li rdf:value="BX"/>
			<rdf:li rdf:value="box"/>
		</rdfs:label>
		<!-- <owl:sameAs rdf:resource="wmlo#box"/> -->
	</owl:NamedIndividual><owl:NamedIndividual rdf:ID="bSmallBall">
		<rdf:type rdf:resource="av7#SmallPartsWarning"/>
		<rdfs:label rdf:parseType="Resource">
			<rdf:li rdf:value="B"/>
			<rdf:li rdf:value="Is a small ball. Not for children under 3 years."/>
		</rdfs:label>
	</owl:NamedIndividual>
	<owl:NamedIndividual rdf:ID="bushel" rdf:type="av7#PackType">
		<rdfs:label rdf:parseType="Resource">
			<rdf:li rdf:value="BU"/>
			<rdf:li rdf:value="bushel"/>
		</rdfs:label>
		<!-- <owl:sameAs rdf:resource="wmlo#bushel"/> -->
	</owl:NamedIndividual><owl:NamedIndividual rdf:ID="businessDay" rdf:type="av7#OrderLeadTimeCode" rdfs:label="business day"/>
	<owl:NamedIndividual rdf:ID="can" rdf:type="av7#PackType">
		<rdfs:label rdf:parseType="Resource">
			<rdf:li rdf:value="CN"/>
			<rdf:li rdf:value="can"/>
		</rdfs:label>
		<!-- <owl:sameAs rdf:resource="wmlo#can"/> -->
	</owl:NamedIndividual><owl:NamedIndividual rdf:ID="canadaDollar">
		<rdf:type rdf:resource="av7#PriceUOM"/>
		<rdfs:label>
			<rdf:Bag>
				<rdf:li rdf:value="CAD"/>
				<rdf:li rdf:value="Canadian Dollar"/>
			</rdf:Bag>
		</rdfs:label>
		<!-- <owl:sameAs rdf:resource="wmlo#CAD_CanadaDollar"/> -->
	</owl:NamedIndividual><owl:NamedIndividual rdf:ID="capsule" rdf:type="av7#PackType">
		<rdfs:label rdf:parseType="Resource">
			<rdf:li rdf:value="AV"/>
			<rdf:li rdf:value="capsule"/>
		</rdfs:label>
		<!-- <owl:sameAs rdf:resource="wmlo#capsule"/> -->
	</owl:NamedIndividual><owl:NamedIndividual rdf:ID="carton" rdf:type="av7#PackType">
		<rdfs:label rdf:parseType="Resource">
			<rdf:li rdf:value="CT"/>
			<rdf:li rdf:value="carton"/>
		</rdfs:label>
		<!-- <owl:sameAs rdf:resource="wmlo#carton"/> -->
	</owl:NamedIndividual><owl:NamedIndividual rdf:ID="case">
		<rdf:type rdf:resource="av7#PackType"/>
		<rdf:type rdf:resource="av7#LoadOrderingFactorUOM"/>
		<rdfs:label rdf:parseType="Resource">
			<rdf:li rdf:value="CA"/>
			<rdf:li rdf:value="case"/>
		</rdfs:label>
		<!-- <owl:sameAs rdf:resource="wmlo#case"/> -->
	</owl:NamedIndividual><owl:NamedIndividual rdf:ID="centigram" rdf:type="av7#PackType">
		<rdfs:label rdf:parseType="Resource">
			<rdf:li rdf:value="AF"/>
			<rdf:li rdf:value="centigram"/>
		</rdfs:label>
		<!-- <owl:sameAs rdf:resource="wmlo#centigram"/> -->
	</owl:NamedIndividual><owl:NamedIndividual rdf:ID="centiliter">
		<rdf:type rdf:resource="av7#PackType"/>
		<rdf:type rdf:resource="av7#PackVolumeUOM"/>
		<rdfs:label rdf:parseType="Resource">
			<rdf:li rdf:value="C3"/>
			<rdf:li rdf:value="centiliter"/>
		</rdfs:label>
		<!-- <owl:sameAs rdf:resource="wmlo#centiliter"/> -->
	</owl:NamedIndividual><owl:NamedIndividual rdf:ID="centimeter">
		<rdf:type rdf:resource="av7#PackType"/>
		<rdf:type rdf:resource="av7#SpatialUOM"/>
		<rdfs:label rdf:parseType="Resource">
			<rdf:li rdf:value="cm"/>
			<rdf:li rdf:value="CM"/>
			<rdf:li rdf:value="centimeter"/>
			<rdf:li rdf:value="Centimeter"/>
			<rdf:li rdf:value="centimeters"/>
			<rdf:li rdf:value="Centimeters"/>
		</rdfs:label>
		<!-- <owl:sameAs rdf:resource="wmlo#centimeter"/> -->
	</owl:NamedIndividual><owl:NamedIndividual rdf:ID="collateral">
		<rdf:type rdf:resource="av7#SpecialItemCode"/>
		<rdfs:label>
			<rdf:Alt>
				<rdf:li rdf:value="CL"/>
				<rdf:li rdf:value="Collateral"/>
			</rdf:Alt>
		</rdfs:label>
	</owl:NamedIndividual>
	<owl:NamedIndividual rdf:ID="compatibleHazMat" rdf:type="av7#HazardousMaterialQualifier" rdfs:label="C (Storage Compatibility Group)"/>
	<owl:NamedIndividual rdf:ID="container" rdf:type="av7#PackType">
		<rdfs:label rdf:parseType="Resource">
			<rdf:li rdf:value="CH"/>
			<rdf:li rdf:value="container"/>
		</rdfs:label>
		<!-- <owl:sameAs rdf:resource="wmlo#centiliter"/> -->
	</owl:NamedIndividual><owl:NamedIndividual rdf:ID="cSmallBall">
		<rdf:type rdf:resource="av7#SmallPartsWarning"/>
		<rdfs:label rdf:parseType="Resource">
			<rdf:li rdf:value="C"/>
			<rdf:li rdf:value="Contains a small ball. Not for children under 3 years."/>
		</rdfs:label>
	</owl:NamedIndividual>
	<owl:NamedIndividual rdf:ID="cubicCentimeter">
		<rdf:type rdf:resource="av7#PackType"/>
		<rdf:type rdf:resource="av7#PackVolumeUOM"/>
		<rdfs:label rdf:parseType="Resource">
			<rdf:li rdf:value="CC"/>
			<rdf:li rdf:value="cubic centimeter"/>
		</rdfs:label>
		<!-- <owl:sameAs rdf:resource="wmlo#cubicCentimeter"/> -->
	</owl:NamedIndividual><owl:NamedIndividual rdf:ID="cubicFoot">
		<rdf:type rdf:resource="av7#PackType"/>
		<rdf:type rdf:resource="av7#PackVolumeUOM"/>
		<rdf:type rdf:resource="av7#LoadOrderingFactorUOM"/>
		<rdfs:label rdf:parseType="Resource">
			<rdf:li rdf:value="CF"/>
			<rdf:li rdf:value="cubic feet"/>
		</rdfs:label>
		<!-- <owl:sameAs rdf:resource="wmlo#cubicFoot"/> -->
	</owl:NamedIndividual><owl:NamedIndividual rdf:ID="cubicInch">
		<rdf:type rdf:resource="av7#PackType"/>
		<rdf:type rdf:resource="av7#PackVolumeUOM"/>
		<rdfs:label rdf:parseType="Resource">
			<rdf:li rdf:value="CI"/>
			<rdf:li rdf:value="cubic inches"/>
		</rdfs:label>
		<!-- <owl:sameAs rdf:resource="wmlo#cubicInch"/> -->
	</owl:NamedIndividual><owl:NamedIndividual rdf:ID="cubicMeter">
		<rdf:type rdf:resource="av7#PackType"/>
		<rdf:type rdf:resource="av7#PackVolumeUOM"/>
		<rdfs:label rdf:parseType="Resource">
			<rdf:li rdf:value="CR"/>
			<rdf:li rdf:value="cubic meter"/>
		</rdfs:label>
		<!-- <owl:sameAs rdf:resource="wmlo#cubicMeter"/> -->
	</owl:NamedIndividual><owl:NamedIndividual rdf:ID="cubicYard">
		<rdf:type rdf:resource="av7#PackType"/>
		<rdf:type rdf:resource="av7#PackVolumeUOM"/>
		<rdfs:label rdf:parseType="Resource">
			<rdf:li rdf:value="CY"/>
			<rdf:li rdf:value="cubic yard"/>
		</rdfs:label>
		<!-- <owl:sameAs rdf:resource="wmlo#cubicYard"/> -->
	</owl:NamedIndividual><owl:NamedIndividual rdf:ID="cup" rdf:type="av7#PackType">
		<rdfs:label rdf:parseType="Resource">
			<rdf:li rdf:value="CU"/>
			<rdf:li rdf:value="cup"/>
		</rdfs:label>
		<!-- <owl:sameAs rdf:resource="wmlo#cupUSA"/> -->
	</owl:NamedIndividual><owl:NamedIndividual rdf:ID="day">
		<rdf:type rdf:resource="av7#OpenTimeUOM"/>
		<rdf:type rdf:resource="av7#OrderLeadTimeCode"/>
		<rdf:type rdf:resource="av7#WorkingTimeUOM"/>
		<rdfs:label rdf:parseType="Resource">
			<rdf:li rdf:value="day"/>
			<rdf:li rdf:value="days"/>
			<rdf:li rdf:value="week day"/>
		</rdfs:label>
	</owl:NamedIndividual>
	<owl:NamedIndividual rdf:ID="decigram" rdf:type="av7#PackType">
		<rdfs:label rdf:parseType="Resource">
			<rdf:li rdf:value="DC"/>
			<rdf:li rdf:value="decigram"/>
		</rdfs:label>
		<!-- <owl:sameAs rdf:resource="wmlo#decigram"/> -->
	</owl:NamedIndividual><owl:NamedIndividual rdf:ID="deciliter">
		<rdf:type rdf:resource="av7#PackType"/>
		<rdf:type rdf:resource="av7#PackVolumeUOM"/>
		<rdfs:label rdf:parseType="Resource">
			<rdf:li rdf:value="DL"/>
			<rdf:li rdf:value="deciliter"/>
		</rdfs:label>
		<!-- <owl:sameAs rdf:resource="wmlo#deciliter"/> -->
	</owl:NamedIndividual><owl:NamedIndividual rdf:ID="decimeter" rdf:type="av7#SpatialUOM">
		<rdfs:label rdf:parseType="Resource">
			<rdf:li rdf:value="DM"/>
			<rdf:li rdf:value="decimeter"/>
		</rdfs:label>
		<!-- <owl:sameAs rdf:resource="wmlo#decimeter"/> -->
	</owl:NamedIndividual><owl:NamedIndividual rdf:ID="dHazMat" rdf:type="av7#HazardousMaterialQualifier">
		<rdfs:label rdf:parseType="Resource">
			<rdf:li rdf:value="D (Hazardous Materials ID, DOT)"/>
			<rdf:li rdf:value="D"/>
		</rdfs:label>
	</owl:NamedIndividual>
	<owl:NamedIndividual rdf:ID="degreeCelsius" rdf:type="av7#TempUOM">
		<rdfs:label rdf:parseType="Resource">
			<rdf:li rdf:value="c"/>
			<rdf:li rdf:value="C"/>
			<rdf:li rdf:value="celsius"/>
			<rdf:li rdf:value="Celsius"/>
		</rdfs:label>
		<!-- <owl:sameAs rdf:resource="wmlo#celsius"/> -->
	</owl:NamedIndividual><owl:NamedIndividual rdf:ID="degreeFahrenheit" rdf:type="av7#TempUOM">
		<rdfs:label rdf:parseType="Resource">
			<rdf:li rdf:value="f"/>
			<rdf:li rdf:value="F"/>
			<rdf:li rdf:value="fahrenheit"/>
			<rdf:li rdf:value="Fahrenheit"/>
		</rdfs:label>
		<!-- <owl:sameAs rdf:resource="wmlo#fahrenheit"/> -->
	</owl:NamedIndividual><owl:NamedIndividual rdf:ID="degreeKelvin" rdf:type="av7#TempUOM">
		<rdfs:label rdf:parseType="Resource">
			<rdf:li rdf:value="k"/>
			<rdf:li rdf:value="K"/>
			<rdf:li rdf:value="kelvin"/>
			<rdf:li rdf:value="Kelvin"/>
		</rdfs:label>
	</owl:NamedIndividual>
	<owl:NamedIndividual rdf:ID="destroyForCredit">
		<rdf:type rdf:resource="av7#ReturnCode"/>
		<rdfs:label>
			<rdf:Alt>
				<rdf:li rdf:value="DFC"/>
				<rdf:li rdf:value="destroy for credit"/>
			</rdf:Alt>
		</rdfs:label>
	</owl:NamedIndividual>
	<owl:NamedIndividual rdf:ID="directShipPrice">
		<rdf:type rdf:resource="av7#PriceQualifier"/>
		<rdfs:label rdf:parseType="Resource">
			<rdf:li rdf:value="DIP"/>
			<rdf:li rdf:value="Direct Ship Price"/>
		</rdfs:label>
	</owl:NamedIndividual>
	<owl:NamedIndividual rdf:ID="display" rdf:type="av7#PackType">
		<rdfs:label rdf:parseType="Resource">
			<rdf:li rdf:value="DS"/>
			<rdf:li rdf:value="display"/>
		</rdfs:label>
		<!-- <owl:sameAs rdf:resource="wmlo#display"/> -->
	</owl:NamedIndividual><owl:NamedIndividual rdf:ID="domesticShipHazMat" rdf:type="av7#HazardousMaterialQualifier" rdfs:label="D (Domestic shipping with proper shipping name)"/>
	<owl:NamedIndividual rdf:ID="doNotFreeze">
		<rdf:type rdf:resource="av7#SpecialHandlingCode"/>
		<rdfs:label rdf:parseType="Resource">
			<rdf:li rdf:value="DNF"/>
			<rdf:li rdf:value="Do Not Freeze"/>
		</rdfs:label>
	</owl:NamedIndividual>
	<owl:NamedIndividual rdf:ID="dropShipPrice">
		<rdf:type rdf:resource="av7#PriceQualifier"/>
		<rdfs:label rdf:parseType="Resource">
			<rdf:li rdf:value="DRP"/>
			<rdf:li rdf:value="Drop Ship Price"/>
		</rdfs:label>
	</owl:NamedIndividual>
	<owl:NamedIndividual rdf:ID="dSmallParts">
		<rdf:type rdf:resource="av7#SmallPartsWarning"/>
		<rdfs:label rdf:parseType="Resource">
			<rdf:li rdf:value="D"/>
			<rdf:li rdf:value="Small parts. Not for children under 3 years."/>
		</rdfs:label>
	</owl:NamedIndividual>
	<owl:NamedIndividual rdf:ID="eachPack">
		<rdf:type rdf:resource="av7#PackType"/>
		<rdf:type rdf:resource="av7#LoadOrderingFactorUOM"/>
		<rdfs:label rdf:parseType="Resource">
			<rdf:li rdf:value="EA"/>
			<rdf:li rdf:value="each"/>
		</rdfs:label>
		<!-- <owl:sameAs rdf:resource="wmlo#each"/> -->
	</owl:NamedIndividual><owl:NamedIndividual rdf:ID="earlyChildhoodRating" rdf:type="av7#ESRBRating" rdfs:label="Early Childhood"/>
	<owl:NamedIndividual rdf:ID="eBalloon">
		<rdfs:type rdf:resource="av7#SmallPartsWarning"/>
		<rdfs:label rdf:parseType="Resource">
			<rdf:li rdf:value="E"/>
			<rdf:li rdf:value="Is or contains a balloon. Not for children under 8 years."/>
		</rdfs:label>
	</owl:NamedIndividual>
	<owl:NamedIndividual rdf:ID="eightPack" rdf:type="av7#PackType">
		<rdfs:label rdf:parseType="Resource">
			<rdf:li rdf:value="P8"/>
			<rdf:li rdf:value="eight pack"/>
		</rdfs:label>
		<!-- <owl:sameAs rdf:resource="wmlo#eightPack"/> -->
	</owl:NamedIndividual><owl:NamedIndividual rdf:ID="environmentalControlLimits">
		<rdf:type rdf:resource="av7#SpecialHandlingCode"/>
		<rdfs:label rdf:parseType="Resource">
			<rdf:li rdf:value="EL"/>
			<rdf:li rdf:value="Environmental Control Limits"/>
		</rdfs:label>
	</owl:NamedIndividual>
	<owl:NamedIndividual rdf:ID="euroCurrency">
		<rdf:type rdf:resource="av7#PriceUOM"/>
		<rdfs:label>
			<rdf:Bag>
				<rdf:li rdf:value="EUR"/>
				<rdf:li rdf:value="Euro"/>
			</rdf:Bag>
		</rdfs:label>
		<!-- <owl:sameAs rdf:resource="wmlo#EUR_EuroMemberCountries"/> -->
	</owl:NamedIndividual><owl:NamedIndividual rdf:ID="everyone10Rating" rdf:type="av7#ESRBRating" rdfs:label="Everyone 10+"/>
	<owl:NamedIndividual rdf:ID="everyoneRating" rdf:type="av7#ESRBRating" rdfs:label="Everyone"/>
	<owl:NamedIndividual rdf:ID="fivePack" rdf:type="av7#PackType">
		<rdfs:label rdf:parseType="Resource">
			<rdf:li rdf:value="P5"/>
			<rdf:li rdf:value="five pack"/>
		</rdfs:label>
		<!-- <owl:sameAs rdf:resource="wmlo#fivePack"/> -->
	</owl:NamedIndividual><owl:NamedIndividual rdf:ID="flammable">
		<rdf:type rdf:resource="av7#SpecialHandlingCode"/>
		<rdfs:label rdf:parseType="Resource">
			<rdf:li rdf:value="FL"/>
			<rdf:li rdf:value="Flammable"/>
		</rdfs:label>
	</owl:NamedIndividual>
	<owl:NamedIndividual rdf:ID="fluidOunce">
		<rdf:type rdf:resource="av7#PackVolumeUOM"/>
		<rdfs:label rdf:parseType="Resource">
			<rdf:li rdf:value="FO"/>
			<rdf:li rdf:value="fluid ounce"/>
		</rdfs:label>
		<!-- <owl:sameAs rdf:resource="wmlo#fluidOunce"/> -->
	</owl:NamedIndividual><owl:NamedIndividual rdf:ID="fMarble">
		<rdf:type rdf:resource="av7#SmallPartsWarning"/>
		<rdfs:label rdf:parseType="Resource">
			<rdf:li rdf:value="F"/>
			<rdf:li rdf:value="Contains a marble. Not for children under 3 years."/>
		</rdfs:label>
	</owl:NamedIndividual>
	<owl:NamedIndividual rdf:ID="footMeasure">
		<rdf:type rdf:resource="av7#PackType"/>
		<rdf:type rdf:resource="av7#SpatialUOM"/>
		<rdfs:label rdf:parseType="Resource">
			<rdf:li rdf:value="FT"/>
			<rdf:li rdf:value="foot"/>
		</rdfs:label>
		<!-- <owl:sameAs rdf:resource="wmlo#foot"/> -->
	</owl:NamedIndividual><owl:NamedIndividual rdf:ID="fourPack" rdf:type="av7#PackType">
		<rdfs:label rdf:parseType="Resource">
			<rdf:li rdf:value="P4"/>
			<rdf:li rdf:value="four pack"/>
		</rdfs:label>
		<!-- <owl:sameAs rdf:resource="wmlo#fourPack"/> -->
	</owl:NamedIndividual><owl:NamedIndividual rdf:ID="fourSixHazMat" rdf:type="av7#HazardousMaterialQualifier" rdfs:label="4 (46-Level DOT Code)"/>
	<owl:NamedIndividual rdf:ID="gallon">
		<rdf:type rdf:resource="av7#PackType"/>
		<rdf:type rdf:resource="av7#PackVolumeUOM"/>
		<rdf:type rdf:resource="av7#UsagePerTimeUOM"/>
		<rdfs:label rdf:parseType="Resource">
			<rdf:li rdf:value="GA"/>
			<rdf:li rdf:value="G"/>
			<rdf:li rdf:value="gallon"/>
		</rdfs:label>
		<!-- <owl:sameAs rdf:resource="wmlo#gallon"/> -->
	</owl:NamedIndividual><owl:NamedIndividual rdf:ID="genericHazMat" rdf:type="av7#HazardousMaterialQualifier" rdfs:label="G (No proper shipping name; generic name only)"/>
	<owl:NamedIndividual rdf:ID="giftWithPurchase">
		<rdf:type rdf:resource="av7#SpecialItemCode"/>
		<rdfs:label>
			<rdf:Alt>
				<rdf:li rdf:value="GW"/>
				<rdf:li rdf:value="Gift With Purchase"/>
			</rdf:Alt>
		</rdfs:label>
	</owl:NamedIndividual>
	<owl:NamedIndividual rdf:ID="gigahertz" rdfs:type="av7#ProcessorSpeedUOM" rdfs:label="GHz"/>
	<owl:NamedIndividual rdf:ID="gMarble">
		<rdf:type rdf:resource="av7#SmallPartsWarning"/>
		<rdfs:label rdf:parseType="Resource">
			<rdf:li rdf:value="G"/>
			<rdf:li rdf:value="Is a marble. Not for children under 3 years."/>
		</rdfs:label>
	</owl:NamedIndividual>
	<owl:NamedIndividual rdf:ID="gram" rdf:type="av7#PackWeightUOM">
		<rdfs:label rdf:parseType="Resource">
			<rdf:li rdf:value="GR"/>
			<rdf:li rdf:value="gram"/>
		</rdfs:label>
	</owl:NamedIndividual>
	<owl:NamedIndividual rdf:ID="greatDanger" rdf:type="av7#PackingGroup" rdfs:label="Group I: Great Danger"/>
	<owl:NamedIndividual rdf:ID="halfDozen" rdf:type="av7#PackType">
		<rdfs:label rdf:parseType="Resource">
			<rdf:li rdf:value="HD"/>
			<rdf:li rdf:value="half dozen"/>
		</rdfs:label>
		<!-- <owl:sameAs rdf:resource="wmlo#halfDozen"/> -->
	</owl:NamedIndividual><owl:NamedIndividual rdf:ID="hazardHazMat" rdf:type="av7#HazardousMaterialQualifier" rdfs:label="X (Hazard Class or Division)"/>
	<owl:NamedIndividual rdf:ID="hertz" rdfs:type="av7#ProcessorSpeedUOM" rdfs:label="Hz"/>
	<owl:NamedIndividual rdf:ID="holdForInspection">
		<rdf:type rdf:resource="av7#ReturnCode"/>
		<rdfs:label>
			<rdf:Alt>
				<rdf:li rdf:value="HRI"/>
				<rdf:li rdf:value="hold for inspection"/>
			</rdf:Alt>
		</rdfs:label>
	</owl:NamedIndividual>
	<owl:NamedIndividual rdf:ID="hongKongDollar">
		<rdf:type rdf:resource="av7#PriceUOM"/>
		<rdfs:label>
			<rdf:Bag>
				<rdf:li rdf:value="HKD"/>
				<rdf:li rdf:value="Hong Kong Dollar"/>
			</rdf:Bag>
		</rdfs:label>
		<!-- <owl:sameAs rdf:resource="wmlo#HKD_HongKongDollar"/> -->
	</owl:NamedIndividual><owl:NamedIndividual rdf:ID="hour">
		<rdf:type rdf:resource="av7#OpenTimeUOM"/>
		<rdf:type rdf:resource="av7#OrderLeadTimeCode"/>
		<rdf:type rdf:resource="av7#WorkingTimeUOM"/>
		<rdfs:label rdf:parseType="Resource">
			<rdf:li rdf:value="hour"/>
			<rdf:li rdf:value="hours"/>
		</rdfs:label>
	</owl:NamedIndividual>
	<owl:NamedIndividual rdf:ID="hundredCount" rdf:type="av7#PackType">
		<rdfs:label rdf:parseType="Resource">
			<rdf:li rdf:value="HC"/>
			<rdf:li rdf:value="hundred count"/>
		</rdfs:label>
		<!-- <owl:sameAs rdf:resource="wmlo#hundredCount"/> -->
	</owl:NamedIndividual><owl:NamedIndividual rdf:ID="hundredFoot" rdf:type="av7#PackType">
		<rdfs:label rdf:parseType="Resource">
			<rdf:li rdf:value="HL"/>
			<rdf:li rdf:value="hundred feet"/>
		</rdfs:label>
		<!-- <owl:sameAs rdf:resource="wmlo#hundredFeet"/> -->
	</owl:NamedIndividual><owl:NamedIndividual rdf:ID="importedOrigin" rdf:type="av7#CountryOfOriginComponents" rdfs:label="Imported"/>
	<owl:NamedIndividual rdf:ID="inch">
		<rdf:type rdf:resource="av7#PackType"/>
		<rdf:type rdf:resource="av7#SpatialUOM"/>
		<rdfs:label rdf:parseType="Resource">
			<rdf:li rdf:value="in"/>
			<rdf:li rdf:value="IN"/>
			<rdf:li rdf:value="inch"/>
			<rdf:li rdf:value="Inch"/>
			<rdf:li rdf:value="inches"/>
			<rdf:li rdf:value="Inches"/>
		</rdfs:label>
		<!-- <owl:sameAs rdf:resource="wmlo#inch"/> -->
	</owl:NamedIndividual><owl:NamedIndividual rdf:ID="indiaRupee">
		<rdf:type rdf:resource="av7#PriceUOM"/>
		<rdfs:label>
			<rdf:Bag>
				<rdf:li rdf:value="INR"/>
				<rdf:li rdf:value="Indian Rupee"/>
			</rdf:Bag>
		</rdfs:label>
		<!-- <owl:sameAs rdf:resource="wmlo#INR_IndiaRupee"/> -->
	</owl:NamedIndividual><owl:NamedIndividual rdf:ID="internationalHazMat" rdf:type="av7#HazardousMaterialQualifier" rdfs:label="I (International shipping with proper shipping name)"/>
	<owl:NamedIndividual rdf:ID="internetMinimumAdvertisedPrice">
		<rdf:type rdf:resource="av7#PriceQualifier"/>
		<rdfs:label rdf:parseType="Resource">
			<rdf:li rdf:value="IMP"/>
			<rdf:li rdf:value="Internet Minimum Advertised Price"/>
		</rdfs:label>
	</owl:NamedIndividual>
	<owl:NamedIndividual rdf:ID="japanYen">
		<rdf:type rdf:resource="av7#PriceUOM"/>
		<rdfs:label>
			<rdf:Bag>
				<rdf:li rdf:value="JPY"/>
				<rdf:li rdf:value="Japanese Yen"/>
			</rdf:Bag>
		</rdfs:label>
		<!-- <owl:sameAs rdf:resource="wmlo#JPY_JapanYen"/> -->
	</owl:NamedIndividual><owl:NamedIndividual rdf:ID="jar" rdf:type="av7#PackType">
		<rdfs:label rdf:parseType="Resource">
			<rdf:li rdf:value="JR"/>
			<rdf:li rdf:value="jar"/>
		</rdfs:label>
		<!-- <owl:sameAs rdf:resource="wmlo#jar"/> -->
	</owl:NamedIndividual><owl:NamedIndividual rdf:ID="keg" rdf:type="av7#PackType">
		<rdfs:label rdf:parseType="Resource">
			<rdf:li rdf:value="KE"/>
			<rdf:li rdf:value="keg"/>
		</rdfs:label>
		<!-- <owl:sameAs rdf:resource="wmlo#keg"/> -->
	</owl:NamedIndividual><owl:NamedIndividual rdf:ID="kilogram">
		<rdf:type rdf:resource="av7#PackType"/>
		<rdf:type rdf:resource="av7#PackWeightUOM"/>
		<rdfs:label rdf:parseType="Resource">
			<rdf:li rdf:value="KG"/>
			<rdf:li rdf:value="kilogram"/>
		</rdfs:label>
		<!-- <owl:sameAs rdf:resource="wmlo#kilogram"/> -->
	</owl:NamedIndividual><owl:NamedIndividual rdf:ID="leastDanger" rdf:type="av7#PackingGroup" rdfs:label="Group III: Least Danger"/>
	<owl:NamedIndividual rdf:ID="listPrice">
		<rdf:type rdf:resource="av7#PriceQualifier"/>
		<rdfs:label rdf:parseType="Resource">
			<rdf:li rdf:value="LRP"/>
			<rdf:li rdf:value="List Price"/>
		</rdfs:label>
	</owl:NamedIndividual>
	<owl:NamedIndividual rdf:ID="liter">
		<rdf:type rdf:resource="av7#PackType"/>
		<rdf:type rdf:resource="av7#PackVolumeUOM"/>
		<rdfs:label rdf:parseType="Resource">
			<rdf:li rdf:value="LT"/>
			<rdf:li rdf:value="liter"/>
		</rdfs:label>
		<!-- <owl:sameAs rdf:resource="wmlo#liter"/> -->
	</owl:NamedIndividual>
	<owl:NamedIndividual rdf:ID="manufacturerSuggestedRetailPrice">
		<rdf:type rdf:resource="av7#PriceQualifier"/>
		<rdfs:label rdf:parseType="Resource">
			<rdf:li rdf:value="MSR"/>
			<rdf:li rdf:value="Manufacturer Suggested Retail Price"/>
		</rdfs:label>
	</owl:NamedIndividual>
	<owl:NamedIndividual rdf:ID="marketRetailPrice">
		<rdf:type rdf:resource="av7#PriceQualifier"/>
		<rdfs:label rdf:parseType="Resource">
			<rdf:li rdf:value="RTL"/>
			<rdf:li rdf:value="Market Retail Price"/>
		</rdfs:label>
	</owl:NamedIndividual>
	<owl:NamedIndividual rdf:ID="matureRating" rdf:type="av7#ESRBRating" rdfs:label="Mature"/>
	<owl:NamedIndividual rdf:ID="mediumDanger" rdf:type="av7#PackingGroup" rdfs:label="Group II: Medium Danger"/>
	<owl:NamedIndividual rdf:ID="megahertz" rdfs:type="av7#ProcessorSpeedUOM" rdfs:label="MHz"/>
	<owl:NamedIndividual rdf:ID="meter">
		<rdf:type rdf:resource="av7#PackType"/>
		<rdf:type rdf:resource="av7#SpatialUOM"/>
		<rdfs:label rdf:parseType="Resource">
			<rdf:li rdf:value="MR"/>
			<rdf:li rdf:value="ME"/>
			<rdf:li rdf:value="meter"/>
		</rdfs:label>
		<!-- <owl:sameAs rdf:resource="wmlo#meter"/> -->
	</owl:NamedIndividual><owl:NamedIndividual rdf:ID="mexicoPeso">
		<rdf:type rdf:resource="av7#PriceUOM"/>
		<rdfs:label>
			<rdf:Bag>
				<rdf:li rdf:value="MXN"/>
				<rdf:li rdf:value="Mexican Peso"/>
			</rdf:Bag>
		</rdfs:label>
		<!-- <owl:sameAs rdf:resource="wmlo#MXN_MexicoPeso"/> -->
	</owl:NamedIndividual><owl:NamedIndividual rdf:ID="milligram" rdf:type="av7#PackType">
		<rdfs:label rdf:parseType="Resource">
			<rdf:li rdf:value="ME"/>
			<rdf:li rdf:value="milligram"/>
		</rdfs:label>
		<!-- <owl:sameAs rdf:resource="wmlo#milligram"/> -->
	</owl:NamedIndividual><owl:NamedIndividual rdf:ID="milliliter">
		<rdf:type rdf:resource="av7#PackType"/>
		<rdf:type rdf:resource="av7#PackVolumeUOM"/>
		<rdfs:label rdf:parseType="Resource">
			<rdf:li rdf:value="ML"/>
			<rdf:li rdf:value="milliliter"/>
		</rdfs:label>
	</owl:NamedIndividual>
	<owl:NamedIndividual rdf:ID="millimeter">
		<rdf:type rdf:resource="av7#PackType"/>
		<rdf:type rdf:resource="av7#SpatialUOM"/>
		<rdfs:label rdf:parseType="Resource">
			<rdf:li rdf:value="mm"/>
			<rdf:li rdf:value="MM"/>
			<rdf:li rdf:value="millimeter"/>
			<rdf:li rdf:value="Millimeter"/>
			<rdf:li rdf:value="millimeters"/>
			<rdf:li rdf:value="Millimeters"/>
		</rdfs:label>
		<!-- <owl:sameAs rdf:resource="wmlo#milliliter"/> -->
	</owl:NamedIndividual><owl:NamedIndividual rdf:ID="minute">
		<rdf:type rdf:resource="av7#OpenTimeUOM"/>
		<rdf:type rdf:resource="av7#WorkingTimeUOM"/>
		<rdfs:label rdf:parseType="Resource">
			<rdf:li rdf:value="minute"/>
			<rdf:li rdf:value="minutes"/>
		</rdfs:label>
	</owl:NamedIndividual>
	<owl:NamedIndividual rdf:ID="nafCompositeWood" rdf:type="av7#CompositeWoodCertificationCode">
		<rdfs:label rdf:parseType="Resource">
			<rdf:li rdf:value="D"/>
			<rdf:li rdf:value="Product is compliant with NAF (no added formaldehyde) as certified by CARB."/>
		</rdfs:label>
	</owl:NamedIndividual>
	<owl:NamedIndividual rdf:ID="ninePack" rdf:type="av7#PackType">
		<rdfs:label rdf:parseType="Resource">
			<rdf:li rdf:value="P9"/>
			<rdf:li rdf:value="nine pack"/>
		</rdfs:label>
		<!-- <owl:sameAs rdf:resource="wmlo#ninePack"/> -->
	</owl:NamedIndividual><owl:NamedIndividual rdf:ID="noCompositeWood" rdf:type="av7#CompositeWoodCertificationCode">
		<rdfs:label rdf:parseType="Resource">
			<rdf:li rdf:value="A"/>
			<rdf:li rdf:value="Does not contain composite wood."/>
		</rdfs:label>
	</owl:NamedIndividual>
	<owl:NamedIndividual rdf:ID="northKoreaWon">
		<rdf:type rdf:resource="av7#PriceUOM"/>
		<rdfs:label>
			<rdf:Bag>
				<rdf:li rdf:value="KPW"/>
				<rdf:li rdf:value="North Korean Won"/>
			</rdf:Bag>
		</rdfs:label>
		<!-- <owl:sameAs rdf:resource="wmlo#KPW_NorthKoreaYen"/> -->
	</owl:NamedIndividual><owl:NamedIndividual rdf:ID="ohm">
		<rdf:type rdf:resource="av7#UsagePerTimeUOM"/>
		<rdfs:label>
			<rdf:Alt>
				<rdf:li rdf:value="O"/>
				<rdf:li rdf:value="Ohm"/>
			</rdf:Alt>
		</rdfs:label>
		<!-- <owl:sameAs rdf:resource="wmlo#ohm"/> -->
	</owl:NamedIndividual><owl:NamedIndividual rdf:ID="ounce">
		<rdf:type rdf:resource="av7#PackType"/>
		<rdf:type rdf:resource="av7#PackWeightUOM"/>
		<rdfs:label rdf:parseType="Resource">
			<rdf:li rdf:value="OZ"/>
			<rdf:li rdf:value="ounce"/>
		</rdfs:label>
		<!-- <owl:sameAs rdf:resource="wmlo#ounce"/> -->
	</owl:NamedIndividual><owl:NamedIndividual rdf:ID="package" rdf:type="av7#PackType">
		<rdfs:label rdf:parseType="Resource">
			<rdf:li rdf:value="PK"/>
			<rdf:li rdf:value="package"/>
		</rdfs:label>
		<!-- <owl:sameAs rdf:resource="wmlo#package"/> -->
	</owl:NamedIndividual><owl:NamedIndividual rdf:ID="pair" rdf:type="av7#PackType">
		<rdfs:label rdf:parseType="Resource">
			<rdf:li rdf:value="PR"/>
			<rdf:li rdf:value="pair"/>
		</rdfs:label>
		<!-- <owl:sameAs rdf:resource="wmlo#pair"/> -->
	</owl:NamedIndividual><owl:NamedIndividual rdf:ID="pallet">
		<rdf:type rdf:resource="av7#PackType"/>
		<rdf:type rdf:resource="av7#LoadOrderingFactorUOM"/>
		<rdfs:label rdf:parseType="Resource">
			<rdf:li rdf:value="PL"/>
			<rdf:li rdf:value="pallet unit/load"/>
		</rdfs:label>
		<!-- <owl:sameAs rdf:resource="wmlo#pallet"/> -->
	</owl:NamedIndividual>
	<owl:NamedIndividual rdf:ID="pendingRating" rdf:type="av7#ESRBRating" rdfs:label="Rating Pending"/>
	<owl:NamedIndividual rdf:ID="perishable">
		<rdf:type rdf:resource="av7#SpecialHandlingCode"/>
		<rdfs:label rdf:parseType="Resource">
			<rdf:li rdf:value="OPR"/>
			<rdf:li rdf:value="Perishable"/>
		</rdfs:label>
	</owl:NamedIndividual>
	<owl:NamedIndividual rdf:ID="phaseThreeCompositeWood" rdf:type="av7#CompositeWoodCertificationCode">
		<rdfs:label rdf:parseType="Resource">
			<rdf:li rdf:value="C"/>
			<rdf:li rdf:value="Product is compliant with phase 2 emission levels."/>
		</rdfs:label>
	</owl:NamedIndividual>
	<owl:NamedIndividual rdf:ID="phaseTwoCompositeWood" rdf:type="av7#CompositeWoodCertificationCode">
		<rdfs:label rdf:parseType="Resource">
			<rdf:li rdf:value="B"/>
			<rdf:li rdf:value="Product is compliant with phase 2 emission levels. Not legal for sale in California."/>
		</rdfs:label>
	</owl:NamedIndividual>
	<owl:NamedIndividual rdf:ID="piecePack" rdf:type="av7#PackType">
		<rdfs:label rdf:parseType="Resource">
			<rdf:li rdf:value="PC"/>
			<rdf:li rdf:value="piece"/>
		</rdfs:label>
		<!-- <owl:sameAs rdf:resource="wmlo#piece"/> -->
	</owl:NamedIndividual><owl:NamedIndividual rdf:ID="pint">
		<rdf:type rdf:resource="av7#PackType"/>
		<rdf:type rdf:resource="av7#PackVolumeUOM"/>
		<rdfs:label rdf:parseType="Resource">
			<rdf:li rdf:value="PT"/>
			<rdf:li rdf:value="pint"/>
		</rdfs:label>
	</owl:NamedIndividual>
	<owl:NamedIndividual rdf:ID="pound">
		<rdf:type rdf:resource="av7#PackType"/>
		<rdf:type rdf:resource="av7#LoadOrderingFactorUOM"/>
		<rdf:type rdf:resource="av7#PackWeightUOM"/>
		<rdfs:label rdf:parseType="Resource">
			<rdf:li rdf:value="LB"/>
			<rdf:li rdf:value="pound"/>
		</rdfs:label>
		<!-- <owl:sameAs rdf:resource="wmlo#poundAvoirdupois"/> -->
	</owl:NamedIndividual><owl:NamedIndividual rdf:ID="protectFromHeat">
		<rdf:type rdf:resource="av7#SpecialHandlingCode"/>
		<rdfs:label rdf:parseType="Resource">
			<rdf:li rdf:value="PFH"/>
			<rdf:li rdf:value="Protect From Heat"/>
		</rdfs:label>
	</owl:NamedIndividual>
	<owl:NamedIndividual rdf:ID="quart">
		<rdf:type rdf:resource="av7#PackType"/>
		<rdf:type rdf:resource="av7#PackVolumeUOM"/>
		<rdfs:label rdf:parseType="Resource">
			<rdf:li rdf:value="QT"/>
			<rdf:li rdf:value="quart"/>
		</rdfs:label>
		<!-- <owl:sameAs rdf:resource="wmlo#quartUSA"/> -->
	</owl:NamedIndividual><owl:NamedIndividual rdf:ID="purchaseWithPurchase">
		<rdf:type rdf:resource="av7#SpecialItemCode"/>
		<rdfs:label>
			<rdf:Alt>
				<rdf:li rdf:value="PW"/>
				<rdf:li rdf:value="Purchase With Purchase"/>
			</rdf:Alt>
		</rdfs:label>
	</owl:NamedIndividual>
	<owl:NamedIndividual rdf:ID="ratedG" rdf:type="av7#MPAARating" rdfs:label="G"/>
	<owl:NamedIndividual rdf:ID="ratedNCSeventeen" rdf:type="av7#MPAARating" rdfs:label="NC-17"/>
	<owl:NamedIndividual rdf:ID="ratedPG" rdf:type="av7#MPAARating" rdfs:label="PG"/>
	<owl:NamedIndividual rdf:ID="ratedPGThirteen" rdf:type="av7#MPAARating" rdfs:label="PG-13"/>
	<owl:NamedIndividual rdf:ID="ratedR" rdf:type="av7#MPAARating" rdfs:label="R"/>
	<owl:NamedIndividual rdf:ID="ratedUnrated" rdf:type="av7#MPAARating" rdfs:label="Unrated"/>
	<owl:NamedIndividual rdf:ID="ratedX" rdf:type="av7#MPAARating" rdfs:label="X"/>
	<owl:NamedIndividual rdf:ID="refrigerated">
		<rdf:type rdf:resource="av7#SpecialHandlingCode"/>
		<rdfs:label rdf:parseType="Resource">
			<rdf:li rdf:value="MRF"/>
			<rdf:li rdf:value="Refrigerated"/>
		</rdfs:label>
	</owl:NamedIndividual>
	<owl:NamedIndividual rdf:ID="returnForCredit">
		<rdf:type rdf:resource="av7#ReturnCode"/>
		<rdfs:label>
			<rdf:Alt>
				<rdf:li rdf:value="RFC"/>
				<rdf:li rdf:value="return for credit"/>
			</rdf:Alt>
		</rdfs:label>
	</owl:NamedIndividual>
	<owl:NamedIndividual rdf:ID="roll" rdf:type="av7#PackType">
		<rdfs:label rdf:parseType="Resource">
			<rdf:li rdf:value="RL"/>
			<rdf:li rdf:value="roll"/>
		</rdfs:label>
		<!-- <owl:sameAs rdf:resource="wmlo#roll"/> -->
	</owl:NamedIndividual><owl:NamedIndividual rdf:ID="russiaRuble">
		<rdf:type rdf:resource="av7#PriceUOM"/>
		<rdfs:label>
			<rdf:Bag>
				<rdf:li rdf:value="RUB"/>
				<rdf:li rdf:value="Russian Ruble"/>
			</rdf:Bag>
		</rdfs:label>
		<!-- <owl:sameAs rdf:resource="wmlo#RUB_RussiaRuble"/> -->
	</owl:NamedIndividual><owl:NamedIndividual rdf:ID="second">
		<rdf:type rdf:resource="av7#OpenTimeUOM"/>
		<rdf:type rdf:resource="av7#WorkingTimeUOM"/>
		<rdfs:label rdf:value="seconds"/>
	</owl:NamedIndividual>
	<owl:NamedIndividual rdf:ID="sevenPack" rdf:type="av7#PackType">
		<rdfs:label rdf:parseType="Resource">
			<rdf:li rdf:value="P7"/>
			<rdf:li rdf:value="seven pack"/>
		</rdfs:label>
		<!-- <owl:sameAs rdf:resource="wmlo#sevenPack"/> -->
	</owl:NamedIndividual>
	<owl:NamedIndividual rdf:ID="sheet" rdf:type="av7#PackType">
		<rdfs:label rdf:parseType="Resource">
			<rdf:li rdf:value="SH"/>
			<rdf:li rdf:value="sheet"/>
		</rdfs:label>
		<!-- <owl:sameAs rdf:resource="wmlo#sheet"/> -->
	</owl:NamedIndividual>
	<owl:NamedIndividual rdf:ID="sixPack" rdf:type="av7#PackType">
		<rdfs:label rdf:parseType="Resource">
			<rdf:li rdf:value="P6"/>
			<rdf:li rdf:value="six pack"/>
		</rdfs:label>
		<!-- <owl:sameAs rdf:resource="wmlo#sixPack"/> -->
	</owl:NamedIndividual><owl:NamedIndividual rdf:ID="southKoreanWon">
		<rdf:type rdf:resource="av7#PriceUOM"/>
		<rdfs:label>
			<rdf:Bag>
				<rdf:li rdf:value="KRW"/>
				<rdf:li rdf:value="South Korean Won"/>
			</rdf:Bag>
		</rdfs:label>
		<!-- <owl:sameAs rdf:resource="wmlo#KRW_SouthKoreaYen"/> -->
	</owl:NamedIndividual><owl:NamedIndividual rdf:ID="squareFoot">
		<rdf:type rdf:resource="av7#CoverageAreaUOM"/>
		<rdf:type rdf:resource="av7#PackType"/>
		<rdf:type rdf:resource="av7#SpreadRateUOM"/>
		<rdfs:label rdf:parseType="Resource">
			<rdf:li rdf:value="SF"/>
			<rdf:li rdf:value="square foot"/>
			<rdf:li rdf:value="square feet"/>
		</rdfs:label>
		<!-- <owl:sameAs rdf:resource="wmlo#squareFoot"/> -->
	</owl:NamedIndividual><owl:NamedIndividual rdf:ID="squareMeter">
		<rdf:type rdf:resource="av7#CoverageAreaUOM"/>
		<rdf:type rdf:resource="av7#SpreadRateUOM"/>
		<rdfs:label rdf:parseType="Resource">
			<rdf:li rdf:value="SM"/>
			<rdf:li rdf:value="square meter"/>
			<rdf:li rdf:value="square meters"/>
		</rdfs:label>
	</owl:NamedIndividual>
	<owl:NamedIndividual rdf:ID="teenRating" rdf:type="av7#ESRBRating" rdfs:label="Teen"/>
	<owl:NamedIndividual rdf:ID="threePack" rdf:type="av7#PackType">
		<rdfs:label rdf:parseType="Resource">
			<rdf:li rdf:value="P3"/>
			<rdf:li rdf:value="three pack"/>
		</rdfs:label>
	</owl:NamedIndividual>
	<owl:NamedIndividual rdf:ID="twelvePack" rdf:type="av7#PackType">
		<rdfs:label rdf:parseType="Resource">
			<rdf:li rdf:value="12"/>
			<rdf:li rdf:value="pack"/>
			<rdf:li rdf:value="12 pack"/>
		</rdfs:label>
		<!-- <owl:sameAs rdf:resource="wmlo#twelvePack"/> -->
	</owl:NamedIndividual><owl:NamedIndividual rdf:ID="twoPack" rdf:type="av7#PackType">
		<rdfs:label rdf:parseType="Resource">
			<rdf:li rdf:value="OP"/>
			<rdf:li rdf:value="two pack"/>
		</rdfs:label>
		<!-- <owl:sameAs rdf:resource="wmlo#twoPack"/> -->
	</owl:NamedIndividual><owl:NamedIndividual rdf:ID="ulefCompositeWood" rdf:type="av7#CompositeWoodCertificationCode">
		<rdfs:label rdf:parseType="Resource">
			<rdf:li rdf:value="E"/>
			<rdf:li rdf:value="Product is compliant with ULEF (ultra low emitting formaldehyde) as certified by CARB."/>
		</rdfs:label>
	</owl:NamedIndividual>
	<owl:NamedIndividual rdf:ID="unilateralMinimumAdvertisedPrice">
		<rdf:type rdf:resource="av7#PriceQualifier"/>
		<rdfs:label rdf:parseType="Resource">
			<rdf:li rdf:value="UMA"/>
			<rdf:li rdf:value="Unilateral Minimum Advertised Price"/>
		</rdfs:label>
	</owl:NamedIndividual>
	<owl:NamedIndividual rdf:ID="unit" rdf:type="av7#LoadOrderingFactorUOM">
		<rdfs:label rdf:parseType="Resource">
			<rdf:li rdf:value="UNIT"/>
			<rdf:li rdf:value="unit"/>
		</rdfs:label>
	</owl:NamedIndividual>
	<owl:NamedIndividual rdf:ID="unitCostPrice">
		<skos:closeMatch rdf:resource=""/>
		<rdf:type rdf:resource="av7#PriceQualifier"/>
		<rdfs:label rdf:parseType="Resource">
			<rdf:li rdf:value="UCP"/>
			<rdf:li rdf:value="Unit Cost Price"/>
		</rdfs:label>
	</owl:NamedIndividual>
	<owl:NamedIndividual rdf:ID="unitedStatesDollar">
		<rdf:type rdf:resource="av7#PriceUOM"/>
		<rdfs:label>
			<rdf:Bag>
				<rdf:li rdf:value="USD"/>
				<rdf:li rdf:value="United States Dollar"/>
			</rdf:Bag>
		</rdfs:label>
		<!-- <owl:sameAs rdf:resource="wmlo#USD_UnitedStatesDollar"/> -->
	</owl:NamedIndividual><owl:NamedIndividual rdf:ID="unratedRating" rdf:type="av7#ESRBRating" rdfs:label="Unrated"/>
	<owl:NamedIndividual rdf:ID="usaAndImportedOrigin" rdf:type="av7#CountryOfOriginComponents" rdfs:label="USA and Imported"/>
	<owl:NamedIndividual rdf:ID="usaOrigin" rdf:type="av7#CountryOfOriginComponents" rdfs:label="USA"/>
	<owl:NamedIndividual rdf:ID="usaOrImportedOrigin" rdf:type="av7#CountryOfOriginComponents" rdfs:label="USA or Imported"/>
	<owl:NamedIndividual rdf:ID="volt">
		<rdf:type rdf:resource="av7#UsagePerTimeUOM"/>
		<rdfs:label>
			<rdf:Alt>
				<rdf:li rdf:value="V"/>
				<rdf:li rdf:value="Volt"/>
			</rdf:Alt>
		</rdfs:label>
		<!-- <owl:sameAs rdf:resource="wmlo#volt"/> -->
	</owl:NamedIndividual><owl:NamedIndividual rdf:ID="waterHazMat" rdf:type="av7#HazardousMaterialQualifier" rdfs:label="W (Shipping by water with rules)"/>
	<owl:NamedIndividual rdf:ID="watt">
		<rdf:type rdf:resource="av7#UsagePerTimeUOM"/>
		<rdfs:label>
			<rdf:Alt>
				<rdf:li rdf:value="W"/>
				<rdf:li rdf:value="Watt"/>
			</rdf:Alt>
		</rdfs:label>
		<!-- <owl:sameAs rdf:resource="wmlo#watt"/> -->
	</owl:NamedIndividual>
	<owl:NamedIndividual rdf:ID="week" rdf:type="av7#OrderLeadTimeCode" rdfs:label="week"/>
	<owl:NamedIndividual rdf:ID="wholesalePrice">
		<rdf:type rdf:resource="av7#PriceQualifier"/>
		<rdfs:label rdf:parseType="Resource">
			<rdf:li rdf:value="WHL"/>
			<rdf:li rdf:value="Wholesale Price"/>
		</rdfs:label>
	</owl:NamedIndividual>
	<owl:NamedIndividual rdf:ID="yard">
		<rdf:type rdf:resource="av7#PackType"/>
		<rdf:type rdf:resource="av7#SpatialUOM"/>
		<rdfs:label rdf:parseType="Resource">
			<rdf:li rdf:value="YD"/>
			<rdf:li rdf:value="yard"/>
		</rdfs:label>
	</owl:NamedIndividual>
	<owl:DatatypeProperty rdf:ID="hasAccessoriesEquipmentIncluded">
		<rdfs:subPropertyOf rdf:resource="av7#accessoriesEquipmentIncluded"/>
		<rdfs:label>Has Accessories/Equipment Included</rdfs:label>
		<rdfs:comment>Indicates whether or not the represented item includes accessories or equipment.</rdfs:comment>
		<rdfs:range rdf:resource="xsd#boolean"/>
	</owl:DatatypeProperty>
	<owl:AnnotationProperty rdf:ID="accessoriesEquipmentIncludedDescription">
		<rdfs:subPropertyOf rdf:resource="av7#accessoriesEquipmentIncluded"/>
		<rdfs:label>Accessories/Equipment Included Description</rdfs:label>
		<rdfs:comment>Describes the accessories or equipment wihch the represented item includes.</rdfs:comment>
		<rdfs:range>
			<owl:equivalentClass>
				<owl:complementOf rdf:resource="xsd#boolean"/>
			</owl:equivalentClass>
		</rdfs:range>
	</owl:AnnotationProperty>
	<owl:AnnotationProperty rdf:ID="activationMeans">
		<rdfs:label>
			<rdf:Bag>
				<rdf:li rdf:value="Activation Means"/>
				<rdf:li rdf:value="Activation Means 1"/>
				<rdf:li rdf:value="Activation Means 2"/>
			</rdf:Bag>
		</rdfs:label>
		<rdfs:comment>Indicates the means by which the represented item becomes ready for use.</rdfs:comment>
	</owl:AnnotationProperty>
	<owl:AnnotationProperty rdf:ID="activationSwitchLocation">
		<rdfs:label>
			<rdf:Bag>
				<rdf:li rdf:value="Activation Switch Location"/>
				<rdf:li rdf:value="Activation Switch Location 1"/>
				<rdf:li rdf:value="Activation Switch Location 2"/>
			</rdf:Bag>
		</rdfs:label>
		<rdfs:comment>Indicates where on a given item the activation, start, or on button is located.</rdfs:comment>
	</owl:AnnotationProperty>
	<owl:DatatypeProperty rdf:ID="adaCompliant">
		<rdfs:label>ADA Compliant</rdfs:label>
		<rdfs:comment>Indicates whether or not manufacturing or selling agents believe that the represented item is in compliance with standards set forth by the Americans with Disabilities Act.</rdfs:comment>
		<av7:userNotes>The ADA does not have compliance provisions for consumer products; users should assume that this attribute does not refer to a legal designation.</av7:userNotes>
		<rdfs:range rdf:resource="xsd#boolean"/>
	</owl:DatatypeProperty>
	<owl:AnnotationProperty rdf:ID="adhesiveRecommendation">
		<rdfs:label>Adhesive Recommendation</rdfs:label>
		<rdfs:comment>Indicates the specific product name or specific type of adhesive recommended for use with the represented item.</rdfs:comment>
	</owl:AnnotationProperty>
	<owl:DatatypeProperty rdf:ID="adjustableHosel">
		<rdfs:label>Adjustable Hosel</rdfs:label>
		<rdfs:comment>Indicates whether or not the represented item's hosel is adjustable.</rdfs:comment>
		<rdfs:range rdf:resource="xsd#boolean"/>
	</owl:DatatypeProperty>
	<owl:DatatypeProperty rdf:ID="adjustableLie">
		<rdfs:label>Adjustable Lie</rdfs:label>
		<rdfs:comment>Indicates whether or not the represented club's lie angle is adjustable.</rdfs:comment>
		<rdfs:range rdf:resource="xsd#boolean"/>
	</owl:DatatypeProperty>
	<owl:DatatypeProperty rdf:ID="adjustableLoft">
		<rdfs:label>Adjustable Loft</rdfs:label>
		<rdfs:comment>Indicates whether or not the represent club's loft is adjustable.</rdfs:comment>
		<rdfs:range rdf:resource="xsd#boolean"/>
	</owl:DatatypeProperty>
	<owl:DatatypeProperty rdf:ID="adjustableObjective">
		<rdfs:label>Adjustable Objective</rdfs:label>
		<rdfs:comment>Indicates whether or not the represented scope or other optical targeting device is able to quickly switch between multiple targets.</rdfs:comment>
		<rdfs:range rdf:resource="xsd#boolean"/>
	</owl:DatatypeProperty>
	<owl:DatatypeProperty rdf:ID="adjustableStrap">
		<rdfs:label>Adjustable Strap</rdfs:label>
		<rdfs:comment>Indicates whether or not the represented item includes an adjustable strap.</rdfs:comment>
		<rdfs:range rdf:resource="xsd#boolean"/>
	</owl:DatatypeProperty>
	<owl:DatatypeProperty rdf:ID="adjustableWeights">
		<rdfs:label>Adjustable Weights</rdfs:label>
		<rdfs:comment>Indicates whether or not the represented item's loft, lie, and face angle are adjustable.</rdfs:comment>
		<rdfs:range rdf:resource="xsd#boolean"/>
	</owl:DatatypeProperty>
	<owl:AnnotationProperty rdf:ID="advertisedOrigin">
		<rdfs:label>Advertised Origin</rdfs:label>
		<rdfs:comment>The advertised origin of the represented item.</rdfs:comment>
	</owl:AnnotationProperty>
	<owl:DatatypeProperty rdf:ID="adultsOnly">
		<rdfs:label>Adults Only</rdfs:label>
		<rdfs:comment>Indicates whether or not an item is intended for adults only.</rdfs:comment>
		<av7:userNotes>'Adult' is typically defined as 18 years or older.</av7:userNotes>
		<rdfs:range rdf:resource="xsd#boolean"/>
	</owl:DatatypeProperty>
	<owl:DatatypeProperty rdf:ID="aerosol">
		<rdfs:label>Aerosol</rdfs:label>
		<rdfs:comment>Indicates whether or not the represented item is an aerosol, or a compressed liquid or gas soluable in the atmosphere.</rdfs:comment>
		<rdfs:range rdf:resource="xsd#boolean"/>
	</owl:DatatypeProperty>
	<owl:ObjectProperty rdf:ID="ageGroup">
		<rdfs:label>Age Group</rdfs:label>
		<rdfs:comment>Comprises a general grouping of human ages.</rdfs:comment>
	</owl:ObjectProperty>
	<owl:AnnotationProperty rdf:ID="ageRange">
		<rdfs:label>Age Range</rdfs:label>
		<rdfs:comment>Indicates the recommended age range for a represented item.</rdfs:comment>
	</owl:AnnotationProperty>
	<owl:AnnotationProperty rdf:ID="alcoholContentByVolume">
		<rdfs:label>Alcohol Content By Volume</rdfs:label>
		<rdfs:comment>Measures the percentage of alcohol measured against the total volume of the represented item.</rdfs:comment>
	</owl:AnnotationProperty>
	<owl:DatatypeProperty rdf:ID="amps">
		<rdfs:label>Amps</rdfs:label>
		<rdfs:comment>Indicates the amperage associated with the represented item.</rdfs:comment>
		<rdfs:range rdf:resource="xsd#float"/>
	</owl:DatatypeProperty>
	<owl:AnnotationProperty rdf:ID="ansiStandard">
		<rdfs:label>ANSI Standard</rdfs:label>
		<rdfs:comment>Indicates ANSI standards pertaining to the represented item.</rdfs:comment>
		<sorg:relatedLink rdf:resource="http://webstore.ansi.org"/>
	</owl:AnnotationProperty>
	<owl:AnnotationProperty rdf:ID="apparelDepartment">
		<rdfs:label>Apparel Department</rdfs:label>
		<rdfs:comment>Indicate the department or category in which ertailers might display the represented item.</rdfs:comment>
	</owl:AnnotationProperty>
	<owl:AnnotationProperty rdf:ID="applicationProductUsage">
		<rdfs:label>Application/Product Usage</rdfs:label>
		<rdfs:comment>Describes the best or recommended use of the product.</rdfs:comment>
	</owl:AnnotationProperty>
	<owl:DatatypeProperty rdf:ID="assemblyRequired">
		<rdfs:label>Assembly Required</rdfs:label>
		<rdfs:comment>Indicates whether or not an item requires consumer assembly.</rdfs:comment>
		<rdfs:range rdf:resource="xsd#boolean"/>
	</owl:DatatypeProperty>
	<owl:AnnotationProperty rdf:ID="athlete">
		<rdfs:label>Athlete</rdfs:label>
		<rdfs:comment>Idenfies the athlete (by name or number) endorsing or featured on the represented item.</rdfs:comment>
	</owl:AnnotationProperty>
	<owl:AnnotationProperty rdf:ID="attachmentType">
		<rdfs:label>
			<rdf:Bag>
				<rdf:li rdf:value="Attachment Type"/>
				<rdf:li rdf:value="Attachment Type 1"/>
				<rdf:li rdf:value="Attachment Type 2"/>
				<rdf:li rdf:value="Attachment Type 3"/>
			</rdf:Bag>
		</rdfs:label>
		<rdfs:comment>Indicates what may be attached to a represented item; in particular to the kit or object being attached (i.e. bayonette; flashlight; camera), perhaps by means of the value of 'Mount Type.'</rdfs:comment>
	</owl:AnnotationProperty>
	<owl:DatatypeProperty rdf:ID="audioLineIn">
		<rdfs:label>Audio Line In</rdfs:label>
		<rdfs:comment>Indicates the number of audio input jacks onboard or supported by a represented item.</rdfs:comment>
		<rdfs:range rdf:resource="xsd#integer"/>
	</owl:DatatypeProperty>
	<owl:DatatypeProperty rdf:ID="audioLineOut">
		<rdfs:label>Audio Line Out</rdfs:label>
		<rdfs:comment>Indicates the number of audio output jacks onboard or supported by a represented item.</rdfs:comment>
		<rdfs:range rdf:resource="xsd#integer"/>
	</owl:DatatypeProperty>
	<owl:AnnotationProperty rdf:ID="author">
		<rdfs:label>Author</rdfs:label>
		<rdfs:comment>Names the author of the represented publication.</rdfs:comment>
	</owl:AnnotationProperty>
	<owl:DatatypeProperty rdf:ID="autoShutoff">
		<rdfs:label>Auto Shutoff</rdfs:label>
		<rdfs:comment>Indicates whether or not the represented item has an automatic shutoff, or a means to turn off without human intervention.</rdfs:comment>
		<rdfs:range rdf:resource="xsd#boolean"/>
	</owl:DatatypeProperty>
	<owl:DatatypeProperty rdf:ID="availableDate">
		<rdfs:label>Available Date</rdfs:label>
		<rdfs:comment>The date the item is available to the retailer for purchase.</rdfs:comment>
		<av7:userNotes>Format varies by upload and explort method. UI and spreadsheet: mm/dd/yyyy; RSX: yyyy-mm-dd.</av7:userNotes>
		<rdfs:range rdf:resource="av7#VariableDate"/>
	</owl:DatatypeProperty>
	<owl:DatatypeProperty rdf:ID="babyFormulaLabelRequired">
		<rdfs:label>Baby Formula Label Required</rdfs:label>
		<rdfs:comment>Indicates whether or not the represented item requires a baby formula label.</rdfs:comment>
		<rdfs:range rdf:resource="xsd#boolean"/>
	</owl:DatatypeProperty>
	<owl:AnnotationProperty rdf:ID="backingType">
		<rdfs:label>Backing Type</rdfs:label>
		<rdfs:comment>Indicates the type of backing on a represented item.</rdfs:comment>
	</owl:AnnotationProperty>
	<owl:AnnotationProperty rdf:ID="ballCoreMaterial">
		<rdfs:label>Ball Core Material</rdfs:label>
		<rdfs:comment>Describes the material that makes up the core of the represented ball.</rdfs:comment>
	</owl:AnnotationProperty>
	<owl:DatatypeProperty rdf:ID="baseCurve">
		<rdfs:label>Base Curve</rdfs:label>
		<rdfs:comment>Measures base curve of a lens in millimeters.</rdfs:comment>
		<rdfs:range rdf:resource="xsd#float"/>
	</owl:DatatypeProperty>
	<owl:AnnotationProperty rdf:ID="batDrop">
		<rdfs:label>Bat Drop</rdfs:label>
		<rdfs:comment>Describes the length-to-weight ratio of a bat.</rdfs:comment>
	</owl:AnnotationProperty>
	<owl:DatatypeProperty rdf:ID="batteryIncluded">
		<rdfs:subPropertyOf rdf:resource="av7#battery"/>
		<rdfs:label>Battery Included</rdfs:label>
		<rdfs:comment>Indicates whether or not the represented item includes a battery or multiple batteries.</rdfs:comment>
		<rdfs:range rdf:resource="xsd#boolean"/>
	</owl:DatatypeProperty>
	<owl:DatatypeProperty rdf:ID="batteryLife">
		<rdfs:label>Battery Life</rdfs:label>
		<rdfs:comment>Estimates the number of hours for which a battery is able to power the represented item with which it is associated.</rdfs:comment>
	</owl:DatatypeProperty>
	<owl:DatatypeProperty rdf:ID="batteryQuantity">
		<rdfs:subPropertyOf rdf:resource="av7#battery"/>
		<rdfs:label>Battery Quantity</rdfs:label>
		<rdfs:comment>Indicates how many batteries a represented item requires in order to operate.</rdfs:comment>
		<rdfs:range rdf:resource="xsd#integer"/>
	</owl:DatatypeProperty>
	<owl:DatatypeProperty rdf:ID="batteryRequired">
		<rdfs:label>Battery Required</rdfs:label>
		<rdfs:comment>Indicates whether or not the represented item requires a battery in order to operate.</rdfs:comment>
		<rdfs:range rdf:resource="xsd#boolean"/>
	</owl:DatatypeProperty>
	<owl:AnnotationProperty rdf:ID="batterySize">
		<rdfs:label>Battery Size</rdfs:label>
		<rdfs:comment>Indicates battery size (and peculiarities, such as rechargeability, etc.).</rdfs:comment>
		<sorg:relatedLink rdf:resource="https://en.wikipedia.org/wiki/List_of_battery_sizes"/>
	</owl:AnnotationProperty>
	<owl:AnnotationProperty rdf:ID="batteryType">
		<rdfs:label>Battery Type</rdfs:label>
		<rdfs:comment>Indicates the type of battery used by the represented item.</rdfs:comment>
	</owl:AnnotationProperty>
	<owl:DatatypeProperty rdf:ID="bearingRollingElements">
		<rdf:subPropertyOf rdf:resource="bearing"/>
		<rdfs:label>Bearing Rolling Elements</rdfs:label>
		<rdfs:comment>Indicates the number of rolling elements in a represented bearing.</rdfs:comment>
		<rdfs:range rdf:resource="xsd#integer"/>
	</owl:DatatypeProperty>
	<owl:ObjectProperty rdf:ID="bearingType">
		<rdf:subPropertyOf rdf:resource="bearing"/>
		<rdfs:label>Bearing Type</rdfs:label>
		<rdfs:comment>Indicates the style of bearing used in the item.</rdfs:comment>
	</owl:ObjectProperty>
	<owl:DatatypeProperty rdf:ID="bendDegree">
		<rdf:subPropertyOf rdf:resource="bend"/>
		<rdfs:label>Bend Degree</rdfs:label>
		<rdfs:comment>Indicates the degree of bend type associated with the represented item.</rdfs:comment>
		<rdfs:range rdf:resource="xsd#float"/>
	</owl:DatatypeProperty>
	<owl:AnnotationProperty rdf:ID="bendType">
		<rdf:subPropertyOf rdf:resource="bend"/>
		<rdfs:label>Bend Type.</rdfs:label>
		<rdfs:comment>Indicates the bend type associated with the represented item.</rdfs:comment>
		<rdfs:range>
			<owl:equivalentClass>
				<owl:complmentOf rdf:resource="xsd#float"/>
			</owl:equivalentClass>
		</rdfs:range>
	</owl:AnnotationProperty>
	<owl:AnnotationProperty rdf:ID="bladderMaterial">
		<rdfs:label>Bladder Material</rdfs:label>
		<rdfs:comment>Indicates the material that makes up the bladder of the represented item.</rdfs:comment>
	</owl:AnnotationProperty>
	<owl:AnnotationProperty rdf:ID="bladePattern">
		<rdfs:label>Blade Pattern</rdfs:label>
		<rdfs:comment>Describes the type of blade curve such as lie, depth, curve, and face.</rdfs:comment>
	</owl:AnnotationProperty>
	<owl:DatatypeProperty rdf:ID="bluetooth">
		<rdfs:label>Bluetooth</rdfs:label>
		<rdfs:comment>Indicates whether or not Bluetooth is supported by a represented item.</rdfs:comment>
		<rdfs:range rdf:resource="xsd#boolean"/>
	</owl:DatatypeProperty>
	<owl:DatatypeProperty rdf:ID="boilingPoint">
		<rdfs:label>Boiling Point</rdfs:label>
		<rdfs:comment>Indicates the temperature at which the represented item beigns to boil.</rdfs:comment>
		<wmlo:userNotes>If this attribute obtains a value, 'Boiling Point UOM' must obtain a value.</wmlo:userNotes>
		<rdfs:range rdf:resource="xsd#float"/>
	</owl:DatatypeProperty>
	<owl:ObjectProperty rdf:ID="boilingPointUOM">
		<rdfs:label>Boiling Point UOM</rdfs:label>
		<rdfs:comment>Qualifies the value of 'Boiling Point.'</rdfs:comment>
		<wmlo:userNotes>If this attribute obtains a value, 'Boiling Point' must obtain a value.</wmlo:userNotes>
		<rdfs:range rdf:resource="av7#TempUOM"/>
	</owl:ObjectProperty>
	<owl:DatatypeProperty rdf:ID="bootLegCircumference">
		<rdfs:label>Boot Leg Circumference</rdfs:label>
		<rdfs:comment>Measures the shaft of the represented boot at its widest part.</rdfs:comment>
		<wmlo:userNotes>If this attribute obtains a value, 'Boot Leg Circumference UOM' must obtain a value.</wmlo:userNotes>
		<rdfs:range rdf:resource="xsd#float"/>
	</owl:DatatypeProperty>
	<owl:ObjectProperty rdf:ID="bootLegCircumferenceUOM">
		<rdfs:label>Boot Leg Circumference UOM</rdfs:label>
		<rdfs:comment>Qualifies the value of 'Boot Leg Circumference.'</rdfs:comment>
		<wmlo:userNotes>If this attribute obtains a value, 'Boot Leg Circumference' must obtain a value.</wmlo:userNotes>
		<rdfs:range rdf:resource="av7#SpatialUOM"/>
	</owl:ObjectProperty>
	<owl:DatatypeProperty rdf:ID="bootShaftHeight">
		<rdfs:label>Boot Shaft Height</rdfs:label>
		<rdfs:comment>Measures the shaft of the represented boot from the middle of hte arch up the outsole to the top of the shaft.</rdfs:comment>
		<wmlo:userNotes>If this attribute obtains a value, 'Boot Shaft Height UOM' must obtain a value.</wmlo:userNotes>
		<rdfs:range rdf:resource="xsd#float"/>
	</owl:DatatypeProperty>
	<owl:ObjectProperty rdf:ID="bootShaftHeightUOM">
		<rdfs:label>Boot Shaft Height UOM</rdfs:label>
		<rdfs:comment>Qualifies the value of 'Boot Shaft Height.'</rdfs:comment>
		<wmlo:userNotes>If this attribute obtains a value, 'Boot Shaft Height' must obtain a value.</wmlo:userNotes>
		<rdfs:range rdf:resource="av7#SpatialUOM"/>
	</owl:ObjectProperty>
	<owl:DatatypeProperty rdf:ID="boxesPerItem">
		<rdfs:label>Boxes Per Item</rdfs:label>
		<rdfs:comment>Indicates the number of boxes required to ship a represented item.</rdfs:comment>
		<rdfs:range rdf:resource="xsd#integer"/>
	</owl:DatatypeProperty>
	<owl:DatatypeProperty rdf:ID="bpaFree">
		<rdfs:label>BPA-Free</rdfs:label>
		<rdfs:comment>Affirms or denies that the represented item does not contain Bisphenol A (BPA).</rdfs:comment>
		<rdfs:range rdf:resource="xsd#boolean"/>
	</owl:DatatypeProperty>
	<owl:DatatypeProperty rdf:ID="braBandSize">
		<rdfs:label>Bra Band Size</rdfs:label>
		<rdfs:comment>Indicates the size of a represented bra band in inches.'</rdfs:comment>
		<rdfs:range rdf:resource="xsd#integer"/>
	</owl:DatatypeProperty>
	<owl:AnnotationProperty rdf:ID="braCupSize">
		<rdfs:label>Bra Cup Size</rdfs:label>
		<rdfs:comment>Indicates the size of a represented bra cup.</rdfs:comment>
	</owl:AnnotationProperty>
	<owl:AnnotationProperty rdf:ID="brand">
		<rdfs:label>Brand</rdfs:label>
		<rdfs:comment>Indicates item brand owner.</rdfs:comment>
	</owl:AnnotationProperty>
	<owl:AnnotationProperty rdf:ID="bridgeFitStyle">
		<rdfs:label>Bridge Fit Style</rdfs:label>
		<rdfs:comment>Indicates how a represented item is intended to fall over the bridge of the nose.</rdfs:comment>
	</owl:AnnotationProperty>
	<owl:DatatypeProperty rdf:ID="bridgeSize">
		<rdfs:label>Bridge Size</rdfs:label>
		<rdfs:comment>Measures the bridge of a nose in millimeters.</rdfs:comment>
		<rdfs:range rdf:resource="xsd#float"/>
	</owl:DatatypeProperty>
	<owl:DatatypeProperty rdf:ID="brightness">
		<rdfs:label>Brightness</rdfs:label>
		<rdfs:comment>The measure of visible light output produced by the represented item. Measured in Lumens.</rdfs:comment>
		<rdfs:range rdf:resource="xsd#float"/>
	</owl:DatatypeProperty>
	<owl:AnnotationProperty rdf:ID="bulbBaseType">
		<rdfs:label>Resource</rdfs:label>
		<rdfs:comment>Indicates the shape of the bulb being described, or the shape of a bulb which is compatible with the represented item.</rdfs:comment>
		<av7:userNotes>While there is no set associated with this attribute, common bulb bases include: 2g11 4-Pin Base, Bi Pin, Candelabra, Double Cont Bay, Double End, E14 Euro Base, Four Pin, Gu24, 4mm for Bi Pin, 6mm for Bi Pin, 8mm for Bi Pin, Looped Bi Pin, Intermediate, Mini Candelabra, Mini Screw, Mogul, Mogul 3 Contact, Mogul End Prong, Mogul Pre-Focus, Other Bases, Single Cont Bay, S Cont Prefocus, Single End, Standard/Medium, Twistlock Mr16, Two Pin, and Wedge.</av7:userNotes>
	</owl:AnnotationProperty>
	<owl:DatatypeProperty rdf:ID="bulbQty">
		<rdf:subPropertyOf rdf:resource="av7#bulb"/>
		<rdfs:label>Resource</rdfs:label>
		<rdfs:comment>The quantity of bulbs required by a represented item.</rdfs:comment>
		<rdfs:range rdf:resource="xsd#integer"/>
	</owl:DatatypeProperty>
	<owl:AnnotationProperty rdf:ID="bulbShape">
		<rdfs:label>Resource</rdfs:label>
		<rdfs:comment>Indicates the shape of the bulb being described, or the shape of a bulb which is compatible with the represented item.</rdfs:comment>
		<av7:userNotes>
			<rdf:Bag>
				<rdf:li
					rdf:value="While there is no set associated with this attribute, common bulb shapes include: A21 Household, A-23, A-25, Appliance, Bt014.5, Bt-15, Bubble Reflecto, CP-19, Chandalierblunt, Chandalierflame, Circular, Compact Fluor, Fan, Fanblunt, Fluorescent, Globe, Gu24 Spring CFL, Household, Lincandescent, Mirrored Reflec, Parabolic, Ps-25, Ps-30, Reflector, Tube, TB-19, and U Lamp Shape. "/>
				<rdf:li rdf:value="If this attribute obtains a value, 'Bulb Base Type' must also obtain a value."/>
			</rdf:Bag>
		</av7:userNotes>
	</owl:AnnotationProperty>
	<owl:AnnotationProperty rdf:ID="bulbType">
		<rdf:subPropertyOf rdf:resource="av7#bulb"/>
		<rdfs:label>Resource</rdfs:label>
		<rdfs:comment>Indicates the type of bulb associated with the represented item.</rdfs:comment>
		<rdfs:range>
			<owl:equivalentClass>
				<owl:complementOf rdf:resource="xsd#integer"/>
			</owl:equivalentClass>
		</rdfs:range>
	</owl:AnnotationProperty>
	<owl:DatatypeProperty rdf:ID="fuelBurnerQuantity">
		<rdfs:subPropertyOf rdf:resource="av7#fuelBurner"/>
		<rdfs:label>Fuel Burner Quantity</rdfs:label>
		<rdfs:comment>Indicates a quantity of fuel burners.</rdfs:comment>
		<rdfs:range rdf:resource="xsd#integer"/>
	</owl:DatatypeProperty>
	<owl:DatatypeProperty rdf:ID="fuelBurnerType">
		<rdfs:subPropertyOf rdf:resource="av7#fuelBurner"/>
		<rdfs:label>Fuel Burner Type</rdfs:label>
		<rdfs:comment>Indicates a type or kind of fuel burner.</rdfs:comment>
		<rdfs:range>
			<owl:equivalentClass>
				<owl:complementOf rdf:resource="xsd#integer"/>
			</owl:equivalentClass>
		</rdfs:range>
	</owl:DatatypeProperty>
	<owl:DatatypeProperty rdf:ID="cableLength">
		<rdfs:label>Cable Length</rdfs:label>
		<rdfs:comment>Indicates the lenght of a cable asociated with a represented item.</rdfs:comment>
		<av7:userNotes>If this attribute obtains a value, 'Cable Length UOM' must also obtain a value.</av7:userNotes>
		<rdfs:range rdf:resource="xsd#float"/>
	</owl:DatatypeProperty>
	<owl:DatatypeProperty rdf:ID="cableLengthUOM">
		<rdfs:label>Cable Length UOM</rdfs:label>
		<rdfs:comment>Qualifies the value of 'Cable Length'.</rdfs:comment>
		<av7:userNotes>If this attribute obtains a value, 'Cable Length' must also obtain a value.</av7:userNotes>
		<rdfs:range rdf:resource="av7#SpatialUOM"/>
	</owl:DatatypeProperty>
	<owl:AnnotationProperty rdf:ID="careInstructions">
		<rdfs:label>Care Instructions</rdfs:label>
		<rdfs:comment>A brief description of how an item should be cleaned, laundered, or otherwise cared for for optimal longevity.</rdfs:comment>
	</owl:AnnotationProperty>
	<owl:AnnotationProperty rdf:ID="carrierRouting">
		<rdfs:label>Carrier Routing</rdfs:label>
		<rdfs:comment>Describes shipping route, including instructions.</rdfs:comment>
	</owl:AnnotationProperty>
	<owl:AnnotationProperty rdf:ID="catalog">
		<rdfs:label>Catalog</rdfs:label>
		<rdfs:comment>Indicates the vendor catalog identifier assigned by SPS Commerce during vendor implementation.</rdfs:comment>
		<av7:userNotes>Assortment requires that this attribute have a value in order to validate.</av7:userNotes>
	</owl:AnnotationProperty>
	<owl:AnnotationProperty rdf:ID="cellularPhoneType">
		<rdfs:label>Cellular Phone Type</rdfs:label>
		<rdfs:comment>Describes a mobile phone's capabilities.</rdfs:comment>
	</owl:AnnotationProperty>
	<owl:DatatypeProperty rdf:ID="hasInedibleChemical">
		<rdfs:subPropertyOf rdf:resource="av7#chemical"/>
		<rdfs:label>Has Inedible Chemical</rdfs:label>
		<rdfs:comment>Indicates whether or not the represented item contains any chemical(s) not intended for human consumption.</rdfs:comment>
		<rdfs:range rdf:resource="xsd#boolean"/>
	</owl:DatatypeProperty>
	<owl:AnnotationProperty rdf:ID="chemicalsIncluded">
		<rdfs:subPropertyOf rdf:resource="av7#chemical"/>
		<rdfs:label>Chemicals Included</rdfs:label>
		<rdfs:comment>Lists chemicals contained in the represented item using the full, proper chemical names for each chemical compound.</rdfs:comment>
		<rdfs:range>
			<owl:equivalentClass>
				<owl:complementOf rdf:resource="xsd#boolean"/>
			</owl:equivalentClass>
		</rdfs:range>
	</owl:AnnotationProperty>
	<owl:AnnotationProperty rdf:ID="childCarSeatType">
		<rdfs:label>Child Car Seat Type</rdfs:label>
		<rdfs:comment>Indicates the kind of carseat (for babies and small children) being represented.</rdfs:comment>
	</owl:AnnotationProperty>
	<owl:DatatypeProperty rdf:ID="childrenUnderTwoLabelRequired">
		<rdfs:label>Children Under 2 Label Required</rdfs:label>
		<rdfs:comment>Indicates whether or not the represented item requires a children under 2 label.</rdfs:comment>
		<rdfs:range rdf:resource="xsd#boolean"/>
	</owl:DatatypeProperty>
	<owl:DatatypeProperty rdf:ID="childrenUnderFourLabelRequired">
		<rdfs:label>Children Under 4 Label Required</rdfs:label>
		<rdfs:comment>Indicates whether or not the represented item requires a children under 4 label.</rdfs:comment>
		<rdfs:range rdf:resource="xsd#boolean"/>
	</owl:DatatypeProperty>
	<owl:DatatypeProperty rdf:ID="cleanAirAct">
		<rdfs:label>Clean Air Act</rdfs:label>
		<rdfs:comment>Indicates whether or not the represented item is compliant with the Clean Air Act.</rdfs:comment>
		<sorg:relatedLink rdf:resource="https://www.epa.gov/compliance/resources-and-guidance-documents-compliance-assistance"/>
		<rdfs:range rdf:resource="xsd#boolean"/>
	</owl:DatatypeProperty>
	<owl:DatatypeProperty rdf:ID="cleanWaterAct">
		<rdfs:label>Clean Water Act</rdfs:label>
		<rdfs:comment>Indicates whether or not the represented item is compliant with the Clean Water Act.</rdfs:comment>
		<sorg:relatedLink rdf:resource="https://www.epa.gov/compliance/resources-and-guidance-documents-compliance-assistance"/>
		<rdfs:range rdf:resource="xsd#boolean"/>
	</owl:DatatypeProperty>
	<owl:AnnotationProperty rdf:ID="closureType">
		<rdfs:label>Closure Type</rdfs:label>
		<rdfs:comment>Indicates the type of closure used on the represented item.</rdfs:comment>
	</owl:AnnotationProperty>
	<owl:DatatypeProperty rdf:ID="clubLength">
		<rdfs:label>Club Length</rdfs:label>
		<rdfs:comment>Measures the length of the represented club.</rdfs:comment>
		<wmlo:userNotes>If this attribute obtains a value, 'Club Length UOM' must obtain a value.</wmlo:userNotes>
		<rdfs:range rdf:resource="xsd#float"/>
	</owl:DatatypeProperty>
	<owl:ObjectProperty rdf:ID="clubLengthUOM">
		<rdfs:label>Club Length UOM</rdfs:label>
		<rdfs:comment>Qualifies the value of 'Club Length.'</rdfs:comment>
		<wmlo:userNotes>If this attribute obtains a value, 'Club Length' must obtain a value.</wmlo:userNotes>
		<rdfs:range rdf:resource="av7#SpatialUOM"/>
	</owl:ObjectProperty>
	<owl:DatatypeProperty rdf:ID="coatLength">
		<rdfs:label>Coat Length</rdfs:label>
		<rdfs:comment>Measures the length of a coat.</rdfs:comment>
		<rdfs:range rdf:resource="xsd#float"/>
	</owl:DatatypeProperty>
	<owl:ObjectProperty rdf:ID="coatLengthUOM">
		<rdfs:label>Coat Length UOM</rdfs:label>
		<rdfs:comment>Qualifies the value of 'Coat Length.'</rdfs:comment>
		<rdfs:range rdf:resource="av7#SpatialUOM"/>
	</owl:ObjectProperty>
	<owl:DatatypeProperty rdf:ID="coaxialDigitalInputs">
		<rdfs:label>Coaxial Digital Inputs</rdfs:label>
		<rdfs:comment>Indicates the number of coaxial digital inputs onboard or supported by a represented item.</rdfs:comment>
		<rdfs:range rdf:resource="xsd#integer"/>
	</owl:DatatypeProperty>
	<owl:DatatypeProperty rdf:ID="coaxialDigitalOutputs">
		<rdfs:label>Coaxial Digital Outputs</rdfs:label>
		<rdfs:comment>Indicates the number of coaxial digital outputs onboard or supported by a represented item.</rdfs:comment>
		<rdfs:range rdf:resource="xsd#integer"/>
	</owl:DatatypeProperty>
	<owl:DatatypeProperty rdf:ID="coiled">
		<rdfs:label>Coiled</rdfs:label>
		<rdfs:comment>Indicates whether or not a represented item is coiled.</rdfs:comment>
		<rdfs:range rdf:resource="xsd#boolean"/>
	</owl:DatatypeProperty>
	<owl:AnnotationProperty rdf:ID="collarType">
		<rdfs:label>Collar Type</rdfs:label>
		<rdfs:comment>Indicates the collar type or style associated with the represented item.</rdfs:comment>
	</owl:AnnotationProperty>
	<owl:AnnotationProperty rdf:ID="colorFamily">
		<rdfs:label>Color Family</rdfs:label>
		<rdfs:comment>Denotes groups of similiarly toned colors.</rdfs:comment>
	</owl:AnnotationProperty>
	<owl:DatatypeProperty rdf:ID="colorTemperature">
		<rdfs:label>Color Temperature</rdfs:label>
		<rdfs:comment>The color tempreature of a represented item. Measured in Kelvin.</rdfs:comment>
		<rdfs:range rdf:resource="xsd#integer"/>
	</owl:DatatypeProperty>
	<owl:AnnotationProperty rdf:ID="compatibleDevices">
		<rdfs:label>Compatible Devices</rdfs:label>
		<rdfs:comment>Lists devices with which the represented item is compatible.</rdfs:comment>
	</owl:AnnotationProperty>
	<owl:DatatypeProperty rdf:ID="compliantWithLabelingRequirements">
		<rdfs:label>Compliant With Labeling Requirements</rdfs:label>
		<rdfs:comment>Indicates whether or not the represented item is compliant with all of labeling requirements which pertain to it.</rdfs:comment>
		<rdfs:range rdf:resource="xsd#boolean"/>
	</owl:DatatypeProperty>
	<owl:DatatypeProperty rdf:ID="componentVideoInputs">
		<rdfs:label>Component Video Inputs</rdfs:label>
		<rdfs:comment>Indicates the number of component video inputs onboard or supported by a represented item.</rdfs:comment>
		<rdfs:range rdf:resource="xsd#integer"/>
	</owl:DatatypeProperty>
	<owl:DatatypeProperty rdf:ID="componentVideoOutputs">
		<rdfs:label>Component Video Outputs</rdfs:label>
		<rdfs:comment>Indicates the number of component video outputs onboard or supported by a represented item.</rdfs:comment>
		<rdfs:range rdf:resource="xsd#integer"/>
	</owl:DatatypeProperty>
	<owl:ObjectProperty rdf:ID="compositeWoodCertificationCode">
		<rdfs:label>Composite Wood Certification Code</rdfs:label>
		<rdfs:comment>Indicates that a portion of the represented item contains any of the following types of composite wood: hardwood plywood veneer core, hardwood plywood composite core, particleboard, or medium density fiberboard (MDF).</rdfs:comment>
		<av7:userNotes>Enter the code corresponding to the highest formaldehyde emission level in any portion of the wood.</av7:userNotes>
		<rdfs:seeAlso rdf:resource="https://www.arb.ca.gov/toxics/compwood/implementation/faq.htm"/>
		<rdfs:range rdf:resource="av7#CompositeWoodCertificationCode"/>
	</owl:ObjectProperty>
	<owl:DatatypeProperty rdf:ID="comprehensiveEnvironmentalResponseCompensationAndLiabilityAct">
		<rdfs:label>Comprehensive Environmental Response Compensation And Liability Act</rdfs:label>
		<rdfs:comment>Indicates whether or not the represented item is compliant with the Comprehensive Environmental Response Compensation And Liability Act.</rdfs:comment>
		<sorg:relatedLink rdf:resource="https://www.epa.gov/compliance/resources-and-guidance-documents-compliance-assistance"/>
		<rdfs:range rdf:resource="xsd#boolean"/>
	</owl:DatatypeProperty>
	<owl:AnnotationProperty rdf:ID="compressionQuality">
		<rdfs:label>Resource</rdfs:label>
		<rdfs:comment>Indicates the compression quality associated with the represented digital asset.</rdfs:comment>
		<av7:userNotes>If this attribute obtains a value, 'Media Name' must also obtain a value.</av7:userNotes>
	</owl:AnnotationProperty>
	<owl:AnnotationProperty rdf:ID="compressorType">
		<rdfs:label>Compressor Type</rdfs:label>
		<rdfs:comment>Indicates the kind of compressor which is either onboard the represented item, which comprises the represented item, or which the represented item can accomodate.</rdfs:comment>
	</owl:AnnotationProperty>
	<owl:AnnotationProperty rdf:ID="condition">
		<rdfs:label>Condition</rdfs:label>
		<rdfs:comment>Indicates the condition or relative newness of the represented item.</rdfs:comment>
		<av7:userNotes>While there is no set associated with this attribute, we suggest the following values: new, like new, very good, good, acceptable, used, and refurbished.</av7:userNotes>
	</owl:AnnotationProperty>
	<owl:AnnotationProperty rdf:ID="constructionMethod">
		<rdfs:label>Construction Method</rdfs:label>
		<rdfs:comment>Described how a represented item is assembled or constructed.</rdfs:comment>
	</owl:AnnotationProperty>
	<owl:DatatypeProperty rdf:ID="consumerAvailableDate">
		<rdfs:label>Consumer Available Date</rdfs:label>
		<rdfs:comment>The date the item bring represented is available to the consumer for purchase.</rdfs:comment>
		<av7:userNotes>Format varies by upload and export method. UI and spreadsheet: mm/dd/yyyy; RSX: yyyy-mm-dd.</av7:userNotes>
		<rdfs:range rdf:resource="av7#VariableDate"/>
	</owl:DatatypeProperty>
	<owl:AnnotationProperty rdf:ID="consumerDescription">
		<rdfs:label>Consumer Description</rdfs:label>
		<rdfs:comment>A brief consumer-facing description of the represented item.</rdfs:comment>
	</owl:AnnotationProperty>
	<owl:DatatypeProperty rdf:ID="consumerItemDiameter">
		<rdfs:label>Consumer Item Diameter</rdfs:label>
		<rdfs:comment>Indicates the measure of a straight line from one sight of a circular item to the other side which passes through the center point (diameter) with reference to out-of-box assembled items.</rdfs:comment>
		<av7:userNotes>If this attribute obtains a value, 'Consumer Item Diameter UOM' must also obtain a value.</av7:userNotes>
		<rdfs:range rdf:resource="xsd#float"/>
	</owl:DatatypeProperty>
	<owl:ObjectProperty rdf:ID="consumerItemDiameterUOM">
		<rdfs:label>Consumer Item Diameter UOM</rdfs:label>
		<rdfs:comment>Qualifies the value of 'Consumer Item Diameter.'</rdfs:comment>
		<av7:userNotes>If this attribute obtains a value, 'Consumer Item Diameter' must also obtain a value.</av7:userNotes>
		<rdfs:range rdf:resource="wmlo#SpatialUOM"/>
	</owl:ObjectProperty>
	<owl:DatatypeProperty rdf:ID="consumerItemHeight">
		<rdfs:label>Consumer Item Height</rdfs:label>
		<rdfs:comment>Describes the height of a consumer item in real numbers.</rdfs:comment>
		<av7:userNotes>If this attribute obtains a value, 'Consumer Item Height UOM' must also obtain a value.</av7:userNotes>
		<rdfs:range rdf:resource="xsd#float"/>
	</owl:DatatypeProperty>
	<owl:ObjectProperty rdf:ID="consumerItemHeightUOM">
		<rdfs:label>Consumer Item Height UOM</rdfs:label>
		<rdfs:comment>Indicates the specific unit of measure which describes the value of 'Consumer Item Height.'</rdfs:comment>
		<av7:userNotes>If this attribute obtains a value, 'Consumer Item Height' must also obtain a value.</av7:userNotes>
		<rdfs:range rdf:resource="av7#SpatialUOM"/>
	</owl:ObjectProperty>
	<owl:DatatypeProperty rdf:ID="consumerItemLength">
		<rdfs:label>Consumer Item Length</rdfs:label>
		<rdfs:comment>Describes the length of a consumer item in real numbers.</rdfs:comment>
		<av7:userNotes>If this attribute obtains a value, 'Consumer Item Length UOM' must also obtain a value.</av7:userNotes>
		<rdfs:range rdf:resource="xsd#float"/>
	</owl:DatatypeProperty>
	<owl:ObjectProperty rdf:ID="consumerItemLengthUOM">
		<rdfs:label>Consumer Item Length UOM</rdfs:label>
		<rdfs:comment>Indicates the specific unit of measure which describes the value of 'Consumer Item Length.'</rdfs:comment>
		<av7:userNotes>If this attribute obtains a value, 'Consumer Item Length' must also obtain a value.</av7:userNotes>
		<rdfs:range rdf:resource="av7#SpatialUOM"/>
	</owl:ObjectProperty>
	<owl:DatatypeProperty rdf:ID="consumerItemWeight">
		<rdfs:label>Consumer Item Weight</rdfs:label>
		<rdfs:comment>Indicates the weight of an out-of-box, assembled item in real numbers.</rdfs:comment>
		<av7:userNotes>If this attribute obtains a value, 'Consumer Item Weight UOM' must also obtain a value.</av7:userNotes>
		<rdfs:range rdf:resource="xsd#float"/>
	</owl:DatatypeProperty>
	<owl:ObjectProperty rdf:ID="consumerItemWeightUOM">
		<rdfs:label>Consumer Item Weight UOM</rdfs:label>
		<rdfs:comment>Qualifies the value of 'Consumer Item Weight.'</rdfs:comment>
		<av7:userNotes>If this attribute obtains a value, 'Consumer Item Weight' must also obtain a value.</av7:userNotes>
		<rdfs:range rdf:resource="av7#PackWeightUOM"/>
	</owl:ObjectProperty>
	<owl:DatatypeProperty rdf:ID="consumerItemWidth">
		<rdfs:label>Consumer Item Width</rdfs:label>
		<rdfs:comment>Describes the width of a consumer item in real numbers.</rdfs:comment>
		<av7:userNotes>If this attribute obtains a value, 'Consumer Item Width UOM' must also obtain a value.</av7:userNotes>
		<rdfs:range rdf:resource="xsd#float"/>
	</owl:DatatypeProperty>
	<owl:ObjectProperty rdf:ID="consumerItemWidthUOM">
		<rdfs:label>Consumer Item Width UOM</rdfs:label>
		<rdfs:comment>Indicates the specific unit of measure which describes the value of 'Consumer Item Width.'</rdfs:comment>
		<av7:userNotes>If this attribute obtains a value, 'Consumer Item Width' must also obtain a value.</av7:userNotes>
		<rdfs:range rdf:resource="av7#SpatialUOM"/>
	</owl:ObjectProperty>
	<owl:DatatypeProperty rdf:ID="consumerPackageHeight">
		<rdfs:label>Consumer Package Height</rdfs:label>
		<rdfs:comment>Describes the height of a consumer package in real numbers.</rdfs:comment>
		<av7:userNotes>If this attribute obtains a value, 'Consumer Package Height UOM' must also obtain a value.</av7:userNotes>
		<rdfs:range rdf:resource="xsd#float"/>
	</owl:DatatypeProperty>
	<owl:ObjectProperty rdf:ID="consumerPackageHeightUOM">
		<rdfs:label>Consumer Package Height UOM</rdfs:label>
		<rdfs:comment>Indicates the specific unit of measure which describes the value of 'Consumer Package Height.'</rdfs:comment>
		<av7:userNotes>If this attribute obtains a value, 'Consumer Package Height' must also obtain a value.</av7:userNotes>
		<rdfs:range rdf:resource="av7#SpatialUOM"/>
	</owl:ObjectProperty>
	<owl:DatatypeProperty rdf:ID="consumerPackageLength">
		<rdfs:label>Consumer Package Length</rdfs:label>
		<rdfs:comment>Describes the length of a consumer package in real numbers.</rdfs:comment>
		<av7:userNotes>If this attribute obtains a value, 'Consumer Package Length UOM' must also obtain a value.</av7:userNotes>
		<rdfs:range rdf:resource="xsd#float"/>
	</owl:DatatypeProperty>
	<owl:ObjectProperty rdf:ID="consumerPackageLengthUOM">
		<rdfs:label>Consumer Package Length UOM</rdfs:label>
		<rdfs:comment>Indicates the specific unit of measure which describes the value of 'Consumer Package Length.'</rdfs:comment>
		<av7:userNotes>If this attribute obtains a value, 'Consumer Package Length' must also obtain a value.</av7:userNotes>
		<rdfs:range rdf:resource="av7#SpatialUOM"/>
	</owl:ObjectProperty>
	<owl:DatatypeProperty rdf:ID="consumerPackageSize">
		<rdfs:label>Consumer Package Size</rdfs:label>
		<rdfs:comment>Indicates the size of an order of consumer packages in real numbers.</rdfs:comment>
		<av7:userNotes>If this attribute obtains a value, 'Consumer Package Size UOM' must also obtain a value.</av7:userNotes>
		<rdfs:range rdf:resource="xsd#float"/>
	</owl:DatatypeProperty>
	<owl:ObjectProperty rdf:ID="consumerPackageSizeUOM">
		<rdfs:label>Consumer Package Size</rdfs:label>
		<rdfs:comment>Qualifies the value of 'Consumer Package Size' by descibing the kind of packaging or volumetric measure pertaining to it.</rdfs:comment>
		<av7:userNotes>If this attribute obtains a value, 'Consumer Package Size' must also obtain a value.</av7:userNotes>
		<rdfs:range rdf:resource="av7#PackType"/>
	</owl:ObjectProperty>
	<owl:DatatypeProperty rdf:ID="consumerPackageVolume">
		<rdfs:label>Consumer Package Volume (Cube)</rdfs:label>
		<rdfs:comment>Describes the volume of a consumer package in real numbers.</rdfs:comment>
		<av7:userNotes>If this attribute obtains a value, 'Consumer Package Volume (Cube) UOM' must also obtain a value.</av7:userNotes>
		<rdfs:range rdf:resource="xsd#float"/>
	</owl:DatatypeProperty>
	<owl:ObjectProperty rdf:ID="consumerPackageVolumeUOM">
		<rdfs:label>Consumer Package Volume (Cube) UOM</rdfs:label>
		<rdfs:comment>Indicates the specific unit of measure which describes the value of 'Consumer Package Volume (Cube).'</rdfs:comment>
		<av7:userNotes>If this attribute obtains a value, 'Consumer Package Volume (Cube)' must also obtain a value.</av7:userNotes>
		<rdfs:range rdf:resource="av7#PackVolumeUOM"/>
	</owl:ObjectProperty>
	<owl:DatatypeProperty rdf:ID="consumerPackageWidth">
		<rdfs:label>Consumer Package Width</rdfs:label>
		<rdfs:comment>Describes the width of a consumer package in real numbers.</rdfs:comment>
		<av7:userNotes>If this attribute obtains a value, 'Consumer Package Width UOM' must also obtain a value.</av7:userNotes>
		<rdfs:range rdf:resource="xsd#float"/>
	</owl:DatatypeProperty>
	<owl:ObjectProperty rdf:ID="consumerPackageWidthUOM">
		<rdfs:label>Consumer Package Width UOM</rdfs:label>
		<rdfs:comment>Indicates the specific unit of measure which describes the value of 'Consumer Package Width.'</rdfs:comment>
		<av7:userNotes>If this attribute obtains a value, 'Consumer Package Width' must also obtain a value.</av7:userNotes>
		<rdfs:range rdf:resource="av7#SpatialUOM"/>
	</owl:ObjectProperty>
	<owl:DatatypeProperty rdf:ID="consumerPackageWeight">
		<rdfs:label>Consumer Package Weight</rdfs:label>
		<rdfs:comment>Describes the weight of a consumer package in real numbers.</rdfs:comment>
		<av7:userNotes>If this attribute obtains a value, 'Consumer Package Weight UOM' must also obtain a value.</av7:userNotes>
		<rdfs:range rdf:resource="xsd#float"/>
	</owl:DatatypeProperty>
	<owl:ObjectProperty rdf:ID="consumerPackageWeightUOM">
		<rdfs:label>Consumer Package Weight UOM</rdfs:label>
		<rdfs:comment>Indicates the specific unit of measure which describes the value of 'Consumer Package Weight.'</rdfs:comment>
		<av7:userNotes>If this attribute obtains a value, 'Consumer Package Weight' must also obtain a value.</av7:userNotes>
		<rdfs:range rdf:resource="av7#PackWeightUOM"/>
	</owl:ObjectProperty>
	<owl:DatatypeProperty rdf:ID="consumerProductCapacityOrVolume">
		<rdfs:label>Resource</rdfs:label>
		<rdfs:comment>Describes the value of 'Consumer Product Capacity or Volume.'</rdfs:comment>
		<av7:userNotes>If this attribute obtains a value, 'Consumer Product Capacity or Volume' must also obtain a value.</av7:userNotes>
		<rdfs:range rdf:resource="av7#PackVolumeUOM"/>
	</owl:DatatypeProperty>
	<owl:DatatypeProperty rdf:ID="containsMercury">
		<rdfs:label>Contains Mercury</rdfs:label>
		<rdfs:comment>Indicates whether or not the represented item contains mercury.</rdfs:comment>
		<rdfs:range rdf:resource="xsd#boolean"/>
	</owl:DatatypeProperty>
	<owl:DatatypeProperty rdf:ID="containsPaperOrWood">
		<rdfs:subPropertyOf rdf:resource="av7#wood"/>
		<rdfs:label>Contains Paper Or Wood</rdfs:label>
		<rdfs:comment>Affirms or denies that the represented item contains paper or wood.</rdfs:comment>
		<rdfs:range rdf:resource="xsd#boolean"/>
	</owl:DatatypeProperty>
	<owl:DatatypeProperty rdf:ID="controlledSubstance">
		<rdfs:label>Controlled Substance</rdfs:label>
		<rdfs:comment>Indicates whether or not the represented item is a drug or chemical whose manufacture, possession, or use is regulated by a government.</rdfs:comment>
		<rdfs:range rdf:resource="xsd#boolean"/>
	</owl:DatatypeProperty>
	<owl:AnnotationProperty rdf:ID="countryOfOrigin">
		<rdfs:label>Country of Origin</rdfs:label>
		<rdfs:comment>Three digit country ISO code(s) which identify a represented item's primary manufacturing location as defined by ISO Country Codes-ISO 3166.</rdfs:comment>
		<sorg:relatedLink rdf:resource="http://www.iso.org/iso/home/standards/country_codes.htm"/>
	</owl:AnnotationProperty>
	<owl:AnnotationProperty rdf:ID="countryOfOriginAssembly">
		<rdfs:label>Country of Origin Assembly</rdfs:label>
		<rdfs:comment>Three digit country ISO code(s) which identify a represented item's primary assembly location (as distinct from and secondary to manufacturing location) as defined by ISO Country Codes-ISO 3166.</rdfs:comment>
		<sorg:relatedLink rdf:resource="http://www.iso.org/iso/home/standards/country_codes.htm"/>
	</owl:AnnotationProperty>
	<owl:AnnotationProperty rdf:ID="countryOfOriginComponents">
		<rdfs:label>
			<rdf:Bag>
				<rdf:li rdf:value="Country of Origin Components"/>
				<rdf:li rdf:value="Country of Origin Components 1"/>
				<rdf:li rdf:value="Country of Origin Components 2"/>
				<rdf:li rdf:value="Country of Origin Components 3"/>
				<rdf:li rdf:value="Country of Origin Components 4"/>
				<rdf:li rdf:value="Country of Origin Components 5"/>
				<rdf:li rdf:value="Country of Origin Components 6"/>
			</rdf:Bag>
		</rdfs:label>
		<rdfs:comment>Indicates the origin of the represented item's components.</rdfs:comment>
	</owl:AnnotationProperty>
	<owl:AnnotationProperty rdf:ID="countiesRestricted">
		<rdfs:label>Counties Restricted</rdfs:label>
		<rdfs:comment>Names the counties in which the represented item is restricted from sale.</rdfs:comment>
		<av7:userNotes>Users should input this value as a 2-letter abbreviation for the state in which the county lies plus the name of the county.</av7:userNotes>
	</owl:AnnotationProperty>
	<owl:AnnotationProperty rdf:ID="countriesRestricted">
		<rdfs:label>Countries Restricted</rdfs:label>
		<rdfs:comment>Names the countries in which the represented item is restricted from sale.</rdfs:comment>
		<av7:userNotes>Use ISO codes.</av7:userNotes>
	</owl:AnnotationProperty>
	<owl:AnnotationProperty rdf:ID="countryRestrictionReasons">
		<rdfs:label>Country Restriction Reasons</rdfs:label>
		<rdfs:comment>Indicates why an item is restricted from sale in a particular country.</rdfs:comment>
		<av7:userNotes>Users should input this value as a country ISO code followed by the specific reason for restriction.</av7:userNotes>
		<sorg:relatedLink rdf:resource="http://www.iso.org/iso/home/standards/country_codes.htm"/>
	</owl:AnnotationProperty>
	<owl:DatatypeProperty rdf:ID="countryRestrictions">
		<rdfs:label>Country Restrictions</rdfs:label>
		<rdfs:comment>Identifies whether or not the represented item is prohibited from sale in foreign countries.</rdfs:comment>
		<sorg:relatedLink rdf:resource="http://www.iso.org/iso/home/standards/country_codes.htm"/>
		<rdfs:range rdf:resource="xsd#boolean"/>
	</owl:DatatypeProperty>
	<owl:DatatypeProperty rdf:ID="countyRestrictions">
		<rdfs:subPropertyOf rdf:resource="av7#county"/>
		<rdfs:label>County Restrictions</rdfs:label>
		<rdfs:comment>Identifies whether or not the represented item is prohibited from sale in discrete counties in the USA.</rdfs:comment>
		<rdfs:range rdf:resource="xsd#boolean"/>
	</owl:DatatypeProperty>
	<owl:AnnotationProperty rdf:ID="countyRestrictionReasons">
		<rdfs:label>County Restriction Reasons</rdfs:label>
		<rdfs:comment>Describes why an item is restricted for sale in a municipality (neither a nation nor a US state).</rdfs:comment>
		<av7:userNotes>Users should input this value as a 2-letter abbreviation for the state in which the county lies, followed by the name of the county, followed by the specific reason for restriction.</av7:userNotes>
	</owl:AnnotationProperty>
	<owl:DatatypeProperty rdf:ID="cordless">
		<rdfs:label>Cordless</rdfs:label>
		<rdfs:comment>Indicates whether or not the represented item is cordless.</rdfs:comment>
		<rdfs:range rdf:resource="xsd#boolean"/>
	</owl:DatatypeProperty>
	<owl:DatatypeProperty rdf:ID="coverageArea">
		<rdfs:label>Coverage Area</rdfs:label>
		<rdfs:comment>Indicates the area that a represented item will cover.</rdfs:comment>
		<wmlo:userNotes>If this attribute obtains a value, 'Coverage Area UOM' must obtain a value.</wmlo:userNotes>
		<rdfs:range rdf:resource="xsd#float"/>
	</owl:DatatypeProperty>
	<owl:ObjectProperty rdf:ID="coverageAreaUOM">
		<rdfs:label>Coverage Area UOM</rdfs:label>
		<rdfs:comment>Qualifies the value of 'Coverage Area.'</rdfs:comment>
		<wmlo:userNotes>If this attribute obtains a value, 'Coverage Area' must obtain a value.</wmlo:userNotes>
		<rdfs:range rdf:resource="av7#CoverageAreaUOM"/>
	</owl:ObjectProperty>
	<owl:DatatypeProperty rdf:ID="cpsiaFlag">
		<rdfs:label>CPSIA Flag</rdfs:label>
		<rdfs:comment>Indicates whether or not hte represented item is compliant with the Consumer Product Safety Improvement Act.</rdfs:comment>
		<sorg:relatedLink rdf:resource="http://cpsc.gov"/>
		<rdfs:range rdf:resource="xsd#boolean"/>
	</owl:DatatypeProperty>
	<owl:DatatypeProperty rdf:ID="customizableCode">
		<rdfs:subPropertyOf rdf:resource="av7#customizability"/>
		<rdfs:label>Customizable Code</rdfs:label>
		<rdfs:comment>Indicates whether or not an item may be customized.</rdfs:comment>
		<rdfs:range rdf:resource="xsd#boolean"/>
	</owl:DatatypeProperty>
	<owl:AnnotationProperty rdf:ID="customizableDescription">
		<rdfs:subPropertyOf rdf:resource="av7#customizability"/>
		<rdfs:label>Customizable Description</rdfs:label>
		<rdfs:comment>A description of customization options; vendors should provide a list.</rdfs:comment>
		<rdfs:range>
			<owl:equivalentClass>
				<owl:complementOf rdf:resource="xsd#boolean"/>
			</owl:equivalentClass>
		</rdfs:range>
	</owl:AnnotationProperty>
	<owl:AnnotationProperty rdf:ID="designerCollection">
		<rdfs:label>Designer/Collection</rdfs:label>
		<rdfs:comment>Refers to clothing, accessories, or other items sold under a brand, label, or trademark associated with a designer, artist, or prominent person, or as part of a named collection.</rdfs:comment>
	</owl:AnnotationProperty>
	<owl:DatatypeProperty rdf:ID="digitalZoom">
		<rdfs:subPropertyOf rdf:resource="av7#magnification"/>
		<rdfs:label>Digital Zoom</rdfs:label>
		<rdfs:comment>Indicates whether or not a represented item uses computer-enhanced imaging as opposed to telescopic imaging only.</rdfs:comment>
		<rdfs:range rdf:resource="xsd#boolean"/>
	</owl:DatatypeProperty>
	<owl:DatatypeProperty rdf:ID="dimmable">
		<rdfs:label>Dimmable</rdfs:label>
		<rdfs:comment>Indicates whether or not the represented item is dimmable.</rdfs:comment>
		<rdfs:range rdf:resource="xsd#boolean"/>
	</owl:DatatypeProperty>
	<owl:ObjectProperty rdf:ID="directShip">
		<rdfs:label>Direct Ship</rdfs:label>
		<rdfs:comment>Indicates or describes phenomena related to direct shipping.</rdfs:comment>
	</owl:ObjectProperty>
	<owl:DatatypeProperty rdf:ID="hasDirectShip">
		<rdfs:subPropertyOf rdf:resource="av7#directShip"/>
		<rdfs:label>Has Direct Ship</rdfs:label>
		<rdfs:comment>Indicates whether or not the represented item may be direct-shipped.</rdfs:comment>
		<rdfs:range rdf:resource="xsd#boolean"/>
	</owl:DatatypeProperty>
	<owl:ObjectProperty rdf:ID="directShipCode">
		<rdfs:subPropertyOf rdf:resource="av7#directShip"/>
		<rdfs:label rdf:value="Direct Ship Code"/>
		<rdfs:comment rdf:value="Describes specific direct-ship capabilities."/>
		<av7:userNotes rdf:value="This attribute may be used with 'Drop Ship Description' or in place of it."/>
		<rdfs:range>
			<owl:equivalentClass>
				<owl:complementOf rdf:resource="xsd#boolean"/>
			</owl:equivalentClass>
		</rdfs:range>
	</owl:ObjectProperty>
	<owl:AnnotationProperty rdf:ID="directShipDescription">
		<rdfs:subPropertyOf rdf:resource="av7#directShip"/>
		<rdfs:label>Direct Ship Description</rdfs:label>
		<rdfs:comment>Describes specific direct-ship capabilities.</rdfs:comment>
	</owl:AnnotationProperty>
	<owl:DatatypeProperty rdf:ID="discontinueDate">
		<rdfs:label>Discontinue Date</rdfs:label>
		<rdfs:comment>The date the item bring represented is no longer available to the retailer for purchase.</rdfs:comment>
		<wmlo:userNotes>Format varies by upload and explort method. UI and spreadsheet: mm/dd/yyyy; RSX: yyyy-mm-dd.</wmlo:userNotes>
		<rdfs:range rdf:resource="av7#VariableDate"/>
	</owl:DatatypeProperty>
	<owl:AnnotationProperty rdf:ID="displayResolution">
		<rdfs:label>Display Resolution</rdfs:label>
		<rdfs:comment>Indicates the represented item's display resolution.</rdfs:comment>
		<wmlo:userNotes>The value of this attribute should be a real number plus a unit of measure.</wmlo:userNotes>
	</owl:AnnotationProperty>
	<owl:AnnotationProperty rdf:ID="displayScreenType">
		<rdfs:subPropertyOf rdf:resource="av7#screenDisplay"/>
		<rdfs:label>Display/Screen Type</rdfs:label>
		<rdfs:comment>Indicates the kind of screen or display onboard the represented item.</rdfs:comment>
		<rdfs:range>
			<owl:equivalentClass>
				<owl:complementOf rdf:resource="xsd#float"/>
			</owl:equivalentClass>
		</rdfs:range>
	</owl:AnnotationProperty>
	<owl:AnnotationProperty rdf:ID="doesNotContain">
		<rdfs:label>Does Not Contain</rdfs:label>
		<rdfs:comment>Lists ingredients or other factors that are not present in the represented item.</rdfs:comment>
		<av7:userNotes>The value(s) of this attribute often describe factors that are undesirable according to dietary or other health trends.</av7:userNotes>
	</owl:AnnotationProperty>
	<owl:ObjectProperty rdf:ID="door">
		<rdfs:label>Door</rdfs:label>
		<rdfs:comment>Indicates or describes phenomena having to do with doors.</rdfs:comment>
	</owl:ObjectProperty>
	<owl:DatatypeProperty rdf:ID="doorQuantity">
		<rdfs:subPropertyOf rdf:resource="av7#door"/>
		<rdfs:label>Door Quantity</rdfs:label>
		<rdfs:comment>Indicates a number or quantity of doors.</rdfs:comment>
		<rdfs:range rdf:resource="xsd#integer"/>
	</owl:DatatypeProperty>
	<owl:AnnotationProperty rdf:ID="doorType">
		<rdfs:subPropertyOf rdf:resource="av7#door"/>
		<rdfs:label>Door Type</rdfs:label>
		<rdfs:comment>Indicates a type or kind of door.</rdfs:comment>
		<rdfs:range>
			<owl:equivalentClass>
				<owl:complmentOf rdf:resource="xsd#integer"/>
			</owl:equivalentClass>
		</rdfs:range>
	</owl:AnnotationProperty>
	<owl:AnnotationProperty rdf:ID="dosageForm">
		<rdfs:label>Dosage Form</rdfs:label>
		<rdfs:comment>Indicates the shape, consistency, or other form that the represented item (i.e. a bottle) or its contents (i.e. tablets) take.</rdfs:comment>
		<av7:userNotes>When this attributes describes drugs, the value of this attribute may indicate how many tablets or milligrams are necessary to relieve pain or lower blood pressure.</av7:userNotes>
	</owl:AnnotationProperty>
	<owl:AnnotationProperty rdf:ID="drainPlacement">
		<rdfs:label>Drain Placement</rdfs:label>
		<rdfs:comment>Indicates where drains are placed in or on a represented item.</rdfs:comment>
	</owl:AnnotationProperty>
	<owl:AnnotationProperty rdf:ID="dressSkirtLengthCut">
		<rdfs:label>Dress/Skirt Cut</rdfs:label>
		<rdfs:comment>Describes the cut or shape of a dress or a skirt'.</rdfs:comment>
		<rdfs:range>
			<owl:equivalentClass>
				<owl:unionOf rdf:parseType="Collection">
					<owl:complementOf rdf:about="xsd#float"/>
					<owl:complementOf rdf:about="av7#SpatialUOM"/>
				</owl:unionOf>
			</owl:equivalentClass>
		</rdfs:range>
	</owl:AnnotationProperty>
	<owl:DatatypeProperty rdf:ID="dressSkirtLength">
		<rdfs:label>Dress/Skirt Length</rdfs:label>
		<rdfs:comment>Measures the length of the represented dress or skirt.</rdfs:comment>
		<av7:userNotes>If this attribute obtains a value, 'Dress/Skirt Length UOM' must also obtain a value.</av7:userNotes>
		<rdfs:range rdf:resource="xsd#float"/>
	</owl:DatatypeProperty>
	<owl:ObjectProperty rdf:ID="dressSkirtLengthUOM">
		<rdfs:label>Dress/Skirt Length UOM</rdfs:label>
		<rdfs:comment>Qualifies the value of 'Dress/Skirt Length'.</rdfs:comment>
		<av7:userNotes>If this attribute obtains a value, 'Dress/Skirt Length' must also obtain a value.</av7:userNotes>
		<rdfs:range rdf:resource="av7#SpatialUOM"/>
	</owl:ObjectProperty>
	<owl:ObjectProperty rdf:ID="dropShip">
		<rdfs:label>Drop Ship</rdfs:label>
		<rdfs:comment>Describes or indicates phenomena related to drop shipping.</rdfs:comment>
	</owl:ObjectProperty>
	<owl:DatatypeProperty rdf:ID="hasDropShip">
		<rdfs:subPropertyOf rdf:resource="av7#dropShip"/>
		<rdfs:label>Has Drop Ship</rdfs:label>
		<rdfs:comment>Indicates whether or not the represented item may be drop-shipped.</rdfs:comment>
		<rdfs:range rdf:resource="xsd#boolean"/>
	</owl:DatatypeProperty>
	<owl:AnnotationProperty rdf:ID="dropShipDescription">
		<rdfs:subPropertyOf rdf:resource="av7#dropShip"/>
		<rdfs:label>Drop Ship Description</rdfs:label>
		<rdfs:comment>Describes specific drop-ship capabilities.</rdfs:comment>
		<rdfs:range>
			<owl:equivalentClass>
				<owl:complementOf rdf:resource="xsd#boolean"/>
			</owl:equivalentClass>
		</rdfs:range>
	</owl:AnnotationProperty>
	<owl:DatatypeProperty rdf:ID="drugFactsLabelRequired">
		<rdfs:label>Drug Facts Label Required</rdfs:label>
		<rdfs:comment>Indicates whether or not the represented item requires a drug facts label.</rdfs:comment>
		<rdfs:range rdf:resource="xsd#boolean"/>
	</owl:DatatypeProperty>
	<owl:AnnotationProperty rdf:ID="durometer">
		<rdfs:label>Durometer</rdfs:label>
		<rdfs:comment>Measures the hardness of the represented item's material on the Durometer scale.</rdfs:comment>
		<sorg:relatedLink rdf:resource="https://en.wikipedia.org/wiki/Shore_durometer"/>
	</owl:AnnotationProperty>
	<owl:AnnotationProperty rdf:ID="dyeMethod">
		<rdfs:label>Dye Method</rdfs:label>
		<rdfs:comment>Indicates the method of dyeing used to color the represented item.</rdfs:comment>
	</owl:AnnotationProperty>
	<owl:ObjectProperty rdf:ID="ean">
		<rdfs:label>EAN</rdfs:label>
		<rdfs:comment>European Article Number a.k.a. GTIN 13. Maintained and defined by GS1.</rdfs:comment>
		<sorg:relatedLink rdf:resource="http://www.gs1.org/barcodes/ean-upc"/>
	</owl:ObjectProperty>
	<owl:DatatypeProperty rdf:ID="earringDrop">
		<rdfs:label>Earring Drop</rdfs:label>
		<rdfs:comment>Measures the length from the post to the bottom of a represented earring.</rdfs:comment>
		<wmlo:userNotes>If this attribute obtains a value, 'Earring Drop UOM' must obtain a value.</wmlo:userNotes>
		<rdfs:range rdf:resource="xsd#float"/>
	</owl:DatatypeProperty>
	<owl:ObjectProperty rdf:ID="earringDropUOM">
		<rdfs:label>Earring Drop UOM</rdfs:label>
		<rdfs:comment>Qualifies the value of 'Earring Drop.'</rdfs:comment>
		<wmlo:userNotes>If this attribute obtains a value, 'Earring Drop' must obtain a value.</wmlo:userNotes>
		<rdfs:range rdf:resource="av7#SpatialUOM"/>
	</owl:ObjectProperty>
	<owl:AnnotationProperty rdf:ID="edition">
		<rdfs:label>Edition</rdfs:label>
		<rdfs:comment>Identifies the edition of the represented publication.</rdfs:comment>
	</owl:AnnotationProperty>
	<owl:AnnotationProperty rdf:ID="electricalBoxPlacement">
		<rdfs:label>Electrical Box Placement</rdfs:label>
		<rdfs:comment>Indicates where electrical boxes should be installed with reference to the represented item; if the represented item is an electrical box, this attribute indicates where it should be installed.</rdfs:comment>
	</owl:AnnotationProperty>
	<owl:DatatypeProperty rdf:ID="energyGuideLabelRequired">
		<rdfs:label>Energy Guide Label Required</rdfs:label>
		<rdfs:comment>Indicates whether or not the represented item requires an energy guide label.</rdfs:comment>
		<rdfs:range rdf:resource="xsd#boolean"/>
	</owl:DatatypeProperty>
	<owl:DatatypeProperty rdf:ID="energyStarCompliant">
		<rdfs:label>Energy Star Compliant</rdfs:label>
		<rdfs:comment>Indicates whether or not the represented item is Energy Star compliant.</rdfs:comment>
		<sorg:relatedLink rdf:resource="https://www.energystar.gov/products/how-product-earns-energy-star-label"/>
		<rdfs:range rdf:resource="xsd#boolean"/>
	</owl:DatatypeProperty>
	<owl:ObjectProperty rdf:ID="esrbRating">
		<rdfs:label>ESRB Rating</rdfs:label>
		<rdfs:comment>Indicates how the Entertainment Software Rating Board rates a represented item.</rdfs:comment>
		<rdfs:range rdf:resource="av7#ESRBRating"/>
	</owl:ObjectProperty>
	<owl:AnnotationProperty rdf:ID="exitPupil">
		<rdfs:label>Exit Pupil</rdfs:label>
		<rdfs:comment>Describes the image size of the aperture stop which follows image capture in an optical device. In a telescope or compound microscope, this image is the image of the objective element(s) as produced by the eyepiece.</rdfs:comment>
		<wmlo:userNotes>Users should input the value of this attribute as a real number plus a unit of measure.</wmlo:userNotes>
	</owl:AnnotationProperty>
	<owl:DatatypeProperty rdf:ID="expirationDateMarked">
		<rdfs:label>Expiration Date Marked</rdfs:label>
		<rdfs:comment>Indicates whether or not an item has an expiration date.</rdfs:comment>
		<rdfs:range rdf:resource="xsd#boolean"/>
	</owl:DatatypeProperty>
	<owl:DatatypeProperty rdf:ID="eyeRelief">
		<rdfs:label>Eye Relief</rdfs:label>
		<rdfs:comment>Indicates how far away the human eye should be from a given lens in order for the magnification mechanism to function optimally.</rdfs:comment>
		<wmlo:userNotes>If this attribute obtains a value, 'Eye Relief UOM' must also obtain a value.</wmlo:userNotes>
		<rdfs:range rdf:resource="xsd#float"/>
	</owl:DatatypeProperty>
	<owl:ObjectProperty rdf:ID="eyeReliefUOM">
		<rdfs:label>Eye Relief UOM</rdfs:label>
		<rdfs:comment>Qualifies the value of 'Eye Relief'.</rdfs:comment>
		<wmlo:userNotes>If this attribute obtains a value, 'Eye Relief' must also obtain a value.</wmlo:userNotes>
		<rdfs:range rdf:resource="av7#SpatialUOM"/>
	</owl:ObjectProperty>
	<owl:AnnotationProperty rdf:ID="eyepieceOrientation">
		<rdfs:label>Eyepiece Orientation</rdfs:label>
		<rdfs:comment>Indicates the orientation of the eyepiece that is attached to a variety of optical devices.</rdfs:comment>
	</owl:AnnotationProperty>
	<owl:AnnotationProperty rdf:ID="faceAngle">
		<rdfs:label>Face Angle</rdfs:label>
		<rdfs:comment>Identifies the position of the represented club's face relative to the target line.</rdfs:comment>
	</owl:AnnotationProperty>
	<owl:DatatypeProperty rdf:ID="faceThickness">
		<rdfs:label>Face Thickness</rdfs:label>
		<rdfs:comment>Indicates the thickness of the face of the represented item.</rdfs:comment>
		<av7:userNotes>If this attribute obtains a value, 'Face Thickness UOM' must also obtain a value.</av7:userNotes>
		<rdfs:range rdf:resource="xsd#float"/>
	</owl:DatatypeProperty>
	<owl:ObjectProperty rdf:ID="faceThicknessUOM">
		<rdfs:label>Face Thickness UOM</rdfs:label>
		<rdfs:comment>Qualifies the value of 'Face Thickness'.</rdfs:comment>
		<av7:userNotes>If this attribute obtains a value, 'Face Thickness' must also obtain a value.</av7:userNotes>
		<rdfs:range rdf:resource="wmlo#SpatialUOM"/>
	</owl:ObjectProperty>
	<owl:DatatypeProperty rdf:ID="faceWeight">
		<rdfs:label>Face Weight</rdfs:label>
		<rdfs:comment>Indicates the weight of the fiber used to manufacture carpeting or rugs in ounces.</rdfs:comment>
		<av7:userNotes>The part of the rug or carpet described by this attribute is also known as its pile.</av7:userNotes>
		<rdfs:range rdf:resource="xsd#float"/>
	</owl:DatatypeProperty>
	<owl:DatatypeProperty rdf:ID="fairTrade">
		<rdfs:label>Fair Trade</rdfs:label>
		<rdfs:comment>Indicates whether or not the represented item is certified fair trade by a third party.</rdfs:comment>
		<rdfs:range rdf:resource="xsd#boolean"/>
	</owl:DatatypeProperty>
	<owl:DatatypeProperty rdf:ID="fastenerQualityAct">
		<rdfs:label>Fastener Quality Act</rdfs:label>
		<rdfs:comment>Indicates whether or not the represented item is subject to the Fastener Quality Act.</rdfs:comment>
		<sorg:relatedLink rdf:resource="http://www.indfast.org/info/fastener_quality_act.asp"/>
		<rdfs:range rdf:resource="xsd#boolean"/>
	</owl:DatatypeProperty>
	<owl:DatatypeProperty rdf:ID="fauxFur">
		<rdfs:label>Faux Fur</rdfs:label>
		<rdfs:comment>Indicates that the represented item is or has synthetic fur.</rdfs:comment>
		<rdfs:range rdf:resource="xsd#boolean"/>
	</owl:DatatypeProperty>
	<owl:AnnotationProperty rdf:ID="featuresBenefits">
		<rdfs:label>Features/Benefits</rdfs:label>
		<rdfs:comment>Describes features or benefits to the end consumer which are associated with the represented item.</rdfs:comment>
	</owl:AnnotationProperty>
	<owl:DatatypeProperty rdf:ID="fhaApproval">
		<rdfs:label>FHA Approval</rdfs:label>
		<rdfs:comment>Indicates whether or not the item owner has specifies that the represented item has Federal Housing Administration (FHA) approval.</rdfs:comment>
		<rdfs:range rdf:resource="xsd#boolean"/>
	</owl:DatatypeProperty>
	<owl:AnnotationProperty rdf:ID="fiberType">
		<rdfs:label>Fiber Type</rdfs:label>
		<rdfs:comment>Indicates the specific fiber type that comprises the represented item.</rdfs:comment>
	</owl:AnnotationProperty>
	<owl:DatatypeProperty rdf:ID="fieldOfViewAngular">
		<rdfs:label>Field of View (Angular)</rdfs:label>
		<rdfs:comment>Describes the maximal extent to which an item is able to represent its environment in degrees.</rdfs:comment>
		<wmlo:userNotes>Values may be between 0-360.</wmlo:userNotes>
		<rdfs:range rdf:resource="xsd#float"/>
	</owl:DatatypeProperty>
	<owl:DatatypeProperty rdf:ID="fieldOfViewAt100">
		<rdfs:label>Field of View at 100</rdfs:label>
		<rdfs:comment>Indicates field of view at 100 units of measure away from a target.</rdfs:comment>
		<wmlo:userNotes>If this attribute obtains a value, 'FIeld of View at 100 UOM' must also obtain a value.</wmlo:userNotes>
		<rdfs:range rdf:resource="xsd#float"/>
	</owl:DatatypeProperty>
	<owl:ObjectProperty rdf:ID="fieldOfViewAt100UOM">
		<rdfs:label>Field of View at 100 UOM</rdfs:label>
		<rdfs:comment>Qualifies the value of 'Field of View at 100'.</rdfs:comment>
		<wmlo:userNotes>If this attribute obtains a value, 'Field of View at 100' must also obtain a value.</wmlo:userNotes>
		<rdfs:range rdf:resource="av7#SpatialUOM"/>
	</owl:ObjectProperty>
	<owl:DatatypeProperty rdf:ID="fieldOfViewAt1000">
		<rdfs:label>Field of View at 1000</rdfs:label>
		<rdfs:comment>Indicates field of view at 1000 units of measure away from a target.</rdfs:comment>
		<wmlo:userNotes>If this attribute obtains a value, 'FIeld of View at 1000 UOM' must also obtain a value.</wmlo:userNotes>
		<rdfs:range rdf:resource="xsd#float"/>
	</owl:DatatypeProperty>
	<owl:ObjectProperty rdf:ID="fieldOfViewAt1000UOM">
		<rdfs:label>Field of View at 1000 UOM</rdfs:label>
		<rdfs:comment>Qualifies the value of 'Field of View at 1000'.</rdfs:comment>
		<wmlo:userNotes>If this attribute obtains a value, 'Field of View at 1000' must also obtain a value.</wmlo:userNotes>
		<rdfs:range rdf:resource="av7#SpatialUOM"/>
	</owl:ObjectProperty>
	<owl:DatatypeProperty rdf:ID="fireResistant">
		<rdfs:label>Fire Resistant</rdfs:label>
		<rdfs:comment>Indicates whether or not a represented item resists fire.</rdfs:comment>
		<rdfs:range rdf:resource="xsd#boolean"/>
	</owl:DatatypeProperty>
	<owl:DatatypeProperty rdf:ID="fittingInletThreadSize">
		<rdfs:label>Fitting Inlet Thread Size</rdfs:label>
		<rdfs:comment>Measures the inlet thread on a threaded fitting.</rdfs:comment>
		<wmlo:userNotes>If this attribute obtains a value, 'Fitting Inlet Thread Size UOM' must obtain a value.</wmlo:userNotes>
		<rdfs:range rdf:resource="xsd#float"/>
	</owl:DatatypeProperty>
	<owl:ObjectProperty rdf:ID="fittingInletThreadSizeUOM">
		<rdfs:label>Fitting Inlet Thread Size UOM</rdfs:label>
		<rdfs:comment>Qualifies the value of 'Fitting Inlet Thread Size.'</rdfs:comment>
		<wmlo:userNotes>If this attribute obtains a value, 'Fitting Inlet Thread Size' must obtain a value.</wmlo:userNotes>
		<rdfs:range rdf:resource="av7#SpatialUOM"/>
	</owl:ObjectProperty>
	<owl:DatatypeProperty rdf:ID="fittingOutletThreadSize">
		<rdfs:label>Fitting Outlet Thread Size</rdfs:label>
		<rdfs:comment>Measures the outlet thread on a threaded fitting.</rdfs:comment>
		<wmlo:userNotes>If this attribute obtains a value, 'Fitting Outlet Thread Size UOM' must obtain a value.</wmlo:userNotes>
		<rdfs:range rdf:resource="xsd#float"/>
	</owl:DatatypeProperty>
	<owl:ObjectProperty rdf:ID="fittingOutletThreadSizeUOM">
		<rdfs:label>Fitting Outlet Thread Size UOM</rdfs:label>
		<rdfs:comment>Qualifies the value of 'Fitting Outlet Thread Size.'</rdfs:comment>
		<wmlo:userNotes>If this attribute obtains a value, 'Fitting Outlet Thread Size' must obtain a value.</wmlo:userNotes>
		<rdfs:range rdf:resource="av7#SpatialUOM"/>
	</owl:ObjectProperty>
	<owl:DatatypeProperty rdf:ID="isFlammable">
		<rdfs:label>Flammable</rdfs:label>
		<rdfs:comment>Indicates whether or not the represented item is flammable or prone to catching fire.</rdfs:comment>
		<rdfs:range rdf:resource="xsd#boolean"/>
	</owl:DatatypeProperty>
	<owl:DatatypeProperty rdf:ID="flangeDiameter">
		<rdfs:label>Flange Diameter</rdfs:label>
		<rdfs:comment>Measures the diameter of the represented item's flange.</rdfs:comment>
		<wmlo:userNotes>If this attribute obtains a value, 'Flange Diameter UOM' must obtain a value.</wmlo:userNotes>
		<rdfs:range rdf:resource="xsd#float"/>
	</owl:DatatypeProperty>
	<owl:ObjectProperty rdf:ID="flangeDiameterUOM">
		<rdfs:label>Flange Diameter UOM</rdfs:label>
		<rdfs:comment>Qualifies the value of 'Flange Diameter.'</rdfs:comment>
		<wmlo:userNotes>If this attribute obtains a value, 'Flange Diameter' must obtain a value.</wmlo:userNotes>
		<rdfs:range rdf:resource="av7#SpatialUOM"/>
	</owl:ObjectProperty>
	<owl:DatatypeProperty rdf:ID="flashlight">
		<rdfs:label>Flashlight</rdfs:label>
		<rdfs:comment>Indicates whether or not a represented item is equipped with a light with which to illuminate objects of interest.</rdfs:comment>
		<rdfs:range rdf:resource="xsd#boolean"/>
	</owl:DatatypeProperty>
	<owl:ObjectProperty rdf:ID="flexibility">
		<rdfs:label>Flexibility</rdfs:label>
		<rdfs:comment>Describes the flexibility of an item.</rdfs:comment>
	</owl:ObjectProperty>
	<owl:AnnotationProperty rdf:ID="stickFlex">
		<rdfs:subPropertyOf rdf:resource="av7#flexibility"/>
		<rdfs:label>Stick Flex</rdfs:label>
		<rdfs:comment>Describes the flexibility of a stick.</rdfs:comment>
		<wmlo:userNotes>In hockey sticks and golf clubs, common 'flex' ratings include light, regular, stiff, extra stiff, and senior.</wmlo:userNotes>
		<rdfs:range>
			<owl:equivalentClass>
				<owl:complementOf rdf:resource="xsd#float"/>
			</owl:equivalentClass>
		</rdfs:range>
	</owl:AnnotationProperty>
	<owl:DatatypeProperty rdf:ID="flexNumber">
		<rdfs:subPropertyOf rdf:resource="av7#flexibility"/>
		<rdfs:label>Flex Number</rdfs:label>
		<rdfs:comment>Describes the flexibility of the represented item using a number.</rdfs:comment>
		<rdfs:range rdf:resource="xsd#float"/>
	</owl:DatatypeProperty>
	<owl:AnnotationProperty rdf:ID="focus">
		<rdfs:label>Focus</rdfs:label>
		<rdfs:comment>Indicates the kinds of focus programs or abilities available in a represented item.</rdfs:comment>
	</owl:AnnotationProperty>
	<owl:DatatypeProperty rdf:ID="fogproof">
		<rdfs:label>Fogproof</rdfs:label>
		<rdfs:comment>Indicates whether or not the represented item, often a lens, has been treated to resist fog.</rdfs:comment>
		<rdfs:range rdf:resource="xsd#boolean"/>
	</owl:DatatypeProperty>
	<owl:AnnotationProperty rdf:ID="foodForm">
		<rdfs:label>Food Form</rdfs:label>
		<rdfs:comment>Describes how a represented food item has been prepared for the consumer (i.e. sliced, whole, pureed).</rdfs:comment>
	</owl:AnnotationProperty>
	<owl:AnnotationProperty rdf:ID="footwearCleatType">
		<rdfs:label>Footwear Cleat Type</rdfs:label>
		<rdfs:comment>Indicates the type of cleats on a represented article of footwear.</rdfs:comment>
	</owl:AnnotationProperty>
	<owl:AnnotationProperty rdf:ID="footType">
		<rdfs:label>Foot Type</rdfs:label>
		<rdfs:comment>Indicates the type of foot which the represented item is intended to fit.</rdfs:comment>
	</owl:AnnotationProperty>
	<owl:AnnotationProperty rdf:ID="footwearWidth">
		<rdfs:label>Footwear Width</rdfs:label>
		<rdfs:comment>Indicates the width associated with a represented article of footwear.</rdfs:comment>
		<sorg:relatedLink rdf:resource="https://en.wikipedia.org/wiki/Shoe_size#Width"/>
	</owl:AnnotationProperty>
	<owl:AnnotationProperty rdf:ID="foundationGrade">
		<rdfs:label>Foundation Grade</rdfs:label>
		<rdfs:comment>Indicates the grade level at which the represented item may be used.</rdfs:comment>
	</owl:AnnotationProperty>
	<owl:AnnotationProperty rdf:ID="frameMaterial">
		<rdfs:label>Frame Material</rdfs:label>
		<rdfs:comment>Indicates the material that makes up the frame of the represented item.</rdfs:comment>
	</owl:AnnotationProperty>
	<owl:AnnotationProperty rdf:ID="frameRate">
		<rdfs:label>Frame Rate</rdfs:label>
		<rdfs:comment>The frequency with which frames of a moving image update. Used for televisions, film or any other affordance for displaying moving images.</rdfs:comment>
		<wmlo:userNotes>Users should input a real number plus a unit of measure.</wmlo:userNotes>
	</owl:AnnotationProperty>
	<owl:DatatypeProperty rdf:ID="frameWidth">
		<rdfs:label>Frame Width</rdfs:label>
		<rdfs:comment>Indicates width of a represented frame in millimeters.</rdfs:comment>
		<rdfs:range rdf:resource="xsd#float"/>
	</owl:DatatypeProperty>
	<owl:AnnotationProperty rdf:ID="freightClass">
		<rdfs:label>Freight Class</rdfs:label>
		<rdfs:comment>A code that describes an object's transportability according to a classification scheme defined by the National Motor Freight Association.</rdfs:comment>
		<sorg:relatedLink rdf:resource="http://www.nmfta.org/(X(1)S(ass2xer4dslbjhgfl4asnxff))/pages/nmfc?AspxAutoDetectCookieSupport=1"/>
	</owl:AnnotationProperty>
	<owl:DatatypeProperty rdf:ID="fuelContainerIncluded">
		<rdfs:label>Fuel Container Included</rdfs:label>
		<rdfs:comment>Indicates whether or not the represented item comes with a fuel container.</rdfs:comment>
		<rdfs:range rdf:resource="xsd#boolean"/>
	</owl:DatatypeProperty>
	<owl:AnnotationProperty rdf:ID="fuelType">
		<rdfs:label>Fuel Type</rdfs:label>
		<rdfs:comment>Indicates the type(s) of fuel which the represented item will accept.</rdfs:comment>
	</owl:AnnotationProperty>
	<owl:AnnotationProperty rdf:ID="furAnimalName">
		<rdfs:label>Fur Animal Name</rdfs:label>
		<rdfs:comment>Indicates the type of natural animal fur used in the represented item.'</rdfs:comment>
		<wmlo:userNotes>If faux or synthetic fur, use the attribute 'Fiber Type.</wmlo:userNotes>
	</owl:AnnotationProperty>
	<owl:ObjectProperty rdf:ID="furCountryOfOrigin">
		<rdfs:label>Fur Country of Origin</rdfs:label>
		<rdfs:comment>Indicates the country of origin for a represented fur item.'</rdfs:comment>
	</owl:ObjectProperty>
	<owl:AnnotationProperty rdf:ID="furTreatment">
		<rdfs:label>Fur Treatment</rdfs:label>
		<rdfs:comment>Indicates the kind of treatment applied to a represented fur item.'</rdfs:comment>
	</owl:AnnotationProperty>
	<owl:DatatypeProperty rdf:ID="futureQtyByLocation">
		<rdfs:label>Future Quantity By Location</rdfs:label>
		<rdfs:comment>Indicates the total quantity of represented items available to order by location.</rdfs:comment>
		<rdfs:range rdf:resource="xsd#integer"/>
	</owl:DatatypeProperty>
	<owl:DatatypeProperty rdf:ID="futureQtyByLocationDate">
		<rdfs:label>Future Quantity By Location Date</rdfs:label>
		<rdfs:comment>The date on which additional quantities of represented items will be available to order from a specific location.</rdfs:comment>
		<av7:userNotes>Format varies by upload and explort method. UI and spreadsheet: mm/dd/yyyy; RSX: yyyy-mm-dd.</av7:userNotes>
		<rdfs:range rdf:resoure="av7#VariableDate"/>
	</owl:DatatypeProperty>
	<owl:DatatypeProperty rdf:ID="futureQtyTotalDate">
		<rdfs:label>Future Quantity Total Date</rdfs:label>
		<rdfs:comment>Indicates the date on which additional quantities of the represented item will be available for order.</rdfs:comment>
		<av7:userNotes>Format varies by upload and explort method. UI and spreadsheet: mm/dd/yyyy; RSX: yyyy-mm-dd.</av7:userNotes>
		<rdfs:range rdf:resource="av7#VariableDate"/>
	</owl:DatatypeProperty>
	<owl:DatatypeProperty rdf:ID="futureQtyTotal">
		<rdfs:label>Future Quantity Total</rdfs:label>
		<rdfs:comment>Indicates the total future quantity available to order.</rdfs:comment>
		<rdfs:range rdf:resource="xsd#integer"/>
	</owl:DatatypeProperty>
	<owl:DatatypeProperty rdf:ID="gangboxQuantity">
		<rdfs:label>Gangbox Quantity</rdfs:label>
		<rdfs:comment>Indicates the number of electrical components which the represented item can accomodate.</rdfs:comment>
		<sorg:relatedLink rdf:resource="https://en.wikipedia.org/wiki/Gang_box"/>
		<rdfs:range rdf:resource="xsd#integer"/>
	</owl:DatatypeProperty>
	<owl:DatatypeProperty rdf:ID="gauge">
		<rdfs:label>Gauge</rdfs:label>
		<rdfs:comment>Indicates the thickness, size, or capacity of the represented item.</rdfs:comment>
		<av7:userNotes>If this attribute obtains a value, 'Gauge UOM' must also obtain a value.</av7:userNotes>
		<rdfs:range rdf:resource="xsd#float"/>
	</owl:DatatypeProperty>
	<owl:ObjectProperty rdf:ID="gaugeUOM">
		<rdfs:label>Gauge UOM</rdfs:label>
		<rdfs:comment>Qualifies the value of 'Gauge'.</rdfs:comment>
		<av7:userNotes>If this attribute obtains a value, 'Gauge' must also obtain a value.</av7:userNotes>
		<rdfs:range rdf:resource="av7#SpatialUOM"/>
	</owl:ObjectProperty>
	<owl:DatatypeProperty rdf:ID="gearRatio">
		<rdfs:label>Gear Ratio</rdfs:label>
		<rdfs:comment>Indicates the number of rotations wanted for the driven gear to rotate with the driver gear.</rdfs:comment>
		<rdfs:range rdf:resource="xsd#float"/>
	</owl:DatatypeProperty>
	<owl:AnnotationProperty rdf:ID="gender">
		<rdfs:label>Gender</rdfs:label>
		<rdfs:comment>Indicates the age-inclusive gender and age range for which item is designed.</rdfs:comment>
		<av7:userNotes>While there is no set associated with this attribute, we recommend the following values: baby, girl, boy, man, woman,unisex.</av7:userNotes>
	</owl:AnnotationProperty>
	<owl:AnnotationProperty rdf:ID="genre">
		<rdfs:label>Genre</rdfs:label>
		<rdfs:comment>Lists the generic type of music, film, writing, or other forms of art or entertianment which pertian to the represented item.</rdfs:comment>
	</owl:AnnotationProperty>
	<owl:DatatypeProperty rdf:ID="gmoFree">
		<rdfs:label>GMO Free</rdfs:label>
		<rdfs:comment>Indicates whether or not the represented item contains genetically modified organisms .</rdfs:comment>
		<rdfs:range rdf:resource="xsd#boolean"/>
	</owl:DatatypeProperty>
	<owl:DatatypeProperty rdf:ID="goldKarat">
		<rdfs:label>Gold Karat</rdfs:label>
		<rdfs:comment>Indicates the karat weight of a represented gold article.</rdfs:comment>
		<rdfs:range rdf:resource="xsd#float"/>
	</owl:DatatypeProperty>
	<owl:AnnotationProperty rdf:ID="grade">
		<rdfs:label>Grade</rdfs:label>
		<rdfs:comment>Describes the quality or grade of an item.</rdfs:comment>
	</owl:AnnotationProperty>
	<owl:AnnotationProperty rdf:ID="gripType">
		<rdfs:label>Grip Type</rdfs:label>
		<rdfs:comment>Describes the grip on the represented item.</rdfs:comment>
		<wmlo:userNotes>While there is no restricted list of values for this attribute, common grip types include corded, rubber, paddle, and pistol.</wmlo:userNotes>
	</owl:AnnotationProperty>
	<owl:DatatypeProperty rdf:ID="groutRecommendation">
		<rdfs:label>Grout Recommendation</rdfs:label>
		<rdfs:comment>Recommends grout size according to the installation guidelines of th erepresented item.</rdfs:comment>
		<wmlo:userNotes>If this attribute obtains a value, 'Grout Recommendation UOM' must obtain a value.</wmlo:userNotes>
		<rdfs:range rdf:resource="xsd#float"/>
	</owl:DatatypeProperty>
	<owl:ObjectProperty rdf:ID="groutRecommendationUOM">
		<rdfs:label>Grout Recommendation UOM</rdfs:label>
		<rdfs:comment>Qualifies the value of 'Grout Recommendation.'</rdfs:comment>
		<wmlo:userNotes>If this attribute obtains a value, 'Grout Recommendation' must obtain a value.</wmlo:userNotes>
		<rdfs:range rdf:resource="av7#SpatialUOM"/>
	</owl:ObjectProperty>
	<owl:AnnotationProperty rdf:ID="gtin">
		<rdfs:label>GTIN</rdfs:label>
		<rdfs:comment>Global Trade Identification Number a.k.a. GTIN 14. Maintained and defined by GS1.</rdfs:comment>
		<sorg:relatedLink rdf:resource="http://www.gs1.org/gtin"/>
	</owl:AnnotationProperty>
	<owl:DatatypeProperty rdf:ID="handbagShoulderDrop">
		<rdfs:label>Handbag Shoulder Drop</rdfs:label>
		<rdfs:comment>Measures the strap or handle from the top of the represented handbag to the peak of the strap or handle as it lies on the hand or shoulder.</rdfs:comment>
		<wmlo:userNotes>If this attribute obtains a value, 'Handbag Shoulder Drop UOM' must obtain a value.</wmlo:userNotes>
		<rdfs:range rdf:resource="xsd#float"/>
	</owl:DatatypeProperty>
	<owl:ObjectProperty rdf:ID="handbagShoulderDropUOM">
		<rdfs:label>Handbag Shoulder Drop UOM</rdfs:label>
		<rdfs:comment>Qualifies the value of 'Handbag Shoulder Drop.'</rdfs:comment>
		<wmlo:userNotes>If this attribute obtains a value, 'Handbag Shoulder Drop' must obtain a value.</wmlo:userNotes>
		<rdfs:range rdf:resource="av7#SpatialUOM"/>
	</owl:ObjectProperty>
	<owl:AnnotationProperty rdf:ID="handleType">
		<rdfs:subPropertyOf rdf:resource="av7#handle"/>
		<rdfs:label>Handle Type</rdfs:label>
		<rdfs:comment>Describes the kind of handle on the represented item.</rdfs:comment>
		<rdfs:range>
			<owl:equivalentClass>
				<owl:complementOf rdf:resource="xsd#integer"/>
			</owl:equivalentClass>
		</rdfs:range>
	</owl:AnnotationProperty>
	<owl:DatatypeProperty rdf:ID="numberOfHandles">
		<rdfs:subPropertyOf rdf:resource="av7#handle"/>
		<rdfs:label>Number of Handles</rdfs:label>
		<rdfs:comment>Describes the kind of handle on the represented item.</rdfs:comment>
		<rdfs:range rdf:resource="xsd#integer"/>
	</owl:DatatypeProperty>
	<owl:AnnotationProperty rdf:ID="hangerType">
		<rdfs:label>Hanger Type</rdfs:label>
		<rdfs:comment>Describes shipping or display hangers associated with the represented item.</rdfs:comment>
	</owl:AnnotationProperty>
	<owl:AnnotationProperty rdf:ID="harmonizedTariffCode">
		<rdfs:label>Resource</rdfs:label>
		<rdfs:comment>Identifies the classification code established by the US government for imported goods.</rdfs:comment>
		<sorg:relatedLink rdf:resource="http://hts.usitc.gov"/>
	</owl:AnnotationProperty>
	<owl:AnnotationProperty rdf:ID="hazardousMaterialClassCode">
		<rdfs:label>Hazardous Material Class Code</rdfs:label>
		<rdfs:comment>Identifies the hazardous material class according to a standard determined by the USA Department of Transportation.</rdfs:comment>
		<sorg:relatedLink rdf:resource="https://www.fmsca.dot.gov/regulations/hazardous-materials/how-comply-federal-hazardous-materials-regulations"/>
	</owl:AnnotationProperty>
	<owl:AnnotationProperty rdf:ID="hazardousMaterialDescription">
		<rdfs:label>Hazardous Material Class Code</rdfs:label>
		<rdfs:comment>Describes the value of 'Hazardous Material Class Code'.</rdfs:comment>
	</owl:AnnotationProperty>
	<owl:ObjectProperty rdf:ID="hazardousMaterialQualifier">
		<rdfs:label>Hazardous Material Qualifier</rdfs:label>
		<rdfs:comment>Affirms the presence of hazardous materials intrinsic to the item being described.</rdfs:comment>
		<rdfs:range rdf:resource="av7#HazardousMaterialQualifier"/>
	</owl:ObjectProperty>
	<owl:DatatypeProperty rdf:ID="hdmiInputs">
		<rdfs:label>HDMI Inputs</rdfs:label>
		<rdfs:comment>Indicates the number of HDMI inputs onboard or supported by a represented item.</rdfs:comment>
		<rdfs:range rdf:resource="xsd#integer"/>
	</owl:DatatypeProperty>
	<owl:DatatypeProperty rdf:ID="hdmiOutputs">
		<rdfs:label>HDMI Outputs</rdfs:label>
		<rdfs:comment>Indicates the number of HDMI outputs onboard or supported by a represented item.</rdfs:comment>
		<rdfs:range rdf:resource="xsd#integer"/>
	</owl:DatatypeProperty>
	<owl:ObjectProperty rdf:ID="clubHead">
		<rdfs:label>Club Head</rdfs:label>
		<rdfs:comment>Describes or indicates phenomena realted to heads of clubs.</rdfs:comment>
	</owl:ObjectProperty>
	<owl:DatatypeProperty rdf:ID="headVolume">
		<rdfs:subPropertyOf rdf:resource="av7#clubHead"/>
		<rdfs:label>Head Volume</rdfs:label>
		<rdfs:comment>Measures the size of a wood head (using liquid displacement) in cubic centimeters.</rdfs:comment>
		<rdfs:range rdf:resource="xsd#float"/>
	</owl:DatatypeProperty>
	<owl:AnnotationProperty rdf:ID="putterHeadStyle">
		<rdfs:subPropertyOf rdf:resource="av7#clubHead"/>
		<rdfs:label>Putter Head Style</rdfs:label>
		<rdfs:comment>Measures the size of a wood head (using liquid displacement) in cubic centimeters.</rdfs:comment>
		<rdfs:range>
			<owl:equivalentClass>
				<owl:complementOf rdf:resource="xsd#float"/>
			</owl:equivalentClass>
		</rdfs:range>
	</owl:AnnotationProperty>
	<owl:DatatypeProperty rdf:ID="heatMoldable">
		<rdfs:label>Heat Moldable</rdfs:label>
		<rdfs:comment>Indicates whether or not a represented item is heat moldable.</rdfs:comment>
		<rdfs:range rdf:resource="xsd#boolean"/>
	</owl:DatatypeProperty>
	<owl:AnnotationProperty rdf:ID="heatingElementType">
		<rdfs:label>Heating Element Type</rdfs:label>
		<rdfs:comment>Indicates the kind of heating element which is either onboard the represented item, which comprises the represented item, or which the represented item can accomodate.</rdfs:comment>
	</owl:AnnotationProperty>
	<owl:AnnotationProperty rdf:ID="heatSystem">
		<rdfs:label>Heat System</rdfs:label>
		<rdfs:comment>Indicates the heat system that comprises the represented item or which the represented item accomodates.</rdfs:comment>
	</owl:AnnotationProperty>
	<owl:DatatypeProperty rdf:ID="heelHeight">
		<rdfs:label>Heel Height</rdfs:label>
		<rdfs:comment>Indicates the height of a heel on a represented article of footwear.</rdfs:comment>
		<wmlo:userNotes>If this attribute obtains a value, 'Heel Height/Platform Sole Height UOM' must obtain a value.</wmlo:userNotes>
		<rdfs:range rdf:resource="xsd#float"/>
	</owl:DatatypeProperty>
	<owl:ObjectProperty rdf:ID="heelHeightPlatformSoleHeightUOM">
		<rdfs:label>Heel Height/Platform Sole Height UOM</rdfs:label>
		<rdfs:comment>Qualifies the values of 'Heel Height' and 'Platform Sole Height'.</rdfs:comment>
		<wmlo:userNotes>If this attribute obtains a value, either 'Heel Height,' 'Platform Sole Height,' or both must obtain values.</wmlo:userNotes>
		<rdfs:range rdf:resource="av7#SpatialUOM"/>
	</owl:ObjectProperty>
	<owl:DatatypeProperty rdf:ID="highEfficiency">
		<rdfs:label>High Efficiency</rdfs:label>
		<rdfs:comment>Indicates whether or not the respresented item is labled as 'high efficiency' by its manufacturer or vendor.</rdfs:comment>
		<rdfs:range rdf:resource="xsd#boolean"/>
	</owl:DatatypeProperty>
	<owl:AnnotationProperty rdf:ID="handedness">
		<rdfs:label>Hand</rdfs:label>
		<rdfs:comment>Indicates which hand (right or left) the represented item is fit for.</rdfs:comment>
	</owl:AnnotationProperty>
	<owl:DatatypeProperty rdf:ID="hypoallergenic">
		<rdfs:label>Hypo-Allergenic</rdfs:label>
		<rdfs:comment>Indicates whether or not the represented item is hypoallergenic.</rdfs:comment>
		<rdfs:range rdf:resource="xsd#boolean"/>
	</owl:DatatypeProperty>
	<owl:DatatypeProperty rdf:ID="inclinometer">
		<rdfs:label>Inclinometer</rdfs:label>
		<rdfs:comment>Indicates that the represented item includes an inclinometer or clinometer (an instrument for measuring angles of elevation).</rdfs:comment>
		<rdfs:range rdf:resource="xsd#boolean"/>
	</owl:DatatypeProperty>
	<owl:AnnotationProperty rdf:ID="ignitionType">
		<rdfs:label>Ignition Type</rdfs:label>
		<rdfs:comment>Indicates the type of ignition system on or compatible with a represented item.</rdfs:comment>
	</owl:AnnotationProperty>
	<owl:DatatypeProperty rdf:ID="hasInfrared">
		<rdfs:label>Infrared</rdfs:label>
		<rdfs:comment>Indicates whether or not the represented item has infrared or heat-detecting capabilities).</rdfs:comment>
		<rdfs:range rdf:resource="xsd#boolean"/>
	</owl:DatatypeProperty>
	<owl:DatatypeProperty rdf:ID="innerDiameter">
		<rdfs:label>Inner Diameter</rdfs:label>
		<rdfs:comment>Indicates the measure of an object's inner diameter; of particular use for tubular objects.</rdfs:comment>
		<wmlo:userNotes>If this attribute obtains a value, 'Inner Diameter UOM' must obtain a value.</wmlo:userNotes>
		<rdfs:range rdf:resource="xsd#float"/>
	</owl:DatatypeProperty>
	<owl:ObjectProperty rdf:ID="innerDiameterUOM">
		<rdfs:label>Inner Diameter UOM</rdfs:label>
		<rdfs:comment>Indicates units of measure which describe the value of 'Inner Diameter.'</rdfs:comment>
		<wmlo:userNotes>If this attribute obtains a value, 'Inner Diameter' must obtain a value.</wmlo:userNotes>
		<rdfs:range rdf:resource="wmlo#SpatialUOM"/>
	</owl:ObjectProperty>
	<owl:AnnotationProperty rdf:ID="innerPackGTIN">
		<rdfs:label>Inner Pack GTIN</rdfs:label>
		<rdfs:comment>The GTIN which identifies a unique inner pack or case contained by a master pack.</rdfs:comment>
	</owl:AnnotationProperty>
	<owl:DatatypeProperty rdf:ID="innerPackHeight">
		<rdfs:label>Inner Pack Height</rdfs:label>
		<rdfs:comment>Describes the length of an inner pack in real numbers.</rdfs:comment>
		<av7:userNotes>If this attribute obtains a value, 'Inner Pack Height UOM' must also obtain a value.</av7:userNotes>
		<rdfs:range rdf:resource="xsd#float"/>
	</owl:DatatypeProperty>
	<owl:ObjectProperty rdf:ID="innerPackHeightUOM">
		<rdfs:label>Inner Pack Height UOM</rdfs:label>
		<rdfs:comment>Indicates the specific unit of measure which describes the value of 'Inner Pack Height.'</rdfs:comment>
		<av7:userNotes>If this attribute obtains a value, 'Inner Pack Height' must also obtain a value.</av7:userNotes>
		<rdfs:range rdf:resource="av7#SpatialUOM"/>
	</owl:ObjectProperty>
	<owl:DatatypeProperty rdf:ID="innerPackLength">
		<rdfs:label>Inner Pack Length</rdfs:label>
		<rdfs:comment>Describes the length of an inner pack in real numbers.</rdfs:comment>
		<av7:userNotes>If this attribute obtains a value, 'Inner Pack Length UOM' must also obtain a value.</av7:userNotes>
		<rdfs:range rdf:resource="xsd#float"/>
	</owl:DatatypeProperty>
	<owl:ObjectProperty rdf:ID="innerPackLengthUOM">
		<rdfs:label>Inner Pack Length UOM</rdfs:label>
		<rdfs:comment>Indicates the specific unit of measure which describes the value of 'Inner Pack Length.'</rdfs:comment>
		<av7:userNotes>If this attribute obtains a value, 'Inner Pack Length' must also obtain a value.</av7:userNotes>
		<rdfs:range rdf:resource="av7#SpatialUOM"/>
	</owl:ObjectProperty>
	<owl:DatatypeProperty rdf:ID="innerPackVolume">
		<rdfs:label>Inner Pack Volume</rdfs:label>
		<rdfs:comment>Describes the volume of an inner pack in real numbers.</rdfs:comment>
		<av7:userNotes>If this attribute obtains a value, 'Inner Pack Volume UOM' must also obtain a value.</av7:userNotes>
		<rdfs:range rdf:resource="xsd#float"/>
	</owl:DatatypeProperty>
	<owl:ObjectProperty rdf:ID="innerPackVolumeUOM">
		<rdfs:label>Inner Pack Volume UOM</rdfs:label>
		<rdfs:comment>Indicates the specific unit of measure which describes the value of 'Inner Pack Volume.'</rdfs:comment>
		<av7:userNotes>If this attribute obtains a value, 'Inner Pack Volume' must also obtain a value.</av7:userNotes>
		<rdfs:range rdf:resource="av7#PackVolumeUOM"/>
	</owl:ObjectProperty>
	<owl:DatatypeProperty rdf:ID="innerPackWeight">
		<rdfs:label>Inner Pack Weight</rdfs:label>
		<rdfs:comment>Describes the weight of an inner pack in real numbers.</rdfs:comment>
		<av7:userNotes>If this attribute obtains a value, 'Inner Pack Weight UOM' must also obtain a value.</av7:userNotes>
		<rdfs:range rdf:resource="xsd#float"/>
	</owl:DatatypeProperty>
	<owl:ObjectProperty rdf:ID="innerPackWeightUOM">
		<rdfs:label>Inner Pack Weight UOM</rdfs:label>
		<rdfs:comment>Indicates the specific unit of measure which describes the value of 'Inner Pack Weight.'</rdfs:comment>
		<av7:userNotes>If this attribute obtains a value, 'Inner Pack Weight' must also obtain a value.</av7:userNotes>
		<rdfs:range rdf:resource="av7#PackWeightUOM"/>
	</owl:ObjectProperty>
	<owl:DatatypeProperty rdf:ID="innerPackWidth">
		<rdfs:label>Inner Pack Width</rdfs:label>
		<rdfs:comment>Describes the width of an inner pack in real numbers.</rdfs:comment>
		<av7:userNotes>If this attribute obtains a value, 'Inner Pack Width UOM' must also obtain a value.</av7:userNotes>
		<rdfs:range rdf:resource="xsd#float"/>
	</owl:DatatypeProperty>
	<owl:ObjectProperty rdf:ID="innerPackWidthUOM">
		<rdfs:label>Inner Pack Width UOM</rdfs:label>
		<rdfs:comment>Indicates the specific unit of measure which describes the value of 'Inner Pack Width.'</rdfs:comment>
		<av7:userNotes>If this attribute obtains a value, 'Inner Pack Width' must also obtain a value.</av7:userNotes>
		<rdfs:range rdf:resource="av7#SpatialUOM"/>
	</owl:ObjectProperty>
	<owl:DatatypeProperty rdf:ID="innerPackQty">
		<rdfs:label>Inner Pack Quantity</rdfs:label>
		<rdfs:comment>Indicates the total number of saleable units as contained by an outer pack.</rdfs:comment>
		<rdfs:range rdf:resource="xsd#integer"/>
	</owl:DatatypeProperty>
	<owl:ObjectProperty rdf:ID="insulation">
		<rdfs:label>Insulation</rdfs:label>
		<rdfs:comment>Indicates or describes phenomena related to insulation.</rdfs:comment>
	</owl:ObjectProperty>
	<owl:DatatypeProperty rdf:ID="insulated">
		<rdfs:subPropertyOf rdf:resource="av7#insulation"/>
		<rdfs:label>Insulated</rdfs:label>
		<rdfs:comment>Indicates whether or not the respresented item is insulated.</rdfs:comment>
		<rdfs:range rdf:resource="xsd#boolean"/>
	</owl:DatatypeProperty>
	<owl:AnnotationProperty rdf:ID="insulationRValue">
		<rdfs:subPropertyOf rdf:resource="av7#insulation"/>
		<rdfs:label>Insulation R Value</rdfs:label>
		<rdfs:comment>The specific R-value pertaining to a represented item.</rdfs:comment>
		<sorg:relatedLink rdf:resource="http://energy.gov/energysaver/insulation"/>
	</owl:AnnotationProperty>
	<owl:AnnotationProperty rdf:ID="insulationType">
		<rdfs:subPropertyOf rdf:resource="av7#insulation"/>
		<rdfs:label>Insulation Type</rdfs:label>
		<rdfs:comment>Indicates a kind, type, or category of insulation.</rdfs:comment>
		<rdfs:range>
			<owl:equivalentClass>
				<owl:complementOf rdf:resource="xsd#boolean"/>
			</owl:equivalentClass>
		</rdfs:range>
	</owl:AnnotationProperty>
	<owl:DatatypeProperty rdf:ID="internalMemory">
		<rdfs:subPropertyOf rdf:resource="av7#memory"/>
		<rdfs:label>Internal Memory</rdfs:label>
		<rdfs:comment>Indicates whether or not the represented item has onboard memory.</rdfs:comment>
		<rdfs:range rdf:resource="xsd#boolean"/>
	</owl:DatatypeProperty>
	<owl:AnnotationProperty rdf:ID="isbn">
		<rdfs:label>ISBN</rdfs:label>
		<rdfs:comment>International Standard Book Number. Maintained and defined by ISBN.org.</rdfs:comment>
		<sorg:relatedLink rdf:resource="http://www.isbn.org/about_isbn_standard"/>
	</owl:AnnotationProperty>
	<owl:AnnotationProperty rdf:ID="issn">
		<rdfs:label>ISSN</rdfs:label>
		<rdfs:comment>International Standard Serial Number. A unique global identifier used by vendors to identify their items maintained by ISSN.org.</rdfs:comment>
		<av7:userNotes>Users should input this value as 3 digits followed by a hyphen followed by 3 digits (i.e. ###-###).</av7:userNotes>
		<sorg:relatedLink rdf:resource="http://www.issn.org"/>
	</owl:AnnotationProperty>
	<owl:AnnotationProperty rdf:ID="itemExtendedDescription">
		<rdfs:label>Item Extended Description</rdfs:label>
		<rdfs:comment>Describes the represented item in detail.</rdfs:comment>
	</owl:AnnotationProperty>
	<owl:DatatypeProperty rdf:ID="itemPriceBasisQuantity">
		<rdfs:label>Item Price Basis Quantity</rdfs:label>
		<rdfs:comment>The net quantity of the represented item from which the price per unit cost can be calculated.</rdfs:comment>
		<av7:userNotes>If this attribute obtains a value, 'Item Price Baiss Quantity UOM' must also obtain a value.</av7:userNotes>
		<rdfs:range rdf:resource="xsd#float"/>
	</owl:DatatypeProperty>
	<owl:ObjectProperty rdf:ID="itemPriceBasisQuantityUOM">
		<rdfs:label>Item Price Basis Quantity UOM</rdfs:label>
		<rdfs:comment>Qualifies the value of 'Item Price Basis Quantity'.</rdfs:comment>
		<av7:userNotes>If this attribute obtains a value, 'Item Price Basis Quantity' must also obtain a value.</av7:userNotes>
		<rdfs:range rdf:resource="av7#PackType"/>
	</owl:ObjectProperty>
	<owl:DatatypeProperty rdf:ID="jankaHardness">
		<rdfs:label>Janka Hardness</rdfs:label>
		<rdfs:comment>Indicates how the represented item scores against the Janka Hardness Test in pounds-force.</rdfs:comment>
		<rdfs:range rdf:resource="xsd#integer"/>
	</owl:DatatypeProperty>
	<owl:AnnotationProperty rdf:ID="jewelryStyle">
		<rdfs:label>Jewelry Style</rdfs:label>
		<rdfs:comment>Indicates the style of jewelry being represented.</rdfs:comment>
	</owl:AnnotationProperty>
	<owl:AnnotationProperty rdf:ID="keyActiveIngredients">
		<rdfs:label>Key Active Ingredients</rdfs:label>
		<rdfs:comment>Lists ingredients in the represented item which are considered important by the seller for marketing or other purposes.</rdfs:comment>
	</owl:AnnotationProperty>
	<owl:AnnotationProperty rdf:ID="keywords">
		<rdfs:label>Keywords</rdfs:label>
		<rdfs:comment>Lists keywords associated with the represented item.</rdfs:comment>
		<av7:userNotes>This attribute is typically used to improve search engine optimization (SEO).</av7:userNotes>
	</owl:AnnotationProperty>
	<owl:ObjectProperty rdf:ID="kickPoint">
		<rdfs:label>Kick Point</rdfs:label>
		<rdfs:comment>Indicates which part of a shaft exhibits the greatest amount of bend.</rdfs:comment>
		<wmlo:userNotes>Kick point is also referred to as 'flex point' or 'bend point.'</wmlo:userNotes>
	</owl:ObjectProperty>
	<owl:DatatypeProperty rdf:ID="lampLife">
		<rdfs:label>Lamp Life</rdfs:label>
		<rdfs:comment>Measures the expected life of the represented lamp in hours.</rdfs:comment>
		<rdfs:range rdf:resource="xsd#float"/>
	</owl:DatatypeProperty>
	<owl:AnnotationProperty rdf:ID="laserColor">
		<rdfs:label>Laser Color</rdfs:label>
		<rdfs:comment>Describes the color of the laser beam emitted by a represented item.</rdfs:comment>
	</owl:AnnotationProperty>
	<owl:DatatypeProperty rdf:ID="leadLawsApplicable">
		<rdfs:label>Lead Laws Applicable</rdfs:label>
		<rdfs:comment>Indicates whether or not the represented item is subject to laws pertaining to lead content. These laws vary by US state.</rdfs:comment>
		<rdfs:range rdf:resource="xsd#boolean"/>
	</owl:DatatypeProperty>
	<owl:AnnotationProperty rdf:ID="league">
		<rdfs:label>League</rdfs:label>
		<rdfs:comment>Indicates the league associated with the represented item.</rdfs:comment>
	</owl:AnnotationProperty>
	<owl:AnnotationProperty rdf:ID="lensColorTint">
		<rdfs:label>Lens Color/Tint</rdfs:label>
		<rdfs:comment>Indicates the color or tint pertaining to the represented lens.</rdfs:comment>
	</owl:AnnotationProperty>
	<owl:DatatypeProperty rdf:ID="lensDiameter">
		<rdfs:label>Lens Diameter</rdfs:label>
		<rdfs:comment>Measures the diameter of a lens in real numbers.</rdfs:comment>
		<wmlo:userNotes>If this attribute obtains a value, 'Lens Diameter UOM' must obtain a value.</wmlo:userNotes>
		<rdfs:range rdf:resource="xsd#float"/>
	</owl:DatatypeProperty>
	<owl:ObjectProperty rdf:ID="lensDiameterUOM">
		<rdfs:label>Lens Diameter UOM</rdfs:label>
		<rdfs:comment>Qualifies the value of 'Lens Diameter.'</rdfs:comment>
		<wmlo:userNotes>If this attribute obtains a value, 'Lens Diameter' must obtain a value.</wmlo:userNotes>
		<rdfs:range rdf:resource="wmlo#SpatialUOM"/>
	</owl:ObjectProperty>
	<owl:DatatypeProperty rdf:ID="lensHeight">
		<rdfs:label>Lens Height</rdfs:label>
		<rdfs:comment>Measures the length of the represented lens.</rdfs:comment>
		<wmlo:userNotes>If this attribute obtains a value, 'Lens Height UOM' must obtain a value.</wmlo:userNotes>
		<rdfs:range rdf:resource="xsd#float"/>
	</owl:DatatypeProperty>
	<owl:ObjectProperty rdf:ID="lensHeightUOM">
		<rdfs:label>Lens Height UOM</rdfs:label>
		<rdfs:comment>Qualifies the value of 'Lens Height.'</rdfs:comment>
		<wmlo:userNotes>If this attribute obtains a value, 'Lens Height' must obtain a value.</wmlo:userNotes>
		<rdfs:range rdf:resource="av7#SpatialUOM"/>
	</owl:ObjectProperty>
	<owl:AnnotationProperty rdf:ID="lensMaterial">
		<rdfs:label>Lens Material</rdfs:label>
		<rdfs:comment>Indicates the material out of which the represented lens is made.</rdfs:comment>
	</owl:AnnotationProperty>
	<owl:AnnotationProperty rdf:ID="lensType">
		<rdfs:label>Lens Type</rdfs:label>
		<rdfs:comment>Indicates the kind of represented lens or the treatment applied to a represented lens.</rdfs:comment>
	</owl:AnnotationProperty>
	<owl:DatatypeProperty rdf:ID="lensWidth">
		<rdfs:label>Lens Width</rdfs:label>
		<rdfs:comment>Measures the width of the represented lens.</rdfs:comment>
		<wmlo:userNotes>If this attribute obtains a value, 'Lens Width UOM' must obtain a value.</wmlo:userNotes>
		<rdfs:range rdf:resource="xsd#float"/>
	</owl:DatatypeProperty>
	<owl:ObjectProperty rdf:ID="lensWidthUOM">
		<rdfs:label>Lens Width UOM</rdfs:label>
		<rdfs:comment>Qualifies the value of 'Lens Width.'</rdfs:comment>
		<wmlo:userNotes>If this attribute obtains a value, 'Lens Width' must obtain a value.</wmlo:userNotes>
		<rdfs:range rdf:resource="av7#SpatialUOM"/>
	</owl:ObjectProperty>
	<owl:DatatypeProperty rdf:ID="clubLieDegree">
		<rdfs:label>Lie Degree</rdfs:label>
		<rdfs:comment>Identifies the represented club's angle from shaft to ground line.</rdfs:comment>
	</owl:DatatypeProperty>
	<owl:DatatypeProperty rdf:ID="lightingFactsLabelRequired">
		<rdfs:label>Lighting Facts Label Required</rdfs:label>
		<rdfs:comment>Indicates whether or not the represented item requires a lighting facts label.</rdfs:comment>
		<rdfs:range rdf:resource="xsd#boolean"/>
	</owl:DatatypeProperty>
	<owl:DatatypeProperty rdf:ID="linePairResolution">
		<rdfs:label>Line Pair Resolution</rdfs:label>
		<rdfs:comment>A resolution measure which uses lines-per-milimeter (versus pixels) to indicate resolution.</rdfs:comment>
		<rdfs:range rdf:resource="xsd#float"/>
	</owl:DatatypeProperty>
	<owl:AnnotationProperty rdf:ID="liningMaterial">
		<rdfs:label>Lining Material</rdfs:label>
		<rdfs:comment>Indicates what sort of material lines the represented item.</rdfs:comment>
	</owl:AnnotationProperty>
	<owl:DatatypeProperty rdf:ID="isLiquid">
		<rdfs:label>Liquid</rdfs:label>
		<rdfs:comment>Indicates whether or not the represented item is entirely or in large part a liquid.</rdfs:comment>
		<rdfs:range rdf:resource="xsd#boolean"/>
	</owl:DatatypeProperty>
	<owl:DatatypeProperty rdf:ID="loadOrderingFactor">
		<rdfs:label>Load Ordering Factor</rdfs:label>
		<rdfs:comment>A numeric measurement exclusive of weight and volume. Used for building orders and loads or for pricing purposes.</rdfs:comment>
		<av7:userNotes>If this attribute obtains a value, 'Load Ordering Factor UOM' must also obtain a value.</av7:userNotes>
		<rdfs:range rdf:resource="xsd#integer"/>
	</owl:DatatypeProperty>
	<owl:ObjectProperty rdf:ID="loadOrderingFactorUOM">
		<rdfs:label>Load Ordering Factor UOM</rdfs:label>
		<rdfs:comment>Idenfifies a specific unit of measure for the load ordering factor as it applies to each item representeted. If this attribute has a value, 'Load Ordreing Factor' must also have a value.</rdfs:comment>
		<av7:userNotes>If this attribute obtains a value, 'Load Ordering Factor' must also obtain a value.</av7:userNotes>
		<rdfs:range rdf:resource="av7#LoadOrderingFactorUOM"/>
	</owl:ObjectProperty>
	<owl:AnnotationProperty rdf:ID="hasLocationID">
		<rdfs:label>Resource</rdfs:label>
		<rdfs:comment>The ship-from location identifier.</rdfs:comment>
		<av7:userNotes>Location can be used only if vendor has provided shipping location information via the IMS UI.</av7:userNotes>
	</owl:AnnotationProperty>
	<owl:AnnotationProperty rdf:ID="locationsRequiringSpecialLabeling">
		<rdfs:label>Locations Requiring Special Labeling</rdfs:label>
		<rdfs:comment>Lists US states that require special labeling. States should be expressed as 2 letter abbreviations.</rdfs:comment>
	</owl:AnnotationProperty>
	<owl:DatatypeProperty rdf:ID="lockable">
		<rdfs:label>Lockable</rdfs:label>
		<rdfs:comment>Indicates whether or not the represented item may be locked.</rdfs:comment>
		<rdfs:range rdf:resource="xsd#boolean"/>
	</owl:DatatypeProperty>
	<owl:DatatypeProperty rdf:ID="clubLoftDegree">
		<rdfs:label>Loft Degree</rdfs:label>
		<rdfs:comment>Indicates the degree of a represented club's face-angle relative to the vertical plane (rather than the ground).</rdfs:comment>
		<rdfs:range rdf:resource="xsd#float"/>
	</owl:DatatypeProperty>
	<owl:AnnotationProperty rdf:ID="longMarketingMessage">
		<rdfs:label>Long Marketing Message</rdfs:label>
		<rdfs:comment>Communicates a detailed marketing message, description, tagline, or other text associated with the represented item.</rdfs:comment>
		<av7:userNotes>This attribute typically communicates short, consumer-friendly headlines such as brand slogan, product purpose, and e-commerce site quick views.</av7:userNotes>
	</owl:AnnotationProperty>
	<owl:DatatypeProperty rdf:ID="lotSensitive">
		<rdfs:label>Lot Sensitive</rdfs:label>
		<rdfs:comment>Identifies whether or not an item might differ from items in its model due to variations in production lot.</rdfs:comment>
		<rdfs:range rdf:resource="xsd#boolean"/>
	</owl:DatatypeProperty>
	<owl:DatatypeProperty rdf:ID="madeFromRecycledMaterial">
		<rdfs:subPropertyOf rdf:resource="av7#recycling"/>
		<rdfs:label>Made From Recycled Material</rdfs:label>
		<rdfs:comment>Indicates whether or not a represented item is made from recycled material.</rdfs:comment>
		<rdfs:range rdf:resource="xsd#boolean"/>
	</owl:DatatypeProperty>
	<owl:DatatypeProperty rdf:ID="madeToOrder">
		<rdfs:label>Made To Order</rdfs:label>
		<rdfs:comment>Indicates whether or not an item can be made to order.</rdfs:comment>
		<rdfs:range rdf:resource="xsd#boolean"/>
	</owl:DatatypeProperty>
	<owl:DatatypeProperty rdf:ID="maxMagnification">
		<rdfs:subPropertyOf rdf:resource="av7#magnification"/>
		<rdfs:label>Maximum Magnification</rdfs:label>
		<rdfs:comment>Describes the greatest degree of magnification that the represented device is able to produce in real numbers. This measure may sometimes be referred to as 'zoom.''</rdfs:comment>
		<rdfs:range rdf:resource="xsd#float"/>
	</owl:DatatypeProperty>
	<owl:DatatypeProperty rdf:ID="hasManualGain">
		<rdfs:label>Manual Gain</rdfs:label>
		<rdfs:comment>Indicates whether or not users of a represented item may manually adjust input signal strength without using other devices.</rdfs:comment>
		<wmlo:userNotes>In optics, 'signal' refers to image quality; in audio, 'signal' refers to sound quality; etc.</wmlo:userNotes>
		<rdfs:range rdf:resource="xsd#boolean"/>
	</owl:DatatypeProperty>
	<owl:AnnotationProperty rdf:ID="manufacturerName">
		<rdfs:label>Manufacturer Name</rdfs:label>
		<rdfs:comment>Indicates item manufacturer.</rdfs:comment>
	</owl:AnnotationProperty>
	<owl:AnnotationProperty rdf:ID="manufacturerPartNumber">
		<rdfs:label>Manufacturer Part Number</rdfs:label>
		<rdfs:comment>Indicates the manufacturer-created number used by a vendor who is not the original manufacturer, such as a distributor or a reseller.</rdfs:comment>
	</owl:AnnotationProperty>
	<owl:AnnotationProperty rdf:ID="masterPackCaseGTIN">
		<rdfs:label>Master Pack or Case GTIN</rdfs:label>
		<rdfs:comment>The GTIN which identifies a unique master pack or case, which contains unique inner pack(s).</rdfs:comment>
	</owl:AnnotationProperty>
	<owl:DatatypeProperty rdf:ID="masterPackCaseHeight">
		<rdfs:label>Master Pack or Case Height</rdfs:label>
		<rdfs:comment>Describes the height of a master pack or case in real numbers.</rdfs:comment>
		<av7:userNotes>If this attribute obtains a value, 'Master Pack or Case Height UOM' must also obtain a value.</av7:userNotes>
		<rdfs:range rdf:resource="xsd#float"/>
	</owl:DatatypeProperty>
	<owl:ObjectProperty rdf:ID="masterPackCaseHeightUOM">
		<rdfs:label>Master Pack or Case Height UOM</rdfs:label>
		<rdfs:comment>Indicates the specific unit of measure which describes the value of 'Master Pack or Case Height.'</rdfs:comment>
		<av7:userNotes>If this attribute obtains a value, 'Master Pack or Case Height' must also obtain a value.</av7:userNotes>
		<rdfs:range rdf:resource="av7#SpatialUOM"/>
	</owl:ObjectProperty>
	<owl:DatatypeProperty rdf:ID="masterPackCaseLength">
		<rdfs:label>Master Pack or Case Length</rdfs:label>
		<rdfs:comment>Describes the length of a master pack or case in real numbers.</rdfs:comment>
		<av7:userNotes>If this attribute obtains a value, 'Master Pack or Case Length UOM' must also obtain a value.</av7:userNotes>
		<rdfs:range rdf:resource="xsd#float"/>
	</owl:DatatypeProperty>
	<owl:ObjectProperty rdf:ID="masterPackCaseLengthUOM">
		<rdfs:label>Master Pack or Case Length UOM</rdfs:label>
		<rdfs:comment>Indicates the specific unit of measure which describes the value of 'Master Pack or Case Length.'</rdfs:comment>
		<av7:userNotes>If this attribute obtains a value, 'Master Pack or Case Length' must also obtain a value.</av7:userNotes>
		<rdfs:range rdf:resource="av7#SpatialUOM"/>
	</owl:ObjectProperty>
	<owl:DatatypeProperty rdf:ID="masterPackCaseVolume">
		<rdfs:label>Master Pack or Case Volume</rdfs:label>
		<rdfs:comment>Describes the volume of a master pack or case in real numbers.</rdfs:comment>
		<av7:userNotes>If this attribute obtains a value, 'Master Pack or Case Volume UOM' must also obtain a value.</av7:userNotes>
		<rdfs:range rdf:resource="xsd#float"/>
	</owl:DatatypeProperty>
	<owl:ObjectProperty rdf:ID="masterPackCaseVolumeUOM">
		<rdfs:label>Master Pack or Case Volume UOM</rdfs:label>
		<rdfs:comment>Indicates the specific unit of measure which describes the value of 'Master Pack or Case Volume.'</rdfs:comment>
		<av7:userNotes>If this attribute obtains a value, 'Master Pack or Case Volume' must also obtain a value.</av7:userNotes>
		<rdfs:range rdf:resource="av7#PackVolumeUOM"/>
	</owl:ObjectProperty>
	<owl:DatatypeProperty rdf:ID="masterPackCaseWeight">
		<rdfs:label>Master Pack or Case Weight</rdfs:label>
		<rdfs:comment>Describes the weight of a master pack or case in real numbers.</rdfs:comment>
		<av7:userNotes>If this attribute obtains a value, 'Master Pack or Case Weight UOM' must also obtain a value.</av7:userNotes>
		<rdfs:range rdf:resource="xsd#float"/>
	</owl:DatatypeProperty>
	<owl:ObjectProperty rdf:ID="masterPackCaseWeightUOM">
		<rdfs:label>Master Pack or Case Weight UOM</rdfs:label>
		<rdfs:comment>Indicates the specific unit of measure which describes the value of 'Master Pack or Case Weight.'</rdfs:comment>
		<av7:userNotes>If this attribute obtains a value, 'Master Pack or Case Weight' must also obtain a value.</av7:userNotes>
		<rdfs:range rdf:resource="av7#PackWeightUOM"/>
	</owl:ObjectProperty>
	<owl:DatatypeProperty rdf:ID="masterPackCaseWidth">
		<rdfs:label>Master Pack or Case Width</rdfs:label>
		<rdfs:comment>Describes the width of a master pack or case in real numbers.</rdfs:comment>
		<av7:userNotes>If this attribute obtains a value, 'Master Pack or Case Width UOM' must also obtain a value.</av7:userNotes>
		<rdfs:range rdf:resource="xsd#float"/>
	</owl:DatatypeProperty>
	<owl:ObjectProperty rdf:ID="masterPackCaseWidthUOM">
		<rdfs:label>Master Pack or Case Width UOM</rdfs:label>
		<rdfs:comment>Indicates the specific unit of measure which describes the value of 'Master Pack or Case Width.'</rdfs:comment>
		<av7:userNotes>If this attribute obtains a value, 'Master Pack or Case Width' must also obtain a value.</av7:userNotes>
		<rdfs:range rdf:resource="av7#SpatialUOM"/>
	</owl:ObjectProperty>
	<owl:DatatypeProperty rdf:ID="materialSafetySheetRequired">
		<rdfs:label>Material Safety Sheet Required</rdfs:label>
		<rdfs:comment>Indicates whether or not the represented item requires a material safety data sheet to accompany it when sold.</rdfs:comment>
		<sorg:relatedLink rdf:resource="https://www.osha.gov/html/faq-hazoom.html"/>
		<rdfs:range rdf:resource="xsd#boolean"/>
	</owl:DatatypeProperty>
	<owl:DatatypeProperty rdf:ID="maximumConsumerItemHeight">
		<rdfs:label>Maximum Consumer Item Height</rdfs:label>
		<rdfs:comment>Indicates the maximum height achieved by an unboxed, assembled item.</rdfs:comment>
		<av7:userNotes>If this attribute obtains a value, 'Consumer Item Height UOM' must also obtain a value.</av7:userNotes>
		<rdfs:range rdf:resource="xsd#float"/>
	</owl:DatatypeProperty>
	<owl:DatatypeProperty rdf:ID="maximumDistanceNonReflectiveTarget">
		<rdfs:label>Maximum Distance Non-Reflective Target</rdfs:label>
		<rdfs:comment>Defines in real numbers the maximum distance at which a represented item is able to target a non-reflective object.</rdfs:comment>
		<av7:userNotes>If this attribute obtains a value, 'Maximum Distance Non-Reflective Target UOM' must obtain a value.</av7:userNotes>
		<rdfs:range rdf:resource="xsd#float"/>
	</owl:DatatypeProperty>
	<owl:ObjectProperty rdf:ID="maximumDistanceNonReflectiveTargetUOM">
		<rdfs:label>Maximum Distance Non-Reflective Target UOM</rdfs:label>
		<rdfs:comment>Qualifies the value of 'Maximum Distance Non-Reflective Target.'</rdfs:comment>
		<av7:userNotes>If this attribute obtains a value, 'Maximum Distance Non-Reflective Target' must obtain a value.</av7:userNotes>
		<rdfs:range rdf:resource="av7#SpatialUOM"/>
	</owl:ObjectProperty>
	<owl:DatatypeProperty rdf:ID="maximumDistanceReflectiveTarget">
		<rdfs:label>Maximum Distance Reflective Target</rdfs:label>
		<rdfs:comment>Defines in real numbers the maximum distance at which a represented item is able to target a reflective object.</rdfs:comment>
		<av7:userNotes>If this attribute obtains a value, 'Maximum Distance Reflective Target UOM' must obtain a value.</av7:userNotes>
		<rdfs:range rdf:resource="xsd#float"/>
	</owl:DatatypeProperty>
	<owl:ObjectProperty rdf:ID="maximumDistanceReflectiveTargetUOM">
		<rdfs:label>Maximum Distance Reflective Target UOM</rdfs:label>
		<rdfs:comment>Qualifies the value of 'Maximum Distance Reflective Target.'</rdfs:comment>
		<av7:userNotes>If this attribute obtains a value, 'Maximum Distance Reflective Target' must obtain a value.</av7:userNotes>
		<rdfs:range rdf:resource="av7#SpatialUOM"/>
	</owl:ObjectProperty>
	<owl:DatatypeProperty rdf:ID="maximumElevationAdustment">
		<rdfs:label>Maximum Elevation Adjustment</rdfs:label>
		<rdfs:comment>Indicates the maximum distance to which an optical device is rated to sight when elevation and minute of angle turrets set are at maximum clicks.</rdfs:comment>
		<av7:userNotes>If this attribute obtains a value, 'Maximum Elevation Adjustment UOM' must obtain a value.</av7:userNotes>
		<rdfs:range rdf:resource="xsd#float"/>
	</owl:DatatypeProperty>
	<owl:ObjectProperty rdf:ID="maximumElevationAdustmentUOM">
		<rdfs:label>Maximum Elevation Adjustment UOM</rdfs:label>
		<rdfs:comment>Qualifies the value of 'Maximum Elevation Adjustment.'</rdfs:comment>
		<av7:userNotes>If this attribute obtains a value, 'Maximum Elevation Adjustment' must obtain a value.</av7:userNotes>
		<rdfs:range rdf:resource="av7#SpatialUOM"/>
	</owl:ObjectProperty>
	<owl:DatatypeProperty rdf:ID="maximumItemUseWeight">
		<rdfs:label>Maximum Item Use Weight</rdfs:label>
		<rdfs:comment>Indicates a maximum weight appropriate for use with the represented item.</rdfs:comment>
		<av7:userNotes>If this attribute obtains a value, Maximum Item Use Weight UOM' must obtain a value.</av7:userNotes>
		<rdfs:range rdf:resource="xsd#float"/>
	</owl:DatatypeProperty>
	<owl:ObjectProperty rdf:ID="maximumItemUseWeightUOM">
		<rdfs:label>Maximum Item Use Weight UOM</rdfs:label>
		<rdfs:comment>Qualifies the value of 'Maximum Item Use Weightt.'</rdfs:comment>
		<av7:userNotes>If this attribute obtains a value, 'Maximum Item Use Weight' must obtain a value.</av7:userNotes>
		<rdfs:range rdf:resource="av7#PackWeightUOM"/>
	</owl:ObjectProperty>
	<owl:DatatypeProperty rdf:ID="maximumOrderQty">
		<rdfs:label>Maximum Order Quantity</rdfs:label>
		<rdfs:comment>Indicates the maximum quantity of an item that may be ordered at one time.</rdfs:comment>
		<rdfs:range rdf:resource="xsd#integer"/>
	</owl:DatatypeProperty>
	<owl:DatatypeProperty rdf:ID="maximumStorageTemperature">
		<rdfs:subPropertyOf rdf:resource="av7#storageTemperature"/>
		<rdfs:label>Maximum Storage Temperature</rdfs:label>
		<rdfs:comment>Indicates the maximum temperature at which a represnted item may be stored.</rdfs:comment>
		<av7:userNotes>If this attribute obtains a value, 'Maximum/Minimum Storage Temperature UOM' must also obtain a value.</av7:userNotes>
		<rdfs:range rdf:resource="xsd#float"/>
	</owl:DatatypeProperty>
	<owl:DatatypeProperty rdf:ID="maximumWattage">
		<rdfs:label>Resource</rdfs:label>
		<rdfs:comment>Indicates the maximum wattage output by the represented item.</rdfs:comment>
		<rdfs:range rdf:resource="xsd#float"/>
	</owl:DatatypeProperty>
	<owl:DatatypeProperty rdf:ID="maximumWindageAdjustment">
		<rdfs:label>Maximum Windage Adjustment</rdfs:label>
		<rdfs:comment>Indicates the maximum distance to which an optical device is rated to sight when windage and minute of angle turrets set are at maximum clicks.</rdfs:comment>
		<av7:userNotes>If this attribute obtains a value, 'Maximum Windage Adjustment UOM' must obtain a value.</av7:userNotes>
		<rdfs:range rdf:resource="xsd#float"/>
	</owl:DatatypeProperty>
	<owl:ObjectProperty rdf:ID="maximumWindageAdjustmentUOM">
		<rdfs:label>Maximum Windage Adjustmen UOM</rdfs:label>
		<rdfs:comment>Qualifies the value of 'Maximum Windage Adjustment.'</rdfs:comment>
		<av7:userNotes>If this attribute obtains a value, 'Maximum Windage Adjustment' must obtain a value.</av7:userNotes>
		<rdfs:range rdf:resource="av7#SpatialUOM"/>
	</owl:ObjectProperty>
	<owl:AnnotationProperty rdf:ID="mediaDescription">
		<rdfs:label>Resource</rdfs:label>
		<rdfs:comment>Desribes the represented digital asset.</rdfs:comment>
		<av7:userNotes>Resource</av7:userNotes>
	</owl:AnnotationProperty>
	<owl:AnnotationProperty rdf:ID="mediaFileName">
		<rdfs:label>Resource</rdfs:label>
		<rdfs:comment>Indicates the truncated filename plus extension of the digital asset represented.</rdfs:comment>
		<av7:userNotes>If this attribute obtains a value, 'Media Name' must also obtain a value.</av7:userNotes>
	</owl:AnnotationProperty>
	<owl:DatatypeProperty rdf:ID="mediaFileSizeInBytes">
		<rdfs:label>Resource</rdfs:label>
		<rdfs:comment>Indicates the truncated filename plus extension of the digital asset represented measured in bytes.</rdfs:comment>
		<av7:userNotes>If this attribute obtains a value, 'Media Name' must also obtain a value.</av7:userNotes>
		<rdfs:range rdf:resource="xsd#float"/>
	</owl:DatatypeProperty>
	<owl:AnnotationProperty rdf:ID="mediaFileExtension">
		<rdfs:label>Resource</rdfs:label>
		<rdfs:comment>Indicates the format of the represented digital asset; usually the same as its file extension.</rdfs:comment>
		<av7:userNotes>Resource</av7:userNotes>
	</owl:AnnotationProperty>
	<owl:DatatypeProperty rdf:ID="mediaImageHeight">
		<rdfs:label>Resource</rdfs:label>
		<rdfs:comment>Indicates the height of the represented digital asset in pixels.</rdfs:comment>
		<av7:userNotes>If this attribute obtains a value, 'Media Name' must also obtain a value.</av7:userNotes>
		<rdfs:range rdf:resource="xsd#float"/>
	</owl:DatatypeProperty>
	<owl:DatatypeProperty rdf:ID="mediaImageWidth">
		<rdfs:label>Resource</rdfs:label>
		<rdfs:comment>Indicates the width of the represented digital asset in pixels.</rdfs:comment>
		<av7:userNotes>If this attribute obtains a value, 'Media Name' must also obtain a value.</av7:userNotes>
		<rdfs:range rdf:resource="xsd#float"/>
	</owl:DatatypeProperty>
	<owl:AnnotationProperty rdf:ID="mediaOnScreenLocation">
		<rdfs:label>Media Name</rdfs:label>
		<rdfs:comment>Identifies the relative orientation or cardinality of the represented digital asset.</rdfs:comment>
		<av7:userNotes>Resource</av7:userNotes>
	</owl:AnnotationProperty>
	<owl:AnnotationProperty rdf:ID="mediaOrientation">
		<rdfs:label>Resource</rdfs:label>
		<rdfs:comment>Indicates the on-screen orientation of the represented digital asset.</rdfs:comment>
		<av7:userNotes>Resource</av7:userNotes>
	</owl:AnnotationProperty>
	<owl:AnnotationProperty rdf:ID="mediaPixelDensity">
		<rdfs:label>Resource</rdfs:label>
		<rdfs:comment>Indicates the pixel density of the represented digital asset.</rdfs:comment>
		<av7:userNotes>If this attribute obtains a value, 'Media Name' must also obtain a value.</av7:userNotes>
	</owl:AnnotationProperty>
	<owl:AnnotationProperty rdf:ID="mediaPurpose">
		<rdfs:label>Resource</rdfs:label>
		<rdfs:comment>Indicates the purpose or end use of the represented digital asset.</rdfs:comment>
		<av7:userNotes>Resource</av7:userNotes>
	</owl:AnnotationProperty>
	<owl:AnnotationProperty rdf:ID="mediaDocumentPurpose">
		<rdfs:label>Resource</rdfs:label>
		<rdfs:comment>Identifies the purpose-oriented type associated with the value of 'Media URL'.</rdfs:comment>
		<av7:userNotes>If this attribute obtains a value, 'Media Name' and 'Media URL' must also obtain values.</av7:userNotes>
	</owl:AnnotationProperty>
	<owl:ObjectProperty rdf:ID="mediaURL">
		<rdfs:label>Resource</rdfs:label>
		<rdfs:comment>Identifies the unique resource locator (URL) of the represented digital asset.</rdfs:comment>
		<av7:userNotes>If this attribute obtains a value, 'Media Name' must also obtain a value.</av7:userNotes>
		<rdfs:range rdf:resource="rdf#Resource"/>
	</owl:ObjectProperty>
	<owl:AnnotationProperty rdf:ID="mediaAngleOfView">
		<rdfs:label>Resource</rdfs:label>
		<rdfs:comment>Identifies the angle of view pertaining to the represented digital asset; including but not limited to images.</rdfs:comment>
		<av7:userNotes>If this attribute obtains a value, 'Media Name' must also obtain a value.</av7:userNotes>
	</owl:AnnotationProperty>
	<owl:AnnotationProperty rdf:ID="merchandiseDisplayDescription">
		<rdfs:label>Merchandise Display Description</rdfs:label>
		<rdfs:comment>Describes how a represented item might be displayed in the brick-and-mortar retail store.</rdfs:comment>
	</owl:AnnotationProperty>
	<owl:DatatypeProperty rdf:ID="minimumConsumerItemHeight">
		<rdfs:label>Minimum Consumer Item Height</rdfs:label>
		<rdfs:comment>Indicates the minimum height achieved by an unboxed, assembled item.</rdfs:comment>
		<av7:userNotes> If this attribute obtains a value, 'Consumer Item Height' must also obtain a value.</av7:userNotes>
		<rdfs:range rdf:resource="xsd#float"/>
	</owl:DatatypeProperty>
	<owl:DatatypeProperty rdf:ID="minimumOrderQty">
		<rdfs:label>Minimum Order Quantity</rdfs:label>
		<rdfs:comment>Indicates the minimum quantity of an item that may be ordered at one time.</rdfs:comment>
		<rdfs:range rdf:resource="xsd#integer"/>
	</owl:DatatypeProperty>
	<owl:DatatypeProperty rdf:ID="minimumStorageTemperature">
		<rdfs:subPropertyOf rdf:resource="av7#storageTemperature"/>
		<rdfs:label>Minimum Storage Temperature</rdfs:label>
		<rdfs:comment>Indicates the minimum temperature at which a represnted item may be stored.</rdfs:comment>
		<av7:userNotes> If this attribute obtains a value, 'Minimum/Maximum Storage Temperature UOM' must also obtain a value.</av7:userNotes>
		<rdfs:range rdf:resource="xsd#float"/>
	</owl:DatatypeProperty>
	<owl:ObjectProperty rdf:ID="minimumMaximumStorageTemperatureUOM">
		<rdfs:subPropertyOf rdf:resource="av7#storageTemperature"/>
		<rdfs:label>Mininum/Maximum Storage Temperature UOM</rdfs:label>
		<rdfs:comment>Describes the value of 'Maximum Storage Temperature.'</rdfs:comment>
		<av7:userNotes>If this attribute obtains a value, 'Minimum/Maximum Storage Temperature' must also obtain a value.</av7:userNotes>
		<rdfs:range rdf:resource="av7#TempUOM"/>
	</owl:ObjectProperty>
	<owl:DatatypeProperty rdf:ID="minuteOfAngle">
		<rdfs:label>Minute of Angle</rdfs:label>
		<rdfs:comment>Indicates minute of angle (MOA), or how much a represented projectile's path will vary over time and distance, per click of a scope.</rdfs:comment>
		<rdfs:range rdf:resource="xsd#float"/>
	</owl:DatatypeProperty>
	<owl:AnnotationProperty rdf:ID="mode">
		<rdfs:label>Mode</rdfs:label>
		<rdfs:comment>Lists the programs available as an integral part of a represented item.</rdfs:comment>
	</owl:AnnotationProperty>
	<owl:AnnotationProperty rdf:ID="model">
		<rdfs:label>Model</rdfs:label>
		<rdfs:comment>Denotes an alphanumeric signifier used to differentiate one product in a series from another.</rdfs:comment>
	</owl:AnnotationProperty>
	<owl:AnnotationProperty rdf:ID="mountType">
		<rdfs:label>Mount Type</rdfs:label>
		<rdfs:comment>Describes how a represented item may be mounted; may reference what in particular is used to fasten one item to another (e.g. Screws, Rail System).</rdfs:comment>
	</owl:AnnotationProperty>
	<owl:ObjectProperty rdf:ID="mpaaRating">
		<rdfs:label>MPAA Rating</rdfs:label>
		<rdfs:comment>Indicates how the Motion Picture Association of America rates a represented item.</rdfs:comment>
		<rdfs:range rdf:resource="av7#MPAARating"/>
	</owl:ObjectProperty>
	<owl:AnnotationProperty rdf:ID="neckline">
		<rdfs:label>Neckline</rdfs:label>
		<rdfs:comment>Describes the top edge of the represented garment as it surrounds the neck; typically viewed from the front.</rdfs:comment>
	</owl:AnnotationProperty>
	<owl:DatatypeProperty rdf:ID="neckSize">
		<rdfs:label>Neck Size</rdfs:label>
		<rdfs:comment>Measures the neck of a represented item.</rdfs:comment>
		<wmlo:userNotes>If this attribute obtains a value, 'Neck Size UOM' must obtain a value.</wmlo:userNotes>
		<rdfs:range rdf:resource="xsd#float"/>
	</owl:DatatypeProperty>
	<owl:ObjectProperty rdf:ID="neckSizeUOM">
		<rdfs:label>Neck Size UOM</rdfs:label>
		<rdfs:comment>Qualifies the value of 'Neck Size.'</rdfs:comment>
		<wmlo:userNotes>If this attribute obtains a value, 'Neck Size' must obtain a value.</wmlo:userNotes>
		<rdfs:range rdf:resource="av7#SpatialUOM"/>
	</owl:ObjectProperty>
	<owl:ObjectProperty rdf:ID="newConstructionExistingStructure">
		<rdfs:label>New Construction/Existing Structure</rdfs:label>
		<rdfs:comment>Indicates whether the represented item is appropriate for new construction, for existing structures, or both.</rdfs:comment>
	</owl:ObjectProperty>
	<owl:AnnotationProperty rdf:ID="nfpaStorageClassification">
		<rdfs:label>NFPA Storage Classification</rdfs:label>
		<rdfs:comment>Lists codes defined by the National Fire Protection Association which pertain to the represented item.</rdfs:comment>
		<sorg:relatedLink rdf:resource="http://www.nfpa.org/codes-and-standards/document-information-pages"/>
	</owl:AnnotationProperty>
	<owl:AnnotationProperty rdf:ID="nrfColorCode">
		<rdfs:label>NRF Color Code</rdfs:label>
		<rdfs:comment>Identifies item color according to the Nation Retail Federation's standard.</rdfs:comment>
		<sorg:relatedLink rdf:resource="http://nrf.com/resources/retail-library/standard-color-and-size-codes"/>
	</owl:AnnotationProperty>
	<owl:AnnotationProperty rdf:ID="nrfSizeCode">
		<rdfs:label>NRF Size Code</rdfs:label>
		<rdfs:comment>Identifies item size according to the Nation Retail Federation's standard.</rdfs:comment>
		<sorg:relatedLink rdf:resource="http://nrf.com/resources/retail-library/standard-color-and-size-codes"/>
	</owl:AnnotationProperty>
	<owl:DatatypeProperty rdf:ID="numberOfBasins">
		<rdfs:label>Number Of Basins</rdfs:label>
		<rdfs:comment>Indicates the number of basins that comprise the represented item or which the represented item will accomodate.</rdfs:comment>
		<rdfs:range rdf:resource="xsd#integer"/>
	</owl:DatatypeProperty>
	<owl:DatatypeProperty rdf:ID="numberOfBreakers">
		<rdfs:label>Number Of Breakers</rdfs:label>
		<rdfs:comment>Indicates the number of electrical breakers that comprise the represented item or which the represented item will accomodate.</rdfs:comment>
		<rdfs:range rdf:resource="xsd#integer"/>
	</owl:DatatypeProperty>
	<owl:DatatypeProperty rdf:ID="numberOfCircuitsProtected">
		<rdfs:label>Number Of Circuits Protected</rdfs:label>
		<rdfs:comment>Indicates the number of electrical circuits that the represented item protects.</rdfs:comment>
		<rdfs:range rdf:resource="xsd#integer"/>
	</owl:DatatypeProperty>
	<owl:DatatypeProperty rdf:ID="numberOfConductors">
		<rdfs:label>Number Of Conductors</rdfs:label>
		<rdfs:comment>Indicates the number of conductors that comprise the represented item or which the represented item will accomodate.</rdfs:comment>
		<rdfs:range rdf:resource="xsd#integer"/>
	</owl:DatatypeProperty>
	<owl:DatatypeProperty rdf:ID="numberOfTelescopingSections">
		<rdfs:label>Number of Telescoping Sections</rdfs:label>
		<rdfs:comment>Indicates the number of telescoping sections on a represented item or on a part of an item (i.e., the back of an extendable camper, or the leg of a tripod).</rdfs:comment>
		<rdfs:range rdf:resource="xsd#float"/>
	</owl:DatatypeProperty>
	<owl:DatatypeProperty rdf:ID="nutritionFactsLabelRequired">
		<rdfs:label>Nutrition Facts Label Required</rdfs:label>
		<rdfs:comment>Indicates whether or not the represented item requires a nutrition facts label.</rdfs:comment>
		<rdfs:range rdf:resource="xsd#boolean"/>
	</owl:DatatypeProperty>
	<owl:DatatypeProperty rdf:ID="objectiveDiameterMM">
		<rdfs:label>Objective Diameter MM</rdfs:label>
		<rdfs:comment>Indicates the diameter of an optical device's light-admitting apparatus, measured in real numbers. The unit of measure is always millimeters. Given the same magnification, the larger the objective diameter, the greater the light-collecting power.</rdfs:comment>
		<rdfs:range rdf:resource="xsd#float"/>
	</owl:DatatypeProperty>
	<owl:DatatypeProperty rdf:ID="obsoleteStockAvailable">
		<rdfs:label>Obsolete Stock Available</rdfs:label>
		<rdfs:comment>Indicates whether or not ther is stock available should the represented item be obsolete.</rdfs:comment>
		<rdfs:range rdf:resource="xsd#boolean"/>
	</owl:DatatypeProperty>
	<owl:DatatypeProperty rdf:ID="openTime">
		<rdfs:label>Open Time</rdfs:label>
		<rdfs:comment>The amount of time that an item must be exposed to the working environment before it may be applied.</rdfs:comment>
		<wmlo:userNotes>If this attribute obtains a value, 'Open Time UOM' must obtain a value.</wmlo:userNotes>
		<rdfs:range rdf:resource="xsd#float"/>
	</owl:DatatypeProperty>
	<owl:ObjectProperty rdf:ID="openTimeUOM">
		<rdfs:label>Open Time UOM</rdfs:label>
		<rdfs:comment>Qualifies the value of 'Open Time.'</rdfs:comment>
		<wmlo:userNotes>If this attribute obtains a value, 'Open Time' must obtain a value.</wmlo:userNotes>
		<rdfs:range rdf:resource="av7#OpenTimeUOM"/>
	</owl:ObjectProperty>
	<owl:AnnotationProperty rdf:ID="operatingSystem">
		<rdfs:label>Operating System</rdfs:label>
		<rdfs:comment>Names the operating system installed on or associated with the represented item.</rdfs:comment>
	</owl:AnnotationProperty>
	<owl:DatatypeProperty rdf:ID="opticalInputs">
		<rdfs:label>Optical Inputs</rdfs:label>
		<rdfs:comment>Indicates the number of optical inputs onboard or supported by a represented item.</rdfs:comment>
		<rdfs:range rdf:resource="xsd#integer"/>
	</owl:DatatypeProperty>
	<owl:DatatypeProperty rdf:ID="opticalOutputs">
		<rdfs:label>Optical Outputs</rdfs:label>
		<rdfs:comment>Indicates the number of optical outputs onboard or supported by a represented item.</rdfs:comment>
		<rdfs:range rdf:resource="xsd#integer"/>
	</owl:DatatypeProperty>
	<owl:DatatypeProperty rdf:ID="orderLeadTime">
		<rdfs:label>Order Lead Time</rdfs:label>
		<rdfs:comment>Measures lead time from the date of order placement to shipment date.</rdfs:comment>
		<av7:userNotes>If this attributes obtains a value, 'Order Lead Time Code' must also obtain a value.</av7:userNotes>
		<rdfs:range rdf:resource="xsd#integer"/>
	</owl:DatatypeProperty>
	<owl:ObjectProperty rdf:ID="orderLeadTimeCode">
		<rdfs:label>Order Lead Time Code</rdfs:label>
		<av7:userNotes>If this attributes obtains a value, 'Order Lead Time' must also obtain a value.</av7:userNotes>
		<rdfs:range rdf:resource="xsd#OrderLeadTimeCode"/>
	</owl:ObjectProperty>
	<owl:DatatypeProperty rdf:ID="orderQtyMultiple">
		<rdfs:label>Order Quantity Multiple</rdfs:label>
		<rdfs:comment>Indicates the order quantity multiple in which an item may be ordered.</rdfs:comment>
		<rdfs:range rdf:resource="xsd#float"/>
	</owl:DatatypeProperty>
	<owl:DatatypeProperty rdf:ID="organic">
		<rdfs:label>Organic</rdfs:label>
		<rdfs:comment>Indicates whether or not the represented item is certified organic by a regulatory organization.</rdfs:comment>
		<rdfs:range rdf:resource="xsd#boolean"/>
	</owl:DatatypeProperty>
	<owl:DatatypeProperty rdf:ID="ormD">
		<rdfs:label>ORM-D</rdfs:label>
		<rdfs:comment>Indicates whether or not a represented item is eligible to be shipped with an ORM-D designation, in other words, whether it has in it hazardous materials in limited quantitities.</rdfs:comment>
		<av7:userNotes>Usually used to describe consumer commodities.</av7:userNotes>
		<rdfs:range rdf:resource="xsd#boolean"/>
	</owl:DatatypeProperty>
	<owl:DatatypeProperty rdf:ID="outerDiameter">
		<rdfs:label>Outer Diameter</rdfs:label>
		<rdfs:comment>Indicates the measure of an object's outer diameter; of particular use for tubular objects.</rdfs:comment>
		<av7:userNotes> If this attribute obtains a value, 'Outer Diameter UOM' must also obtain a value.</av7:userNotes>
		<rdfs:range rdf:resource="xsd#float"/>
	</owl:DatatypeProperty>
	<owl:ObjectProperty rdf:ID="outerDiameterUOM">
		<rdfs:label>Outer Diameter UOM</rdfs:label>
		<rdfs:comment>Describes the value of 'Outer Diameter.'</rdfs:comment>
		<av7:userNotes>If this attribute obtains a value, 'Outer Diameter' must also obtain a value.</av7:userNotes>
		<rdfs:range rdf:resource="av7#SpatialUOM"/>
	</owl:ObjectProperty>
	<owl:DatatypeProperty rdf:ID="outerPackQty">
		<rdfs:label>Outer Pack Quantity</rdfs:label>
		<rdfs:comment>Indicates the toal number of outer packs needed to contain the number of inner packs identified by the value of 'Inner Pack Quantity'.</rdfs:comment>
		<rdfs:range rdf:resource="xsd#float"/>
	</owl:DatatypeProperty>
	<owl:ObjectProperty rdf:ID="packingGroup">
		<rdfs:label>Packing Group</rdfs:label>
		<rdfs:comment>The dangerous goods grouping according to the degree of danger presented by hazardous materials as defined by the US Department of Transportation.</rdfs:comment>
		<rdfs:seeAlso rdf:resource="https://en.wikipedia.org/wiki/Dangerous_goods#Packing_groups"/>
		<rdfs:range rdf:resource="av7#PackingGroup"/>
	</owl:ObjectProperty>
	<owl:AnnotationProperty rdf:ID="pageCount">
		<rdfs:label>Page Count</rdfs:label>
		<rdfs:comment>Identifies the number of pages in the represented publication.</rdfs:comment>
	</owl:AnnotationProperty>
	<owl:DatatypeProperty rdf:ID="palletBlocks">
		<rdfs:label>Pallet Blocks</rdfs:label>
		<rdfs:comment>Indicates the number of master packs which can be assembled in a single layer on a single pallet.</rdfs:comment>
		<rdfs:range rdf:resource="xsd#float"/>
	</owl:DatatypeProperty>
	<owl:AnnotationProperty rdf:ID="palletGTIN">
		<rdfs:label>Pallet GTIN</rdfs:label>
		<rdfs:comment>The GTIN which identifies a unique pallet which in turn contains unique master pack(s) or case(s).</rdfs:comment>
	</owl:AnnotationProperty>
	<owl:DatatypeProperty rdf:ID="palletHeight">
		<rdfs:label>Pallet Height</rdfs:label>
		<rdfs:comment>Indicates the height of a pallet in real numbers.</rdfs:comment>
		<av7:userNotes>If this attribute obtains a value, 'Pallet Height UOM' must also obtain a value.</av7:userNotes>
		<rdfs:range rdf:resource="xsd#float"/>
	</owl:DatatypeProperty>
	<owl:ObjectProperty rdf:ID="palletHeightUOM">
		<rdfs:label>Pallet Height UOM</rdfs:label>
		<rdfs:comment>Describes the value of 'Pallet Height.'</rdfs:comment>
		<av7:userNotes>If this attribute obtains a value, 'Pallet Height' must also obtain a value.</av7:userNotes>
		<rdfs:range rdf:resource="av7#SpatialUOM"/>
	</owl:ObjectProperty>
	<owl:DatatypeProperty rdf:ID="palletLength">
		<rdfs:label>Pallet Length</rdfs:label>
		<rdfs:comment>Indicates the length of a pallet in real numbers.</rdfs:comment>
		<av7:userNotes>If this attribute obtains a value, 'Pallet Length UOM' must also obtain a value.</av7:userNotes>
		<rdfs:range rdf:resource="xsd#float"/>
	</owl:DatatypeProperty>
	<owl:ObjectProperty rdf:ID="palletLengthUOM">
		<rdfs:label>Pallet Length UOM</rdfs:label>
		<rdfs:comment>Describes the value of 'Pallet Length.'</rdfs:comment>
		<av7:userNotes>If this attribute obtains a value, 'Pallet Length' must also obtain a value.</av7:userNotes>
		<rdfs:range rdf:resource="av7#SpatialUOM"/>
	</owl:ObjectProperty>
	<owl:DatatypeProperty rdf:ID="palletTiers">
		<rdfs:label>Pallet Tiers</rdfs:label>
		<rdfs:comment>Indicates the number of layers that may be stacked on a pallet.</rdfs:comment>
		<rdfs:range rdf:resource="xsd#integer"/>
	</owl:DatatypeProperty>
	<owl:DatatypeProperty rdf:ID="palletWidth">
		<rdfs:label>Pallet Width</rdfs:label>
		<rdfs:comment>Indicates the width of a pallet in real numbers.</rdfs:comment>
		<av7:userNotes>If this attribute obtains a value, 'Pallet Width UOM' must also obtain a value.</av7:userNotes>
		<rdfs:range rdf:resource="xsd#float"/>
	</owl:DatatypeProperty>
	<owl:ObjectProperty rdf:ID="palletWidthUOM">
		<rdfs:label>Pallet Width UOM</rdfs:label>
		<rdfs:comment>Describes the value of 'Pallet Width.'</rdfs:comment>
		<av7:userNotes>If this attribute obtains a value, 'Pallet Width' must also obtain a value.</av7:userNotes>
		<rdfs:range rdf:resource="av7#SpatialUOM"/>
	</owl:ObjectProperty>
	<owl:DatatypeProperty rdf:ID="palletWeight">
		<rdfs:label>Pallet Weight</rdfs:label>
		<rdfs:comment>Indicates the weight of a pallet in real numbers.</rdfs:comment>
		<av7:userNotes>If this attribute obtains a value, 'Pallet Weight UOM' must also obtain a value.</av7:userNotes>
		<rdfs:range rdf:resource="xsd#float"/>
	</owl:DatatypeProperty>
	<owl:ObjectProperty rdf:ID="palletWeightUOM">
		<rdfs:label>Pallet Weight UOM</rdfs:label>
		<rdfs:comment>Describes the value of 'Pallet Weight.' If this attribute obtains a value, 'Pallet Weight' must also obtain a value.</rdfs:comment>
		<rdfs:range rdf:resource="av7#PackWeightUOM"/>
	</owl:ObjectProperty>
	<owl:AnnotationProperty rdf:ID="pantLegStyle">
		<rdfs:label>Pant Leg Style</rdfs:label>
		<rdfs:comment>Describes the type or shape of trousers, pants, or shorts being represented.</rdfs:comment>
	</owl:AnnotationProperty>
	<owl:AnnotationProperty rdf:ID="pantStyle">
		<rdfs:label>Pant Style</rdfs:label>
		<rdfs:comment>Describes the type or shape of trousers, pants, or shorts being represented.</rdfs:comment>
	</owl:AnnotationProperty>
	<owl:DatatypeProperty rdf:ID="pantInseamLength">
		<rdfs:label>Pant/Inseam Length</rdfs:label>
		<rdfs:comment>Measures an inseam.</rdfs:comment>
		<spsis:userNotes>If this attribute obtains a value, 'Pant/Inseam Length UOM' must also obtain a value.</spsis:userNotes>
		<rdfs:range rdf:resource="xsd#float"/>
	</owl:DatatypeProperty>
	<owl:ObjectProperty rdf:ID="pantInseamLengthUOM">
		<rdfs:label>Pant/Inseam Length UOM</rdfs:label>
		<rdfs:comment>Qualifies the value of 'Pant/Inseam Length'.</rdfs:comment>
		<av7:userNotes>If this attribute obtains a value, 'Pant/Inseam Length' must also obtain a value.</av7:userNotes>
		<rdfs:range rdf:resource="av7#SpatialUOM"/>
	</owl:ObjectProperty>
	<owl:DatatypeProperty rdf:ID="parentalAdvisoryLabel">
		<rdfs:label>Parental Advisory Label</rdfs:label>
		<rdfs:comment>Indicates whether or not the represented item has been labled with a Parental Advisory Label.</rdfs:comment>
		<rdfs:range rdf:resource="xsd#boolean"/>
	</owl:DatatypeProperty>
	<owl:DatatypeProperty rdf:ID="partialPackAllowed">
		<rdfs:subPropertyOf rdf:resource="av7#partialPack"/>
		<rdfs:label>Partial Pack Allowed</rdfs:label>
		<rdfs:comment>Indicates whether or not hte represented item may be purchased in less than full packaging.</rdfs:comment>
		<rdfs:range rdf:resource="xsd#boolean"/>
	</owl:DatatypeProperty>
	<owl:DatatypeProperty rdf:ID="partialPackQty">
		<rdfs:subPropertyOf rdf:resource="av7#partialPack"/>
		<rdfs:label>Partial Pack Quantity</rdfs:label>
		<rdfs:comment>Indicates the partial pack quantity orderable at one time.</rdfs:comment>
		<av7:userNotes>If this attribute obtains a value, 'Partial Pack Quantity UOM' must also obtain a value.</av7:userNotes>
		<rdfs:range rdf:resource="xsd#integer"/>
	</owl:DatatypeProperty>
	<owl:ObjectProperty rdf:ID="partialPackQtyUOM">
		<rdfs:subPropertyOf rdf:resource="av7#partialPack"/>
		<rdfs:label>Partial Pack Quantity UOM</rdfs:label>
		<rdfs:comment>Qualifies the value of 'Partial Pack Quantity'.</rdfs:comment>
		<av7:userNotes>If this attribute obtains a value, 'Partial Pack Quantity' must also obtain a value.</av7:userNotes>
		<rdfs:range rdf:resource="av7#PackType"/>
	</owl:ObjectProperty>
	<owl:DatatypeProperty rdf:ID="partsAvailable">
		<rdfs:label>Parts Available</rdfs:label>
		<rdfs:comment>Indicates whether or not there are replacement or other duplicative parts available for use with a represented item.</rdfs:comment>
		<rdfs:range rdf:resource="xsd#boolean"/>
	</owl:DatatypeProperty>
	<owl:AnnotationProperty rdf:ID="pattern">
		<rdfs:label>Pattern</rdfs:label>
		<rdfs:comment>Describes the surface pattern of any item; may be 2 or 3 dimensional.</rdfs:comment>
	</owl:AnnotationProperty>
	<owl:DatatypeProperty rdf:ID="pesticide">
		<rdfs:label>Pesticide</rdfs:label>
		<rdfs:comment>Indicates whether or not the represented item is a pesticide.</rdfs:comment>
		<rdfs:range rdf:resource="xsd#boolean"/>
	</owl:DatatypeProperty>
	<owl:DatatypeProperty rdf:ID="pieces">
		<rdfs:label>Pieces</rdfs:label>
		<rdfs:comment>Indicates the number of pieces included with the represented item, or how many pieces the represented item comprises.</rdfs:comment>
		<rdfs:range rdf:resource="xsd#integer"/>
	</owl:DatatypeProperty>
	<owl:DatatypeProperty rdf:ID="platformSoleHeight">
		<rdfs:label>Platform Sole Height</rdfs:label>
		<rdfs:comment>Measurese the height of a platform from the bottom of the sole to the bottom of the insole in an article of footwear.</rdfs:comment>
		<wmlo:userNotes>If this attribute obtains a value, 'Heel Height/Platform Sole Height UOM' must also obtain a value.</wmlo:userNotes>
		<rdfs:range rdf:resource="xsd#float"/>
	</owl:DatatypeProperty>
	<owl:AnnotationProperty rdf:ID="playerStance">
		<rdfs:label>Player Stance</rdfs:label>
		<rdfs:comment>Indicates the stance of the player for which the represented item is intended or associated.</rdfs:comment>
	</owl:AnnotationProperty>
	<owl:DatatypeProperty rdf:ID="plies">
		<rdfs:label>Plies</rdfs:label>
		<rdfs:comment>Indicates the number of layers of which a represented item is comprised.</rdfs:comment>
		<rdfs:range rdf:resource="xsd#integer"/>
	</owl:DatatypeProperty>
	<owl:AnnotationProperty rdf:ID="posRegisterDescription">
		<rdfs:label>POS/Register Description</rdfs:label>
		<rdfs:comment>Constitutes an abbreviated description of a represented item.</rdfs:comment>
		<av7:userNotes>Intended for printing on shelf tags and register receipts.</av7:userNotes>
	</owl:AnnotationProperty>
	<owl:AnnotationProperty rdf:ID="potencyStrength">
		<rdfs:label>Potency/Strength</rdfs:label>
		<rdfs:comment>Indicates the amount of the represented item wanted to produced an advertised effect.</rdfs:comment>
		<av7:userNotes>When this attributes describes drugs, the value of this attribute may indicate how many tablets or milligrams are necessary to relieve pain or lower blood pressure.</av7:userNotes>
	</owl:AnnotationProperty>
	<owl:AnnotationProperty rdf:ID="powerType">
		<rdfs:label>Power Type</rdfs:label>
		<rdfs:comment>Indicates the type of power or fuel used by the represented item.</rdfs:comment>
	</owl:AnnotationProperty>
	<owl:DatatypeProperty rdf:ID="prescriptionAvailable">
		<rdfs:label>Prescription Available</rdfs:label>
		<rdfs:comment>Indicates whether or not the represented item is available by prescription.</rdfs:comment>
		<rdfs:range rdf:resource="xsd#boolean"/>
	</owl:DatatypeProperty>
	<owl:DatatypeProperty rdf:ID="priceAmount">
		<rdfs:label>Resource</rdfs:label>
		<rdfs:comment>Indicates the represented item's price in real numbers.</rdfs:comment>
		<av7:userNotes>If this attribute obtains a value, 'Price Unit Of Measure' must also obtain a value.</av7:userNotes>
		<rdfs:range rdf:resource="xsd#float"/>
	</owl:DatatypeProperty>
	<owl:DatatypeProperty rdf:ID="priceEffectiveDate">
		<rdfs:label>Resource</rdfs:label>
		<rdfs:comment>Indicates the date on which the represented item's price goes into effect.</rdfs:comment>
		<av7:userNotes>Format varies by upload and explort method. UI and spreadsheet: mm/dd/yyyy; RSX: yyyy-mm-dd.</av7:userNotes>
		<rdfs:range rdf:resource="av7#VariableDate"/>
	</owl:DatatypeProperty>
	<owl:DatatypeProperty rdf:ID="priceExpirationDate">
		<rdfs:label>Resource</rdfs:label>
		<rdfs:comment>Indicates the date on which the represented item's price expires or ceases to be in effect.</rdfs:comment>
		<av7:userNotes>Format varies by upload and explort method. UI and spreadsheet: mm/dd/yyyy; RSX: yyyy-mm-dd.</av7:userNotes>
		<rdfs:range rdf:resource="av7#VariableDate"/>
	</owl:DatatypeProperty>
	<owl:ObjectProperty rdf:ID="priceQualifier">
		<rdfs:label>Resource</rdfs:label>
		<rdfs:comment>Identifies the price type, or the supply chain destination, of the price being represented.</rdfs:comment>
		<rdfs:range rdf:resource="av7#PriceQualifier"/>
	</owl:ObjectProperty>
	<owl:AnnotationProperty rdf:ID="priceSheetNameNumber">
		<rdfs:label>Resource</rdfs:label>
		<rdfs:comment>Indicates the name or number of the price sheet on which a represented item is listed or which references that item.</rdfs:comment>
	</owl:AnnotationProperty>
	<owl:AnnotationProperty rdf:ID="priceTradingPartnerNumber">
		<rdfs:label>Resource</rdfs:label>
		<rdfs:comment>The value of this attribute is a trading partner-specific identifier assigned by SPS Commerce.</rdfs:comment>
		<av7:userNotes>This attribute may only obtain a value when the value of 'Price Qualifier' obtains 'UCP'.</av7:userNotes>
	</owl:AnnotationProperty>
	<owl:ObjectProperty rdf:ID="priceUnitOfMeasure">
		<rdfs:label>Resource</rdfs:label>
		<rdfs:comment>Qualifies the value of 'Price Amount.'.</rdfs:comment>
		<av7:userNotes>If this attribute obtains a value, 'Price Amount' must also obtain a value.</av7:userNotes>
		<rdfs:range rdf:resource="av7#PriceUOM"/>
	</owl:ObjectProperty>
	<owl:ObjectProperty rdf:ID="printingColorCapacity">
		<rdfs:label>Printing Color Capacity</rdfs:label>
		<rdfs:comment>Identifies whether the represented item supports color or monochrome output; assume that items that support color also support monochrome.</rdfs:comment>
	</owl:ObjectProperty>
	<owl:AnnotationProperty rdf:ID="printingTechnology">
		<rdfs:label>Printing Technology</rdfs:label>
		<rdfs:comment>Indicates the technology that the represented item uses in order to print.</rdfs:comment>
	</owl:AnnotationProperty>
	<owl:AnnotationProperty rdf:ID="prismType">
		<rdfs:label>Prism Type</rdfs:label>
		<rdfs:comment>Indicates the type of prism that is used by the represented item.</rdfs:comment>
	</owl:AnnotationProperty>
	<owl:DatatypeProperty rdf:ID="privateLabel">
		<rdfs:label>Private Label</rdfs:label>
		<rdfs:comment>Indicates whether or not the item is private label.</rdfs:comment>
		<rdfs:range rdf:resource="xsd#boolean"/>
	</owl:DatatypeProperty>
	<owl:AnnotationProperty rdf:ID="processorCore">
		<rdfs:label>Processor Core</rdfs:label>
		<rdfs:comment>Indiactes the number of cores that comprise the represented processor.</rdfs:comment>
	</owl:AnnotationProperty>
	<owl:AnnotationProperty rdf:ID="processorManufacturer">
		<rdfs:label>Processor Manufacturer</rdfs:label>
		<rdfs:comment>Names the manufacturer of the represented processer, alone or onboard another item.</rdfs:comment>
	</owl:AnnotationProperty>
	<owl:AnnotationProperty rdf:ID="processorModel">
		<rdfs:label>Processor Model</rdfs:label>
		<rdfs:comment>Names the model number of the represented processor, alone or onboard another item.</rdfs:comment>
	</owl:AnnotationProperty>
	<owl:DatatypeProperty rdf:ID="processorSpeed">
		<rdfs:label>Processor Speed</rdfs:label>
		<rdfs:comment>Measures the maximum number of calculations per second which the represented processor can perform.</rdfs:comment>
		<wmlo:userNotes>If this attribute obtains a value, 'Processor Speed UOM' must obtain a value.</wmlo:userNotes>
		<rdfs:range rdf:resource="xsd#float"/>
	</owl:DatatypeProperty>
	<owl:ObjectProperty rdf:ID="processorSpeedUOM">
		<rdfs:label>Processor Speed UOM</rdfs:label>
		<rdfs:comment>Qualifies the value of 'Processor Speed.'</rdfs:comment>
		<wmlo:userNotes>If this attribute obtains a value, 'Processor Speed' must obtain a value.</wmlo:userNotes>
		<rdfs:range rdf:resource="av7#ProcessorSpeedUOM"/>
	</owl:ObjectProperty>
	<owl:AnnotationProperty rdf:ID="processorType">
		<rdfs:label>Processor Type</rdfs:label>
		<rdfs:comment>Indiactes the kind of sub-brand of the represented processor.</rdfs:comment>
	</owl:AnnotationProperty>
	<owl:AnnotationProperty rdf:ID="productColorCode">
		<rdfs:label>Product Color Code</rdfs:label>
		<rdfs:comment>Identifies item color exclusively of NRF code.</rdfs:comment>
	</owl:AnnotationProperty>
	<owl:AnnotationProperty rdf:ID="productColorDescription">
		<rdfs:label>Product Color Description</rdfs:label>
		<rdfs:comment>Describes product color in natural language.</rdfs:comment>
	</owl:AnnotationProperty>
	<owl:AnnotationProperty rdf:ID="productCode">
		<rdfs:label>Product Code</rdfs:label>
		<rdfs:comment>Indicates a vendor-created item sub-category identifier.</rdfs:comment>
		<av7:userNotes>Assortment requires that this attribute obtain a value in order to validate.</av7:userNotes>
	</owl:AnnotationProperty>
	<owl:AnnotationProperty rdf:ID="productCodeDescription">
		<rdfs:label>Product Code Description</rdfs:label>
		<rdfs:comment>Indicates a brief, descriptive, vendor-created product sub-name.</rdfs:comment>
		<av7:userNotes>It is highly recommended that this attribute obtain a value in order to contextualize 'Product Code'.</av7:userNotes>
	</owl:AnnotationProperty>
	<owl:AnnotationProperty rdf:ID="productFormat">
		<rdfs:label>Product Format</rdfs:label>
		<rdfs:comment>Identifies means by which a media product is delivered to the consumer.</rdfs:comment>
	</owl:AnnotationProperty>
	<owl:DatatypeProperty rdf:ID="productLotNumberMarked">
		<rdfs:label>Product Lot Number Marked</rdfs:label>
		<rdfs:comment>Identifies whether or not the represented item is marked with a lot number.</rdfs:comment>
		<rdfs:range rdf:resource="xsd#boolean"/>
	</owl:DatatypeProperty>
	<owl:AnnotationProperty rdf:ID="productMaterialCode">
		<rdfs:label>Product Material Code</rdfs:label>
		<rdfs:comment>Identifies materials of which a represented item is composed using trading-partner-identified codes.</rdfs:comment>
	</owl:AnnotationProperty>
	<owl:AnnotationProperty rdf:ID="productMaterialDescription">
		<rdfs:label>Product Material Description</rdfs:label>
		<rdfs:comment>Briefly describes the materials of which a product is composed; may include percentages.</rdfs:comment>
	</owl:AnnotationProperty>
	<owl:AnnotationProperty rdf:ID="productSizeCode">
		<rdfs:label>Product Size Code</rdfs:label>
		<rdfs:comment>Identifies item size exclusively of NRF code.</rdfs:comment>
	</owl:AnnotationProperty>
	<owl:AnnotationProperty rdf:ID="productSizeDescription">
		<rdfs:label>Product Size Description</rdfs:label>
		<rdfs:comment>Briefly describes item size exclusively of NRF code.</rdfs:comment>
	</owl:AnnotationProperty>
	<owl:AnnotationProperty rdf:ID="productType">
		<rdfs:label>Product Type</rdfs:label>
		<rdfs:comment>These properties provide a sense of aboutness which can be used to describe a represented item; product types link market segments with use value.</rdfs:comment>
		<rdfs:range rdf:resource="av7p#ProductType"/>
	</owl:AnnotationProperty>
	<owl:AnnotationProperty rdf:ID="projectorThrowRatio">
		<rdfs:label>Projector Throw Ratio</rdfs:label>
		<rdfs:comment>Indicates the throw ratio of the represented projector, measured as the distance from the lens to the screen dividded by the width of the projected image.</rdfs:comment>
	</owl:AnnotationProperty>
	<owl:AnnotationProperty rdf:ID="properShippingName">
		<rdfs:label>Proper Shipping Name</rdfs:label>
		<rdfs:comment>Identifies the dangerous good on the outside of the represented package as defined by the US Department of Transportation.</rdfs:comment>
		<sorg:relatedLink rdf:resource="http://www.hazmattool.com/info.php"/>
	</owl:AnnotationProperty>
	<owl:DatatypeProperty rdf:ID="propSixtyFiveWarning">
		<rdfs:label>Prop 65 Warning</rdfs:label>
		<rdfs:comment>Indicates whether or not the represented item requires a Proposition 65 warning.</rdfs:comment>
		<sorg:relatedLink rdf:resource="http://oehha.ca.gov/proposition-65"/>
		<rdfs:range rdf:resource="xsd#boolean"/>
	</owl:DatatypeProperty>
	<owl:AnnotationProperty rdf:ID="publisher">
		<rdfs:label>Publisher</rdfs:label>
		<rdfs:comment>Names the publisher of the represented publication.</rdfs:comment>
	</owl:AnnotationProperty>
	<owl:DatatypeProperty rdf:ID="pupillaryDistance">
		<rdfs:label>Pupillary Distance</rdfs:label>
		<rdfs:comment>Measures the distance between the centers of the pupils in each eye, in millimeters.</rdfs:comment>
		<rdfs:range rdf:resource="xsd#float"/>
	</owl:DatatypeProperty>
	<owl:ObjectProperty rdf:ID="qtyCode">
		<rdfs:label>Quantity Code</rdfs:label>
		<rdfs:comment>Identifies quantity according to the following set.</rdfs:comment>
		<rdfs:range rdf:resource="av7#PackType"/>
	</owl:ObjectProperty>
	<owl:DatatypeProperty rdf:ID="qtyOnHandByLocation">
		<rdfs:label>Quantity On Hand By Location</rdfs:label>
		<rdfs:comment>Indicates the total quantity of represented items available to order by location.</rdfs:comment>
		<rdfs:range rdf:resource="xsd#integer"/>
	</owl:DatatypeProperty>
	<owl:DatatypeProperty rdf:ID="qtyOnHandTotal">
		<rdfs:label>Quantity On Hand Total</rdfs:label>
		<rdfs:comment>Indicates the total inventory item quantity available to order.</rdfs:comment>
		<rdfs:range rdf:resource="xsd#integer"/>
	</owl:DatatypeProperty>
	<owl:AnnotationProperty rdf:ID="ramMemory">
		<rdfs:subPropertyOf rdf:resource="av7#memory"/>
		<rdfs:label>RAM Memory</rdfs:label>
		<rdfs:comment>Indicates the amount of random access memory (RAM) onboard the represented item.</rdfs:comment>
		<av7:userNotes>The value of this attribute should be a real number plus a unit of measure, e.g. 250 MB; 8 GB.</av7:userNotes>
		<rdfs:range>
			<owl:equivalentClass>
				<owl:complimentOf rdf:resource="xsd#boolean"/>
			</owl:equivalentClass>
		</rdfs:range>
	</owl:AnnotationProperty>
	<owl:DatatypeProperty rdf:ID="rangeMaximum">
		<rdfs:label>Range Maximum</rdfs:label>
		<rdfs:comment>Indicates the maximum distance or extent to which a represented item is rated by its manufacturer to function as intended under ideal conditions. For example, in automobiles the value of this attribute might be measured in the number of miles it can drive before refuelling, in optics the value of this attribute might be measured as the extent in meters to which a scope is able to acquire a target.</rdfs:comment>
		<wmlo:userNotes>If this attribute obtains a value, 'Range UOM' must obtain a value.</wmlo:userNotes>
		<rdfs:range rdf:resource="xsd#float"/>
	</owl:DatatypeProperty>
	<owl:DatatypeProperty rdf:ID="rangeMinimum">
		<rdfs:label>Range Maximum</rdfs:label>
		<rdfs:comment>Indicates the minimum distance or extent to which a represented item is rated by its manufacturer to function as intended under ideal conditions. For example, in optics the value of this attribute might be measured as the minimal extent in meters at which a binoculars is able to acquire a target.</rdfs:comment>
		<wmlo:userNotes>If this attribute obtains a value, 'Range UOM' must obtain a value.</wmlo:userNotes>
		<rdfs:range rdf:resource="xsd#float"/>
	</owl:DatatypeProperty>
	<owl:ObjectProperty rdf:ID="rangeUOM">
		<rdfs:label>Range UOM</rdfs:label>
		<rdfs:comment>Indicates units of measure which describe the values of 'Range Maximum' and 'Range Minimum.'</rdfs:comment>
		<wmlo:userNotes>If this attribute obtains a value, either ''Range Maximum,' 'Range Minimum,' or both must obtain values</wmlo:userNotes>
		<rdfs:range rdf:resource="av7#SpatialUOM"/>
	</owl:ObjectProperty>
	<owl:DatatypeProperty rdf:ID="rechargeable">
		<rdfs:label>Rechargeable</rdfs:label>
		<rdfs:comment>Indicates whether or not the represented item is rechargeable or whether it contains batteries which are rechargeable.</rdfs:comment>
		<rdfs:range rdf:resource="xsd#boolean"/>
	</owl:DatatypeProperty>
	<owl:AnnotationProperty rdf:ID="recommendedUsageLocation">
		<rdfs:label>Recommended Usage Location</rdfs:label>
		<rdfs:comment>Indicates the physical environment in which an item is designed to be used.</rdfs:comment>
	</owl:AnnotationProperty>
	<owl:DatatypeProperty rdf:ID="recyclableItem">
		<rdfs:label>Recyclable Item</rdfs:label>
		<rdfs:comment>Indicates whether or not the represented item is recyclable. Recylability varies by municipality</rdfs:comment>
		<rdfs:range rdf:resource="xsd#boolean"/>
	</owl:DatatypeProperty>
	<owl:DatatypeProperty rdf:ID="recyclablePackaging">
		<rdfs:label>Recyclable Packaging</rdfs:label>
		<rdfs:comment>Indicates whether or not the represented item is packed in recyclable materials. Recylability varies by municipality</rdfs:comment>
		<rdfs:range rdf:resource="xsd#boolean"/>
	</owl:DatatypeProperty>
	<owl:AnnotationProperty rdf:ID="recycledMaterials">
		<rdfs:subPropertyOf rdf:resource="av7#recycling"/>
		<rdfs:label>Recycled Materials</rdfs:label>
		<rdfs:comment>Lists the recycled materials included in the item; may include material percentages.</rdfs:comment>
		<rdfs:range>
			<owl:equivalentClass>
				<owl:complementOf rdf:resource="xsd#boolean"/>
			</owl:equivalentClass>
		</rdfs:range>
	</owl:AnnotationProperty>
	<owl:ObjectProperty rdf:ID="reelType">
		<rdfs:label>Reel Type</rdfs:label>
		<rdfs:comment>Indicates the type of reel associated with the represented item.</rdfs:comment>
	</owl:ObjectProperty>
	<owl:DatatypeProperty rdf:ID="refrigerant">
		<rdfs:label>Refrigerant</rdfs:label>
		<rdfs:comment>Indicates whether or not the represented item contains refrigerant substances or mixtures.</rdfs:comment>
		<rdfs:range rdf:resource="xsd#boolean"/>
	</owl:DatatypeProperty>
	<owl:DatatypeProperty rdf:ID="refrigerantHandlingCertification">
		<rdfs:label>Refrigerant Handling Certification</rdfs:label>
		<rdfs:comment>Indicates whether or not the represented item's purchaser must possess a refrigerant handling certification in order to purchase the item.</rdfs:comment>
		<rdfs:range rdf:resource="xsd#boolean"/>
	</owl:DatatypeProperty>
	<owl:DatatypeProperty rdf:ID="removableInsole">
		<rdfs:label>Removable Insole</rdfs:label>
		<rdfs:comment>Indicates whether or not the represented item has a removable insole.</rdfs:comment>
		<rdfs:range rdf:resource="xsd#boolean"/>
	</owl:DatatypeProperty>
	<owl:DatatypeProperty rdf:ID="remoteControl">
		<rdfs:label>Remote Control</rdfs:label>
		<rdfs:comment>Indicates whether or not a represented item is equipped with a remote control.</rdfs:comment>
		<rdfs:range rdf:resource="xsd#boolean"/>
	</owl:DatatypeProperty>
	<owl:DatatypeProperty rdf:ID="reorderable">
		<rdfs:label>Reorderable</rdfs:label>
		<rdfs:comment>Identifies whether or not an item may be reordered.</rdfs:comment>
		<rdfs:range rdf:resource="xsd#boolean"/>
	</owl:DatatypeProperty>
	<owl:DatatypeProperty rdf:ID="residentialLeadBasedPaintHazardReeuctionAct">
		<rdfs:label>Residential Lead-Based Paint Hazard Reduction Act</rdfs:label>
		<rdfs:comment>Indicates whether or not the represented item is compliant with the Residential Lead-Based Paint Hazard Reduction Act.</rdfs:comment>
		<sorg:relatedLink rdf:resource="https://www.epa.gov/lead/real-estate-disclosure"/>
		<rdfs:range rdf:resource="xsd#boolean"/>
	</owl:DatatypeProperty>
	<owl:DatatypeProperty rdf:ID="resourceConservationRecoveryAct">
		<rdfs:label>Resource Conservation Recovery Act</rdfs:label>
		<rdfs:comment>Indicates whether or not the represented item is compliant with the Resource Conservation Recovery Act.</rdfs:comment>
		<sorg:relatedLink rdf:resource="https://www.epa.gov/compliance/resources-and-guidance-documents-compliance-assistance"/>
		<rdfs:range rdf:resource="xsd#boolean"/>
	</owl:DatatypeProperty>
	<owl:AnnotationProperty rdf:ID="reticle">
		<rdfs:label>Reticle</rdfs:label>
		<rdfs:comment>Indicates the shape of the reticle, or the indicator of where a projectile will land in ideal conditions. With scopes, this may be a dot or a crosshairs; with ironsights, this may be a fork or trident.</rdfs:comment>
	</owl:AnnotationProperty>
	<owl:AnnotationProperty rdf:ID="reticleColor">
		<rdfs:label>Reticle Color</rdfs:label>
		<rdfs:comment>Indicates the color of optical device's reticle.</rdfs:comment>
	</owl:AnnotationProperty>
	<owl:AnnotationProperty rdf:ID="returnCode">
		<rdfs:label>Return Code</rdfs:label>
		<rdfs:comment>Identifies the retailer-to-vendor return policy which pertains to the represented item.</rdfs:comment>
	</owl:AnnotationProperty>
	<owl:AnnotationProperty rdf:ID="returnInstructions">
		<rdfs:label>Return Instructions</rdfs:label>
		<rdfs:comment>Indicates return instructions.</rdfs:comment>
	</owl:AnnotationProperty>
	<owl:DatatypeProperty rdf:ID="reusable">
		<rdfs:label>Reusable</rdfs:label>
		<rdfs:comment>Indicates whether or not the represented item is reusable according to its manufacturer or seller.</rdfs:comment>
		<rdfs:range rdf:resource="xsd#boolean"/>
	</owl:DatatypeProperty>
	<owl:DatatypeProperty rdf:ID="roughInSize">
		<rdfs:label>Rough In Size</rdfs:label>
		<rdfs:comment>Measures rough-in dimensions required to install the represented item.</rdfs:comment>
		<wmlo:userNotes>If this attribute obtains a value, 'Rough In Size UOM' must obtain a value.</wmlo:userNotes>
		<rdfs:range rdf:resource="xsd#float"/>
	</owl:DatatypeProperty>
	<owl:ObjectProperty rdf:ID="roughInSizeUOM">
		<rdfs:label>Rough In Size UOM</rdfs:label>
		<rdfs:comment>Qualifies the value of 'Rough In Size.'</rdfs:comment>
		<wmlo:userNotes>If this attribute obtains a value, 'Rough In SIze' must obtain a value.</wmlo:userNotes>
		<rdfs:range rdf:resource="av7#SpatialUOM"/>
	</owl:ObjectProperty>
	<owl:DatatypeProperty rdf:ID="runFlat">
		<rdfs:label>Run Flat</rdfs:label>
		<rdfs:comment>Indicates whether or not the represented item is a tire or tyre that will run flat or resist the effects of deflation when punctured.</rdfs:comment>
		<rdfs:range rdf:resource="xsd#boolean"/>
	</owl:DatatypeProperty>
	<owl:DatatypeProperty rdf:ID="sVideoInputs">
		<rdfs:label>S Video Inputs</rdfs:label>
		<rdfs:comment>Indicates the number of S Video inputs onboard or supported by a represented item.</rdfs:comment>
		<rdfs:range rdf:resource="xsd#integer"/>
	</owl:DatatypeProperty>
	<owl:DatatypeProperty rdf:ID="sVideoOutputs">
		<rdfs:label>S Video Outputs</rdfs:label>
		<rdfs:comment>Indicates the number of S Video outputs onboard or supported by a represented item.</rdfs:comment>
		<rdfs:range rdf:resource="xsd#integer"/>
	</owl:DatatypeProperty>
	<owl:DatatypeProperty rdf:ID="safeDrinkingWaterAct">
		<rdfs:label>Safe Drinking Water Act</rdfs:label>
		<rdfs:comment>Indicates whether or not the represented item is compliant with the Safe Drinking Water Act.</rdfs:comment>
		<sorg:relatedLink rdf:resource="https://www.epa.gov/compliance/resources-and-guidance-documents-compliance-assistance"/>
		<rdfs:range rdf:resource="xsd#boolean"/>
	</owl:DatatypeProperty>
	<owl:DatatypeProperty rdf:ID="screenSize">
		<rdfs:subPropertyOf rdf:resource="av7#screenDisplay"/>
		<rdfs:label>Screen Size</rdfs:label>
		<rdfs:comment>The size (in inches) of the area where pictures and videos are displayed by a represented item.</rdfs:comment>
		<rdfs:range rdf:resource="xsd#float"/>
	</owl:DatatypeProperty>
	<owl:DatatypeProperty rdf:ID="seasonalAvailability">
		<rdfs:subPropertyOf rdf:resource="av7#seasonality"/>
		<rdfs:label>Seasonal Availability</rdfs:label>
		<rdfs:comment>Identifies whether or not the represented item is available seasonally.</rdfs:comment>
		<rdfs:range rdf:resource="xsd#boolean"/>
	</owl:DatatypeProperty>
	<owl:ObjectProperty rdf:ID="seasonOccasion">
		<rdfs:subPropertyOf rdf:resource="av7#seasonality"/>
		<rdfs:label>Season/Occasion</rdfs:label>
		<rdfs:comment>A descriptive name for a particular season or occasion that somehow pertains to the represented item.</rdfs:comment>
		<rdfs:range>
			<owl:equivalentClass>
				<owl:complementOf rdf:resource="xsd#boolean"/>
			</owl:equivalentClass>
		</rdfs:range>
	</owl:ObjectProperty>
	<owl:AnnotationProperty rdf:ID="selectionCode">
		<rdfs:label>Selection Code</rdfs:label>
		<rdfs:comment>Indicates a vendor-created item category identifier.</rdfs:comment>
		<av7:userNotes>Assortment requires that this attribute obtain a value in order to validate.</av7:userNotes>
	</owl:AnnotationProperty>
	<owl:AnnotationProperty rdf:ID="selectionCodeDescription">
		<rdfs:label>Selection Code Description</rdfs:label>
		<rdfs:comment>Indicates a brief, descriptive, vendor-created product name.</rdfs:comment>
		<av7:userNotes>It is highly recommended that this attribute obtain a value in order to contextualize 'Selection Code'.</av7:userNotes>
	</owl:AnnotationProperty>
	<owl:DatatypeProperty rdf:ID="serialized">
		<rdfs:label>Serialized</rdfs:label>
		<rdfs:comment>Indicates whether or not an item has a unique serial identifier printed on it.</rdfs:comment>
		<rdfs:range rdf:resource="xsd#boolean"/>
	</owl:DatatypeProperty>
	<owl:AnnotationProperty rdf:ID="series">
		<rdfs:label>Series</rdfs:label>
		<rdfs:comment>Names the series to the represented publication belongs.</rdfs:comment>
	</owl:AnnotationProperty>
	<owl:AnnotationProperty rdf:ID="serviceProvider">
		<rdfs:label>Service Provider</rdfs:label>
		<rdfs:comment>Indicates service providers associated by manufacturers or sellers with the represented item.</rdfs:comment>
	</owl:AnnotationProperty>
	<owl:DatatypeProperty rdf:ID="servingsPerContainer">
		<rdfs:label>Servings Per Container</rdfs:label>
		<rdfs:comment>Indicates the number of recommended servings contained in a represented item.</rdfs:comment>
		<rdfs:range rdf:resource="xsd#float"/>
	</owl:DatatypeProperty>
	<owl:DatatypeProperty rdf:ID="servingsPerDay">
		<rdfs:label>Servings Per Day</rdfs:label>
		<rdfs:comment>Indicates the number of times which a recommended item is to be dispensed or served per day.</rdfs:comment>
		<rdfs:range rdf:resource="xsd#float"/>
	</owl:DatatypeProperty>
	<owl:DatatypeProperty rdf:ID="servingsSize">
		<rdfs:label>Servings Size</rdfs:label>
		<rdfs:comment>Indicates the number of units recommended by the manufacturer or seller to measure servings.</rdfs:comment>
		<rdfs:range rdf:resource="xsd#float"/>
	</owl:DatatypeProperty>
	<owl:AnnotationProperty rdf:ID="shaftType">
		<rdfs:subPropertyOf rdf:resource="av7#shaft"/>
		<rdfs:label>Shaft Type</rdfs:label>
		<rdfs:comment>Describes the kind of shaft on the represented item; a shaft constitutes the long, narrow part or section of an item which is usually fixed at each end to another part.</rdfs:comment>
	</owl:AnnotationProperty>
	<owl:DatatypeProperty rdf:ID="shaftWeight">
		<rdfs:subPropertyOf rdf:resource="av7#shaft"/>
		<rdfs:label>Shaft Weight</rdfs:label>
		<rdfs:comment>Indicates the weight of a shaft in grams.</rdfs:comment>
		<rdfs:range rdf:resource="xsd#float"/>
	</owl:DatatypeProperty>
	<owl:AnnotationProperty rdf:ID="shape">
		<rdfs:label>Shape</rdfs:label>
		<rdfs:comment>Describes or indicates the visual or spatial shape of a represented item.</rdfs:comment>
	</owl:AnnotationProperty>
	<owl:DatatypeProperty rdf:ID="shelfLife">
		<rdfs:label>Shelf Life</rdfs:label>
		<rdfs:comment>Indicates the number of days until the represented item expires.</rdfs:comment>
		<rdfs:range rdf:resource="xsd#integer"/>
	</owl:DatatypeProperty>
	<owl:AnnotationProperty rdf:ID="shortMarketingMessage">
		<rdfs:label>Short Marketing Message</rdfs:label>
		<rdfs:comment>Communicates a brief marketing message, description, tagline, or other text associated with the represented item.</rdfs:comment>
		<av7:userNotes>This attribute typically communicates short, consumer-friendly headlines such as brand slogan, product purpose, and e-commerce site quick views.</av7:userNotes>
	</owl:AnnotationProperty>
	<owl:DatatypeProperty rdf:ID="signalBooster">
		<rdfs:label>Signal Booster</rdfs:label>
		<rdfs:comment>Indicates whether or not a represented item has a signal booster.</rdfs:comment>
		<rdfs:range rdf:resource="xsd#boolean"/>
	</owl:DatatypeProperty>
	<owl:AnnotationProperty rdf:ID="skillLevel">
		<rdfs:label>Skill Level</rdfs:label>
		<rdfs:comment>Indicates the suggested skill level for a represented item's user.</rdfs:comment>
	</owl:AnnotationProperty>
	<owl:AnnotationProperty rdf:ID="sleeveLength">
		<rdfs:label>Sleeve Length</rdfs:label>
		<rdfs:comment>Describes the type or shape of sleeve on the represented item.</rdfs:comment>
	</owl:AnnotationProperty>
	<owl:DatatypeProperty rdf:ID="sleeveMeasurement">
		<rdfs:label>Sleeve Measurement</rdfs:label>
		<rdfs:comment>Measures the represented item from the base of its neck to the sleeve's cuff.</rdfs:comment>
		<av7:userNotes>If this attribute obtains a value, 'Sleeve Measurement UOM' must also obtain a value.</av7:userNotes>
		<rdfs:range rdf:resource="xsd#float"/>
	</owl:DatatypeProperty>
	<owl:ObjectProperty rdf:ID="sleeveMeasurementUOM">
		<rdfs:label>Sleeve MeasurementUOM</rdfs:label>
		<rdfs:comment>Qualifies the value of 'Sleeve Measurement'.</rdfs:comment>
		<av7:userNotes>If this attribute obtains a value, 'Sleeve Measurement' must also obtain a value.</av7:userNotes>
		<rdfs:range rdf:resource="av7#SpatialUOM"/>
	</owl:ObjectProperty>
	<owl:DatatypeProperty rdf:ID="takesSmallPackageCarrier">
		<rdfs:subPropertyOf rdf:resource="av7#smallPackageCarrier"/>
		<rdfs:label>Takes Small Package Carrier</rdfs:label>
		<rdfs:comment>Indicates whether or not the item described may be shipped by a small package carrier (e.g. UPS).</rdfs:comment>
		<wmlo:userNotes> If the value of this attribute is 'N,' 'Small Package Carrier Restriction' must also have a value.</wmlo:userNotes>
		<rdfs:range rdf:resource="xsd#boolean"/>
	</owl:DatatypeProperty>
	<owl:AnnotationProperty rdf:ID="smallPackageCarrierRestriction">
		<rdfs:subPropertyOf rdf:resource="av7#smallPackageCarrier"/>
		<rdfs:label>Small Package Carrier Restriction</rdfs:label>
		<rdfs:comment>Identifies why an item may not be shipped via small package carrier..</rdfs:comment>
		<wmlo:userNotes> If this attribute obtains a value, the value of 'Small Package Carrier' must be 'N.'</wmlo:userNotes>
		<rdfs:range>
			<owl:equivalentClass>
				<owl:complmentOf rdf:resource="xsd#boolean"/>
			</owl:equivalentClass>
		</rdfs:range>
	</owl:AnnotationProperty>
	<owl:ObjectProperty rdf:ID="smallPartsWarning">
		<rdfs:label>
			<rdf:List>
				<rdf:first rdf:value="Small Parts Warning"/>
				<rdf:rest rdf:value="Small Parts Warning 2"/>
				<rdf:rest rdf:value="Small Parts Warning 3"/>
			</rdf:List>
		</rdfs:label>
		<rdfs:comment>Indicates what kind of small parts warning a represented item does or might require.</rdfs:comment>
		<rdfs:range rdf:resource="av7#SmallPartsWarning"/>
	</owl:ObjectProperty>
	<owl:AnnotationProperty rdf:ID="sockStyle">
		<rdfs:label>Sock Style</rdfs:label>
		<rdfs:comment>Describes the appearance or kind of the represented sock.</rdfs:comment>
	</owl:AnnotationProperty>
	<owl:DatatypeProperty rdf:ID="socketQty">
		<rdfs:label>Socket Quantity</rdfs:label>
		<rdfs:comment>Indicates the number of sockets pertaining to the represented item.</rdfs:comment>
		<rdfs:range rdf:resource="xsd#integer"/>
	</owl:DatatypeProperty>
	<owl:AnnotationProperty rdf:ID="softwareType">
		<rdfs:label>Software Type</rdfs:label>
		<rdfs:comment>Specifies function or use value of the represented piece of software.</rdfs:comment>
	</owl:AnnotationProperty>
	<owl:AnnotationProperty rdf:ID="soleType">
		<rdfs:label>Sole Type</rdfs:label>
		<rdfs:comment>Specifies the type of material from which the sole of the represented item is made.</rdfs:comment>
	</owl:AnnotationProperty>
	<owl:DatatypeProperty rdf:ID="speakersIntegrated">
		<rdfs:label>Speakers Integrated</rdfs:label>
		<rdfs:comment>Indicates whether or not a represented item has integrated speakers.</rdfs:comment>
		<rdfs:range rdf:resource="xsd#boolean"/>
	</owl:DatatypeProperty>
	<owl:ObjectProperty rdf:ID="specialHandlingCode">
		<rdfs:label>Special Handling Code</rdfs:label>
		<rdfs:comment>Describes the special transportation handling requirements pertaining to to the represented item.</rdfs:comment>
		<rdfs:range rdf:resource="av7#SpecialHandlingCode"/>
	</owl:ObjectProperty>
	<owl:ObjectProperty rdf:ID="specialItemCode">
		<rdfs:label>Special Item Code</rdfs:label>
		<rdfs:comment>Shows how individual items may be distributed when they are not available for consumer sale.</rdfs:comment>
		<rdfs:range rdf:resource="av7#SpecialItemCode"/>
	</owl:ObjectProperty>
	<owl:AnnotationProperty rdf:ID="specialLabelingReason">
		<rdfs:label>Special Labeling Reason</rdfs:label>
		<rdfs:comment>Qualifies the value of 'Special Labeling Requirements'.</rdfs:comment>
	</owl:AnnotationProperty>
	<owl:DatatypeProperty rdf:ID="specialLabelingRequirements">
		<rdfs:label>Special Labeling Requirements</rdfs:label>
		<rdfs:comment>Indicates whether or not the represented item is subject to special labeling requirements.</rdfs:comment>
		<rdfs:range rdf:resource="xsd#boolean"/>
	</owl:DatatypeProperty>
	<owl:AnnotationProperty rdf:ID="specialtyApparel">
		<rdfs:label>Specialty Apparel</rdfs:label>
		<rdfs:comment>Indicates the apparel size category to which the represented item belongs.</rdfs:comment>
	</owl:AnnotationProperty>
	<owl:AnnotationProperty rdf:ID="sport">
		<rdfs:label>Sport</rdfs:label>
		<rdfs:comment>Indicates the sport(s) associated with the represented item.</rdfs:comment>
	</owl:AnnotationProperty>
	<owl:AnnotationProperty rdf:ID="sportsPosition">
		<rdfs:label>Sports Position</rdfs:label>
		<rdfs:comment>Indicates the player position for which the represented item is intended or otherwise associated.</rdfs:comment>
	</owl:AnnotationProperty>
	<owl:DatatypeProperty rdf:ID="spreadRateMaximum">
		<rdf:subPropertyOf rdf:resource="av7#spreadRate"/>
		<rdfs:label>Spread Rate Maximum</rdfs:label>
		<rdfs:comment>Indicates the maximum area that a represented item can cover depending upon application technique and other variables.</rdfs:comment>
		<wmlo:userNotes>If this attribute obtains a value, 'Spread Rate UOM' must obtain a value.</wmlo:userNotes>
		<rdfs:range rdf:resource="xsd#float"/>
	</owl:DatatypeProperty>
	<owl:DatatypeProperty rdf:ID="spreadRateMinimum">
		<rdf:subPropertyOf rdf:resource="av7#spreadRate"/>
		<rdfs:label>Spread Rate Minimum</rdfs:label>
		<rdfs:comment>Indicates the minimum area that a represented item can cover depending upon application technique and other variables.</rdfs:comment>
		<wmlo:userNotes>If this attribute obtains a value, 'Spread Rate UOM' must obtain a value.</wmlo:userNotes>
		<rdfs:range rdf:resource="xsd#float"/>
	</owl:DatatypeProperty>
	<owl:ObjectProperty rdf:ID="spreadRateUOM">
		<rdf:subPropertyOf rdf:resource="av7#spreadRate"/>
		<rdfs:label>Spread Rate UOM</rdfs:label>
		<rdfs:comment>Qualifies the values of 'Spread Rate Maximum' and 'Spread Rate Minimum'.'</rdfs:comment>
		<wmlo:userNotes>If this attribute obtains a value, either 'Spread Rate Maximum,' 'Spread Rate Minimum,' or both must obtain values.</wmlo:userNotes>
		<rdfs:range rdf:resource="av7#SpreadRateUOM"/>
	</owl:ObjectProperty>
	<owl:AnnotationProperty rdf:ID="statesRestricted">
		<rdf:subPropertyOf rdf:resource="av7#usState"/>
		<rdfs:label>States Restricted</rdfs:label>
		<rdfs:comment>Names the states within the USA in which the represented item is restricted from sale.</rdfs:comment>
		<av7:userNotes>Use 2-letter abbreviations.</av7:userNotes>
	</owl:AnnotationProperty>
	<owl:AnnotationProperty rdf:ID="stateRestrictionReasons">
		<rdfs:label>State Restriction Reasons</rdfs:label>
		<rdfs:comment>Describes why an item is restricted for sale in a US state.</rdfs:comment>
		<av7:userNotes>Users should input this value as a 2-letter abbreviation followed by the specific reason for restriction.</av7:userNotes>
	</owl:AnnotationProperty>
	<owl:DatatypeProperty rdf:ID="stateRestrictions">
		<rdf:subPropertyOf rdf:resource="av7#usState"/>
		<rdfs:label>State Restrictions</rdfs:label>
		<rdfs:comment>Identifies whether or not the represented item is prohibited from sale in discrete states in the USA.</rdfs:comment>
		<rdfs:range rdf:resource="xsd#boolean"/>
	</owl:DatatypeProperty>
	<owl:AnnotationProperty rdf:ID="stoneDetails">
		<rdfs:label>Stone Details</rdfs:label>
		<rdfs:comment>Describes the primary gemstone associated with a represented item.</rdfs:comment>
	</owl:AnnotationProperty>
	<owl:AnnotationProperty rdf:ID="strollerType">
		<rdfs:label>strollerType</rdfs:label>
		<rdfs:comment>Indicates the kind of stroller or pram (for babies and small children) being represented.</rdfs:comment>
	</owl:AnnotationProperty>
	<owl:AnnotationProperty rdf:ID="subfloorType">
		<rdfs:label>Subfloor Type</rdfs:label>
		<rdfs:comment>Indicates the type of subfloor over which the represented item should be installed.</rdfs:comment>
	</owl:AnnotationProperty>
	<owl:AnnotationProperty rdf:ID="subject">
		<rdfs:label>Subject</rdfs:label>
		<rdfs:comment>Names the subject, category, or genre pertaining to the represented publication.</rdfs:comment>
	</owl:AnnotationProperty>
	<owl:AnnotationProperty rdf:ID="subtitle">
		<rdfs:label>Subtitle</rdfs:label>
		<rdfs:comment>Names the subtitle or explanatory title of the represented publication.</rdfs:comment>
	</owl:AnnotationProperty>
	<owl:DatatypeProperty rdf:ID="supplementFactsLabelRequired">
		<rdfs:label>Supplement Facts Label Required</rdfs:label>
		<rdfs:comment>Indicates whether or not the represented item requires a supplement facts label.</rdfs:comment>
		<rdfs:range rdf:resource="xsd#boolean"/>
	</owl:DatatypeProperty>
	<owl:AnnotationProperty rdf:ID="surfaceFinish">
		<rdfs:label>Surface Finish</rdfs:label>
		<rdfs:comment>Describes the general appearance of an item's surface; may be exclusive of pattern.</rdfs:comment>
	</owl:AnnotationProperty>
	<owl:AnnotationProperty rdf:ID="swimsuitType">
		<rdfs:label>Swimsuit Type</rdfs:label>
		<rdfs:comment>Describes the style of the represented swimsuit.</rdfs:comment>
	</owl:AnnotationProperty>
	<owl:AnnotationProperty rdf:ID="swingWeight">
		<rdfs:label>Swing Weight</rdfs:label>
		<rdfs:comment>Measures the weight about a fulcrum point on a represented club, which specifies how heavy the club feels to the person swinging it.</rdfs:comment>
		<wmlo:userNotes>Swing weight is usuallyexpressed with a letter (A-G) and a number (0-9).</wmlo:userNotes>
	</owl:AnnotationProperty>
	<owl:AnnotationProperty rdf:ID="systemRequirements">
		<rdfs:label>System Requirements</rdfs:label>
		<rdfs:comment>Describes what a represented system needs in order to function properly.</rdfs:comment>
	</owl:AnnotationProperty>
	<owl:DatatypeProperty rdf:ID="hasVariant">
		<rdfs:subPropertyOf rdf:resource="av7#variant"/>
		<rdfs:label>Has Variant</rdfs:label>
		<rdfs:comment>Indicates whether or not a thing has a variant.</rdfs:comment>
		<rdfs:range rdf:resource="xsd#boolean"/>
	</owl:DatatypeProperty>
	<owl:AnnotationProperty rdf:ID="variantName">
		<rdfs:subPropertyOf rdf:resource="av7#variant"/>
		<rdfs:label>Variant Name</rdfs:label>
		<rdfs:comment>Indicates the name of a variant.</rdfs:comment>
		<rdfs:range>
			<owl:equivalentClass>
				<owl:complementOf rdf:resource="xsd#boolean"/>
			</owl:equivalentClass>
		</rdfs:range>
	</owl:AnnotationProperty>
	<owl:DatatypeProperty rdf:ID="tactical">
		<rdfs:label>Tactical</rdfs:label>
		<rdfs:comment>Indicates whether or not a represented item is considered to be tactical; in other words, suitable for law enforcement or military use.</rdfs:comment>
		<rdfs:range rdf:resource="xsd#boolean"/>
	</owl:DatatypeProperty>
	<owl:DatatypeProperty rdf:ID="tamperResistant">
		<rdfs:label>Tamper Resistant</rdfs:label>
		<rdfs:comment>Indicates whether or not the represented item has tamper-resistant packaging.</rdfs:comment>
		<rdfs:range rdf:resource="xsd#boolean"/>
	</owl:DatatypeProperty>
	<owl:AnnotationProperty rdf:ID="team">
		<rdfs:label>Team</rdfs:label>
		<rdfs:comment>Indicates the specifric sports team(s) associated with the represented item.</rdfs:comment>
	</owl:AnnotationProperty>
	<owl:DatatypeProperty rdf:ID="tearResistant">
		<rdfs:label>Tear Resistant</rdfs:label>
		<rdfs:comment>Indicates whether or not the represented item is tear resistant.</rdfs:comment>
		<rdfs:range rdf:resource="xsd#boolean"/>
	</owl:DatatypeProperty>
	<owl:AnnotationProperty rdf:ID="technologyStorageCapacity">
		<rdfs:label>Technology Storage Capacity</rdfs:label>
		<rdfs:comment>Indicates the amount of storage onboard or associated with a represented electronic device.</rdfs:comment>
		<av7:userNotes>The value of this attribute should be a real number plus a unit of measure.</av7:userNotes>
	</owl:AnnotationProperty>
	<owl:DatatypeProperty rdf:ID="temperatureSensitive">
		<rdfs:label>Temperature Sensitive</rdfs:label>
		<rdfs:comment>Indicates whether or not the represented item is temperature sensitive.</rdfs:comment>
		<rdfs:range rdf:resource="xsd#boolean"/>
	</owl:DatatypeProperty>
	<owl:DatatypeProperty rdf:ID="templeLength">
		<rdfs:label>Temple Length</rdfs:label>
		<rdfs:comment>Measures the length of the temple-part of a eyeglass frame in millimeters.</rdfs:comment>
		<rdfs:range rdf:resource="xsd#float"/>
	</owl:DatatypeProperty>
	<owl:AnnotationProperty rdf:ID="textureFinish">
		<rdfs:label>Texture Finish</rdfs:label>
		<rdfs:comment>Describes the general texture of an item's surface.</rdfs:comment>
	</owl:AnnotationProperty>
	<owl:DatatypeProperty rdf:ID="thermalImaging">
		<rdfs:label>Thermal Imaging</rdfs:label>
		<rdfs:comment>Indicates whether or not a represented item is equipped with thermal imaging (heat-detecting) capabilities.</rdfs:comment>
		<rdfs:range rdf:resource="xsd#boolean"/>
	</owl:DatatypeProperty>
	<owl:AnnotationProperty rdf:ID="thirdPartyLogo">
		<rdfs:label>3rd Party Logo</rdfs:label>
		<rdfs:comment>Indicates or describes a distinctive design, name, or symbol that is shown on the item. Exclusive of brand, league, or team logo.</rdfs:comment>
	</owl:AnnotationProperty>
	<owl:DatatypeProperty rdf:ID="thumbnail">
		<rdfs:label>Resource</rdfs:label>
		<rdfs:comment>Indicates whether or not the represented digital asset is a thumbnail image.</rdfs:comment>
		<rdfs:range rdf:resource="xsd#boolean"/>
	</owl:DatatypeProperty>
	<owl:DatatypeProperty rdf:ID="tireLoadIndex">
		<rdfs:label>Tire Load Index</rdfs:label>
		<rdfs:comment>References the load-carrying capacity of the tire being represented.</rdfs:comment>
		<sorg:relatedLink rdf:resource="https://en.wikipedia.org/wiki/Tire_code#Load_index"/>
		<rdfs:range rdf:resource="xsd#integer"/>
	</owl:DatatypeProperty>
	<owl:AnnotationProperty rdf:ID="tireSize">
		<rdfs:label>Tire Size</rdfs:label>
		<rdfs:comment>Indicates the size of a represented tire.</rdfs:comment>
		<av7:userNotes>Usually begins with a letter which indicates the type of vehicle for which the tire in question is intended; usually manifests on the sides of tires.</av7:userNotes>
		<sorg:relatedLink rdf:resource="https://en.wikipedia.org/wiki/Tire_code#Tire_geometry"/>
	</owl:AnnotationProperty>
	<owl:AnnotationProperty rdf:ID="tireSpeedRating">
		<rdfs:label>Tire Speed Rating</rdfs:label>
		<rdfs:comment>Indicates the maximum speed capability of the represented tire.</rdfs:comment>
		<av7:userNotes>Usually manifests on the sides of tires with the value of 'Tire Size'.</av7:userNotes>
		<sorg:relatedLink rdf:resource="https://en.wikipedia.org/wiki/Tire_code#Speed_rating"/>
	</owl:AnnotationProperty>
	<owl:AnnotationProperty rdf:ID="tireTreadwearGrade">
		<rdfs:label>Tire Treadwear Grade</rdfs:label>
		<rdfs:comment>Indicates a comparative measure of durability for tire treads.</rdfs:comment>
		<sorg:relatedLink rdf:resource="https://en.wikipedia.org/wiki/Uniform_Tire_Quality_Grading#Treadwear"/>
	</owl:AnnotationProperty>
	<owl:AnnotationProperty rdf:ID="title">
		<rdfs:label>Title</rdfs:label>
		<rdfs:comment>Names the title of the represented publication.</rdfs:comment>
	</owl:AnnotationProperty>
	<owl:AnnotationProperty rdf:ID="toeProtection">
		<rdfs:label>Toe Protection</rdfs:label>
		<rdfs:comment>Describes the kind of barrier or guard which protects the wearer from toe injury while wearing the represented item.</rdfs:comment>
	</owl:AnnotationProperty>
	<owl:AnnotationProperty rdf:ID="toeType">
		<rdfs:label>Toe Type</rdfs:label>
		<rdfs:comment>Indicates the style of toe pertaining to the represented item.</rdfs:comment>
	</owl:AnnotationProperty>
	<owl:DatatypeProperty rdf:ID="torque">
		<rdfs:label>Torque</rdfs:label>
		<rdfs:comment>Measures the twist resistance belonging to a represented club in degrees.</rdfs:comment>
		<rdfs:range rdf:resource="xsd#float"/>
	</owl:DatatypeProperty>
	<owl:DatatypeProperty rdf:ID="toxicSubstancesControlAct">
		<rdfs:label>Toxic Substances Control Act</rdfs:label>
		<rdfs:comment>Indicates whether or not the represented item is compliant with the Toxic Substances Control Act.</rdfs:comment>
		<sorg:relatedLink rdf:resource="https://www.epa.gov/compliance/resources-and-guidance-documents-compliance-assistance"/>
		<rdfs:range rdf:resource="xsd#boolean"/>
	</owl:DatatypeProperty>
	<owl:AnnotationProperty rdf:ID="tradeMarkServicemark">
		<rdfs:label>Trade Mark/Servicemark</rdfs:label>
		<rdfs:comment>A word, phrase, symbol, or design, or a combination thereof, that identifies and distinguishes the source of the goods of one party from those of others. A servicemark is the same as a trademark except that it identifies and distinguishes the source of a service rather than of goods.</rdfs:comment>
	</owl:AnnotationProperty>
	<owl:AnnotationProperty rdf:ID="tradeName">
		<rdfs:label>Trade Name</rdfs:label>
		<rdfs:comment>The official or legal name under which a company does business. It may also be known as a 'doing business as' (DBA) name.</rdfs:comment>
	</owl:AnnotationProperty>
	<owl:AnnotationProperty rdf:ID="trowelConfiguration">
		<rdfs:label>Trowel Configuration</rdfs:label>
		<rdfs:comment>Describes the type of trowel that should be used to install the recommended item, or describes the trowel itself if the trowel is the represented item.'</rdfs:comment>
	</owl:AnnotationProperty>
	<owl:AnnotationProperty rdf:ID="turretStyle">
		<rdfs:label>Turret Style</rdfs:label>
		<rdfs:comment>Indicates the style of turret on a represented item; developed for (but not limited to) optical devices.</rdfs:comment>
	</owl:AnnotationProperty>
	<owl:AnnotationProperty rdf:ID="tvRating">
		<rdfs:label>TV Rating</rdfs:label>
		<rdfs:comment>Indicates how the TV Parental Guidelines Rating body rates a represented item.</rdfs:comment>
	</owl:AnnotationProperty>
	<owl:AnnotationProperty rdf:ID="unNaNumber">
		<rdfs:label>UN/NA Number</rdfs:label>
		<rdfs:comment>The number used to identify hazardous chemicals or classes of chemicals for international transport as defined by the UN or by the USA Department of Transportation.</rdfs:comment>
		<sorg:relatedLink rdf:resource="http://www.hazmattool.com/info.php"/>
	</owl:AnnotationProperty>
	<owl:AnnotationProperty rdf:ID="upc">
		<rdfs:label>UPC</rdfs:label>
		<rdfs:comment>Universal Product Code (UPC) a.k.a. GTIN 12. Maintained and defined by GS1.</rdfs:comment>
		<sorg:relatedLink rdf:resource="http://www.gs1.org/resources/standards"/>
	</owl:AnnotationProperty>
	<owl:DatatypeProperty rdf:ID="usagePerDay">
		<rdfs:label>Usage Per Day</rdfs:label>
		<rdfs:comment>The average energy consumption of a represented item per day.</rdfs:comment>
		<av7:userNotes>If this attribute obtains a value, 'Usage Per Day UOM' must also obtain a value.</av7:userNotes>
		<rdfs:range rdf:resource="xsd#float"/>
	</owl:DatatypeProperty>
	<owl:ObjectProperty rdf:ID="usagePerDayUOM">
		<rdfs:label>Usage Per Day UOM</rdfs:label>
		<rdfs:comment>Qualifies the value of 'Usage Per Day'.</rdfs:comment>
		<av7:userNotes>If this attribute obtains a value, 'Usage Per Day' must also obtain a value.</av7:userNotes>
		<rdfs:range rdf:resource="av7#UsagePerTimeUOM"/>
	</owl:ObjectProperty>
	<owl:ObjectProperty rdf:ID="usagePerHourUOM">
		<rdfs:label>Usage Per Hour UOM</rdfs:label>
		<rdfs:comment>Qualifies the value of 'Usage Per Hour'.</rdfs:comment>
		<av7:userNotes>If this attribute obtains a value, 'Usage Per Hour' must also obtain a value.</av7:userNotes>
		<rdfs:range rdf:resource="av7#UsagePerTimeUOM"/>
	</owl:ObjectProperty>
	<owl:DatatypeProperty rdf:ID="usagePerHour">
		<rdfs:label>Usage Per Hour</rdfs:label>
		<rdfs:comment>The average energy consumption of a represented item per hour.</rdfs:comment>
		<av7:userNotes>If this attribute obtains a value, 'Usage Per Hour UOM' must also obtain a value.</av7:userNotes>
		<rdfs:range rdf:resource="xsd#float"/>
	</owl:DatatypeProperty>
	<owl:DatatypeProperty rdf:ID="usb">
		<rdfs:label>USB</rdfs:label>
		<rdfs:comment>Indicates the number of USB inputs onboard or supported by a represented item.</rdfs:comment>
		<rdfs:range rdf:resource="xsd#integer"/>
	</owl:DatatypeProperty>
	<owl:AnnotationProperty rdf:ID="vehicleMake">
		<rdfs:label>Vehicle Make</rdfs:label>
		<rdfs:comment>Indicates the make or brand of a represented vehicle.</rdfs:comment>
	</owl:AnnotationProperty>
	<owl:AnnotationProperty rdf:ID="vehicleModel">
		<rdfs:label>Vehicle Model</rdfs:label>
		<rdfs:comment>Indicates the model of a represented vehicle.</rdfs:comment>
	</owl:AnnotationProperty>
	<owl:AnnotationProperty rdf:ID="vehicleType">
		<rdfs:label>Vehicle Type</rdfs:label>
		<rdfs:comment>Indicates the type of the represented vehicle, e.g. car, pickup truck, cargo van.</rdfs:comment>
	</owl:AnnotationProperty>
	<owl:AnnotationProperty rdf:ID="vendorMarketingType">
		<rdfs:label>Vendor Marketing Type</rdfs:label>
		<rdfs:comment>Indicates that a particular type of vendor promotion is associated with the represented item.</rdfs:comment>
	</owl:AnnotationProperty>
	<owl:AnnotationProperty rdf:ID="vendorPartDescription">
		<rdfs:label>Vendor Part Description</rdfs:label>
		<rdfs:comment>Briefly identifies the vendor-identified part being represented.</rdfs:comment>
	</owl:AnnotationProperty>
	<owl:AnnotationProperty rdf:ID="vendorPartNumber">
		<rdfs:label>Vendor Part Number</rdfs:label>
		<rdfs:comment>Indicates the vendor-created number used by vendors to itentify their items.</rdfs:comment>
		<av7:userNotes>'Vendor Part Number' is not a universally governed or recognized item identifier. Therefor it is recommended that attibutes 'UPC', 'GTIN', 'EAN', or 'ISBN' obtain values if 'Vendor Part Number' obtains a value.</av7:userNotes>
	</owl:AnnotationProperty>
	<owl:AnnotationProperty rdf:ID="version">
		<rdfs:label>Version</rdfs:label>
		<rdfs:comment>The generation, iteration, or version of a represented item.</rdfs:comment>
	</owl:AnnotationProperty>
	<owl:AnnotationProperty rdf:ID="videoGamePlatform">
		<rdfs:label>Video Game Platform</rdfs:label>
		<rdfs:comment>Indicates the gaming platform associated with the represented item.</rdfs:comment>
	</owl:AnnotationProperty>
	<owl:DatatypeProperty rdf:ID="voltage">
		<rdfs:label>Voltage</rdfs:label>
		<rdfs:comment>Indicates the maximum voltage associated with the represented item.</rdfs:comment>
		<rdfs:range rdf:resource="xsd#float"/>
	</owl:DatatypeProperty>
	<owl:DatatypeProperty rdf:ID="threeDCapabale">
		<rdfs:label>3D Capable</rdfs:label>
		<rdfs:comment>Indicates whether or not a represented item is capable of displaying in 3D.</rdfs:comment>
		<rdfs:range rdf:resource="xsd#boolean"/>
	</owl:DatatypeProperty>
	<owl:DatatypeProperty rdf:ID="touchscreen">
		<rdfs:label>Touchscreen</rdfs:label>
		<rdfs:comment>Indicates whether or not a represented item has a touchscreen.</rdfs:comment>
		<rdfs:range rdf:resource="xsd#boolean"/>
	</owl:DatatypeProperty>
	<owl:AnnotationProperty rdf:ID="waistband">
		<rdfs:label>Waistband</rdfs:label>
		<rdfs:comment>Describes what is used to adjust the waist of the represented item.</rdfs:comment>
	</owl:AnnotationProperty>
	<owl:AnnotationProperty rdf:ID="waistRise">
		<rdfs:label>Waist Rise</rdfs:label>
		<rdfs:comment>Describes how high or low the represented garment is expected to fall relative to the waist.'</rdfs:comment>
	</owl:AnnotationProperty>
	<owl:DatatypeProperty rdf:ID="waistSize">
		<rdfs:label>Waist Size</rdfs:label>
		<rdfs:comment>Indicates the circumference of the waist or hip as pertains to a represented item. May indicate the waist or hip of the consumer, or that of the represented item.</rdfs:comment>
		<av7:userNotes>If this attribute obtains a value, 'Waist Size UOM' must also obtain a value.</av7:userNotes>
		<rdfs:range rdf:resource="xsd#float"/>
	</owl:DatatypeProperty>
	<owl:ObjectProperty rdf:ID="waistSizeUOM">
		<rdfs:label>Waist Size UOM</rdfs:label>
		<rdfs:comment>Qualifies the value of 'Waist Size.'</rdfs:comment>
		<av7:userNotes>If this attribute obtains a value, 'Waist Size' must also obtain a value.</av7:userNotes>
		<rdfs:range rdf:resource="av7#SpatialUOM"/>
	</owl:ObjectProperty>
	<owl:DatatypeProperty rdf:ID="hasWarning">
		<rdf:subPropertyOf rdf:resource="av7#warning"/>
		<rdfs:label>Has Warning</rdfs:label>
		<rdfs:comment>Indicates whether or not an item contains a warning.</rdfs:comment>
		<rdfs:range rdf:resource="xsd#boolean"/>
	</owl:DatatypeProperty>
	<owl:AnnotationProperty rdf:ID="warningDescription">
		<rdf:subPropertyOf rdf:resource="av7#warning"/>
		<rdfs:label>Warning Description</rdfs:label>
		<rdfs:comment>Describes the warning(s) which apply to the represented item.</rdfs:comment>
		<rdfs:range>
			<owl:equivalentClass>
				<owl:complementOf rdf:resource="xsd#boolean"/>
			</owl:equivalentClass>
		</rdfs:range>
	</owl:AnnotationProperty>
	<owl:DatatypeProperty rdf:ID="hasWarranty">
		<rdfs:label>Warranty</rdfs:label>
		<rdfs:comment>Indicates whether or not an item includes a parts and/or labor warranty.</rdfs:comment>
		<rdfs:range rdf:resource="xsd#boolean"/>
	</owl:DatatypeProperty>
	<owl:AnnotationProperty rdf:ID="warrantyDescription">
		<rdfs:label>Warranty Description</rdfs:label>
		<rdfs:comment>Describes warranty terms appertaining to the item being described.</rdfs:comment>
	</owl:AnnotationProperty>
	<owl:AnnotationProperty rdf:ID="warrantyType">
		<rdfs:subPropertyOf rdf:resource="av7#warrantyContainerProperty"/>
		<rdfs:label>
			<rdf:Bag>
				<rdf:li rdf:value="Warranty Type"/>
				<rdf:li rdf:value="Warranty Type 1"/>
				<rdf:li rdf:value="Warranty Type 2"/>
			</rdf:Bag>
		</rdfs:label>
		<rdfs:comment>Describes or indicates a kind of warranty.</rdfs:comment>
	</owl:AnnotationProperty>
	<owl:DatatypeProperty rdf:ID="warrantyLength">
		<rdfs:subPropertyOf rdf:resource="av7#warrantyContainerProperty"/>
		<rdfs:label>
			<rdf:Bag>
				<rdf:li rdf:value="Warranty Length"/>
				<rdf:li rdf:value="Warranty Length 1"/>
				<rdf:li rdf:value="Warranty Length 2"/>
			</rdf:Bag>
		</rdfs:label>
		<rdfs:comment>Describes or indicates the length of warranty.</rdfs:comment>
		<rdfs:range rdf:resource="xsd#float"/>
	</owl:DatatypeProperty>
	<owl:AnnotationProperty rdf:ID="warrantyLengthUOM">
		<rdfs:subPropertyOf rdf:resource="av7#warrantyContainerProperty"/>
		<rdfs:label>
			<rdf:Bag>
				<rdf:li rdf:value="Warranty Length UOM"/>
				<rdf:li rdf:value="Warranty Length UOM 1"/>
				<rdf:li rdf:value="Warranty Length UOM 2"/>
			</rdf:Bag>
		</rdfs:label>
		<rdfs:comment>Qualifies the value of 'Warranty Length'.</rdfs:comment>
		<rdfs:range rdf:resource="xsd#float"/>
	</owl:AnnotationProperty>
	<owl:DatatypeProperty rdf:ID="watchBandWidth">
		<rdfs:label>Watch Band Width</rdfs:label>
		<rdfs:comment>Measures the width of the represented watch band.</rdfs:comment>
		<wmlo:userNotes>If this attribute obtains a value, 'Watch Band Width UOM' must obtain a value.</wmlo:userNotes>
		<rdfs:range rdf:resource="xsd#float"/>
	</owl:DatatypeProperty>
	<owl:ObjectProperty rdf:ID="watchBandWidthUOM">
		<rdfs:label>Watch Band Width UOM</rdfs:label>
		<rdfs:comment>Qualifies the value of 'Watch Band Width.'</rdfs:comment>
		<wmlo:userNotes>If this attribute obtains a value, 'Watch Band Width' must obtain a value.</wmlo:userNotes>
		<rdfs:range rdf:resource="av7#SpatialUOM"/>
	</owl:ObjectProperty>
	<owl:DatatypeProperty rdf:ID="watchCaseWidth">
		<rdfs:label>Watch Case Width</rdfs:label>
		<rdfs:comment>Measures the width of the represented watch case.</rdfs:comment>
		<wmlo:userNotes>If this attribute obtains a value, 'Watch Band Width UOM' must obtain a value.</wmlo:userNotes>
		<rdfs:range rdf:resource="xsd#float"/>
	</owl:DatatypeProperty>
	<owl:ObjectProperty rdf:ID="watchCaseWidthUOM">
		<rdfs:label rdf:value="Watch Case Width UOM"/>
		<rdfs:comment wmlo:txt="Qualifies the value of 'Watch Case Width.'"/>
		<wmlo:userNotes wmlo:txt="If this attribute obtains a value, 'Watch Case Width' must obtain a value."/>
		<av7:hasTab rdf:resource="av7#apparelAttributes"/>
		<rdfs:range rdf:resource="av7#SpatialUOM"/>
	</owl:ObjectProperty>
	<owl:DatatypeProperty rdf:ID="isWaterproof">
		<rdfs:subPropertyOf rdf:resource="av7#waterproof"/>
		<rdfs:label>Is Waterproof</rdfs:label>
		<rdfs:comment>Indicates whether or not the represented item is waterproof.</rdfs:comment>
		<rdfs:range rdf:resource="xsd#boolean"/>
	</owl:DatatypeProperty>
	<owl:AnnotationProperty rdf:ID="waterproofRating">
		<rdfs:subPropertyOf rdf:resource="av7#waterproof"/>
		<rdfs:label>Waterproof Rating</rdfs:label>
		<rdfs:comment>Rates the represented item's water-stopping power based upon IPX (International Protection Marking/Ingress Protection Rating) standard as defined in IEC 60529.</rdfs:comment>
		<sorg:relatedLink rdf:resource="https://www.nema.org/Standards/ComplimentaryDocuments/ANSI-IEC-60529.pdf"/>
		<rdfs:range>
			<owl:equivalentClass>
				<owl:complementOf rdf:resource="xsd#boolean"/>
			</owl:equivalentClass>
		</rdfs:range>
	</owl:AnnotationProperty>
	<owl:DatatypeProperty rdf:ID="waterResistant">
		<rdfs:label>Water Resistant</rdfs:label>
		<rdfs:comment>Indicates whether or not the represented item is water resistant.</rdfs:comment>
		<rdfs:range rdf:resource="xsd#boolean"/>
	</owl:DatatypeProperty>
	<owl:AnnotationProperty rdf:ID="waterResistantDescription">
		<rdfs:label>Water Resistant Description</rdfs:label>
		<rdfs:comment>Describes the water resistance associated with the represented item.</rdfs:comment>
	</owl:AnnotationProperty>
	<owl:DatatypeProperty rdf:ID="wattage">
		<rdfs:label>Wattage</rdfs:label>
		<rdfs:comment>Indicates the wattage associated with the represented item.</rdfs:comment>
		<rdfs:range rdf:resource="xsd#float"/>
	</owl:DatatypeProperty>
	<owl:AnnotationProperty rdf:ID="weaponType">
		<rdfs:label>Weapon Type</rdfs:label>
		<rdfs:comment>Indicates the type of weapon to which the represented item pertains.</rdfs:comment>
	</owl:AnnotationProperty>
	<owl:DatatypeProperty rdf:ID="wearLayer">
		<rdfs:label>Wear Layer</rdfs:label>
		<rdfs:comment>Measures the thickness of the wear layer for hard surfaces.</rdfs:comment>
		<wmlo:userNotes>If this attribute obtains a value, 'Wear Layer UOM' must obtain a value.</wmlo:userNotes>
		<rdfs:range rdf:resource="xsd#float"/>
	</owl:DatatypeProperty>
	<owl:ObjectProperty rdf:ID="wearLayerUOM">
		<rdfs:label>Wear Layer UOM</rdfs:label>
		<rdfs:comment>Qualifies the value of 'Wear Layer.'</rdfs:comment>
		<wmlo:userNotes>If this attribute obtains a value, 'Wear Layer' must obtain a value.</wmlo:userNotes>
		<rdfs:range rdf:resource="av7#SpatialUOM"/>
	</owl:ObjectProperty>
	<owl:DatatypeProperty rdf:ID="weatherResistant">
		<rdfs:label>Weather Resistant</rdfs:label>
		<rdfs:comment>Indicates whether or not the respresented item is resistant to elements including but not limited to wind, rain, snow, and temperature extremes.</rdfs:comment>
		<rdfs:range rdf:resource="xsd#boolean"/>
	</owl:DatatypeProperty>
	<owl:DatatypeProperty rdf:ID="weatherproof">
		<rdfs:label>Weatherproof</rdfs:label>
		<rdfs:comment>Indicates whether or not the respresented item is weatherproof; whether it is able to stop elements including but not limited to wind, rain, snow, and temperature extremes.</rdfs:comment>
		<rdfs:range rdf:resource="xsd#boolean"/>
	</owl:DatatypeProperty>
	<owl:AnnotationProperty rdf:ID="webbingPattern">
		<rdfs:label>Webbing Pattern</rdfs:label>
		<rdfs:comment>Describes the type of webbing on or associated with the represented item.</rdfs:comment>
	</owl:AnnotationProperty>
	<owl:DatatypeProperty rdf:ID="wiFi">
		<rdfs:label>WiFi</rdfs:label>
		<rdfs:comment>Indicates whether or not WiFi is supported by a represented item.</rdfs:comment>
		<rdfs:range rdf:resource="xsd#boolean"/>
	</owl:DatatypeProperty>
	<owl:DatatypeProperty rdf:ID="windResistant">
		<rdfs:label>Wind Resistant</rdfs:label>
		<rdfs:comment>Indicates whether or not the respresented item is resistant to the wind.</rdfs:comment>
		<rdfs:range rdf:resource="xsd#boolean"/>
	</owl:DatatypeProperty>
	<owl:DatatypeProperty rdf:ID="windproof">
		<rdfs:label>Windproof</rdfs:label>
		<rdfs:comment>Indicates whether or not the respresented item is windproof; whether it is able to stop the wind.</rdfs:comment>
		<rdfs:range rdf:resource="xsd#boolean"/>
	</owl:DatatypeProperty>
	<owl:DatatypeProperty rdf:ID="wirelessMicrophone">
		<rdfs:label>Wireless Microphone</rdfs:label>
		<rdfs:comment>Indicates whether or not a represented item has a wireless microphone.</rdfs:comment>
		<rdfs:range rdf:resource="xsd#boolean"/>
	</owl:DatatypeProperty>
	<owl:AnnotationProperty rdf:ID="woodSpecies">
		<rdfs:subPropertyOf rdf:resource="av7#wood"/>
		<rdfs:label>Wood Species</rdfs:label>
		<rdfs:comment>Indicates the hardwood type out of which the represented item is made.</rdfs:comment>
		<rdfs:range>
			<owl:equivlalentClass>
				<owl:complementOf rdf:resource="xsd#boolean"/>
			</owl:equivlalentClass>
		</rdfs:range>
	</owl:AnnotationProperty>
	<owl:DatatypeProperty rdf:ID="workingTime">
		<rdfs:label>Working Time</rdfs:label>
		<rdfs:comment>Indicates the amount of time that a represented item may be exposed and used in a normal working environment before setting.</rdfs:comment>
		<wmlo:userNotes>If this attribute obtains a value, 'Working Time UOM' must obtain a value.</wmlo:userNotes>
		<rdfs:range rdf:resource="xsd#float"/>
	</owl:DatatypeProperty>
	<owl:ObjectProperty rdf:ID="workingTimeUOM">
		<rdfs:label>Working Time UOM</rdfs:label>
		<rdfs:comment>Qualifies the value of 'Working Time.'</rdfs:comment>
		<wmlo:userNotes>If this attribute obtains a value, 'Working Time' must obtain a value.</wmlo:userNotes>
		<rdfs:range rdf:resource="av7#WorkingTimeUOM"/>
	</owl:ObjectProperty>
	<owl:DatatypeProperty rdf:ID="year">
		<rdfs:label>Year</rdfs:label>
		<rdfs:comment>The year in which the represented item was released or introduced.</rdfs:comment>
	</owl:DatatypeProperty>
	<owl:AnnotationProperty rdf:ID="yearsOfCompatibleItems">
		<rdfs:label>Year(s) of Compatible Item(s)</rdfs:label>
		<rdfs:comment>Indicates the production years of products that the represented item supports or is otherwise compatible with.</rdfs:comment>
	</owl:AnnotationProperty>
	<owl:DatatypeProperty rdf:ID="jacketLength">
		<rdfs:subPropertyOf rdf:resource="av7#jacket"/>
		<rdfs:label rdf:value="Jacket Length"/>
		<rdfs:comment rdf:value="Indicates the length of a jacket."/>
		<rdfs:domain/>
		<rdfs:range rdf:resource="xsd#float"/>
	</owl:DatatypeProperty>
	<owl:ObjectProperty rdf:ID="jacketLengthUOM">
		<rdfs:subPropertyOf rdf:resource="av7#jacket"/>
		<rdfs:label rdf:value="Jacket Length UOM"/>
		<rdfs:comment rdf:value="Qualifies the value of 'Jacket Length'."/>
		<rdfs:domain/>
		<rdfs:range rdf:resource="av7#SpatialUOM"/>
	</owl:ObjectProperty>
	<owl:DatatypeProperty rdf:ID="chestSize">
		<rdfs:label rdf:value="Chest Size"/>
		<rdfs:comment rdf:value="Indicates the measure of a human chest."/>
		<rdfs:domain/>
		<rdfs:range rdf:resource="xsd#float"/>
	</owl:DatatypeProperty>
	<owl:ObjectProperty rdf:ID="chestSizeUOM">
		<rdfs:label rdf:value="Chest Size UOM"/>
		<rdfs:comment rdf:value="Qualifies the value of 'Chest Size'."/>
		<rdfs:domain/>
		<rdfs:range rdf:resource="av7#SpatialUOM"/>
	</owl:ObjectProperty>
	<owl:DatatypeProperty rdf:ID="slitLength">
		<rdfs:label rdf:value="slitLength"/>
		<rdfs:comment rdf:value="Indicates the length of a slit."/>
		<rdfs:domain/>
		<rdfs:range rdf:resource="xsd#float"/>
	</owl:DatatypeProperty>
	<owl:ObjectProperty rdf:ID="slitLengthUOM">
		<rdfs:label rdf:value="Slit Length UOM"/>
		<rdfs:comment rdf:value="Qualifies the value of 'Slit Length'."/>
		<rdfs:domain/>
		<rdfs:range rdf:resource="av7#SpatialUOM"/>
	</owl:ObjectProperty>
	<owl:ObjectProperty rdf:ID="accessoriesEquipmentIncluded">
		<rdfs:subPropertyOf rdf:resource="av7c#peripheralsIncluded"/>
		<rdfs:type rdf:resource="av7#TranslationProp"/>
	</owl:ObjectProperty>
	<owl:ObjectProperty rdf:ID="battery">
		<rdfs:type rdf:resource="av7#TranslationProp"/>
	</owl:ObjectProperty>
	<owl:ObjectProperty rdf:ID="bend">
		<rdfs:type rdf:resource="av7#TranslationProp"/>
	</owl:ObjectProperty>
	<owl:ObjectProperty rdf:ID="bearing">
		<rdfs:type rdf:resource="av7#TranslationProp"/>
	</owl:ObjectProperty>
	<owl:ObjectProperty rdf:ID="bulb">
		<rdfs:type rdf:resource="av7#TranslationProp"/>
	</owl:ObjectProperty>
	<owl:ObjectProperty rdf:ID="chemical">
		<rdfs:type rdf:resource="av7#TranslationProp"/>
	</owl:ObjectProperty>
	<owl:ObjectProperty rdf:ID="county">
		<rdfs:type rdf:resource="av7#TranslationProp"/>
	</owl:ObjectProperty>
	<owl:ObjectProperty rdf:ID="customizability">
		<rdfs:type rdf:resource="av7#TranslationProp"/>
	</owl:ObjectProperty>
	<owl:ObjectProperty rdf:ID="handle">
		<rdfs:type rdf:resource="av7#TranslationProp"/>
	</owl:ObjectProperty>
	<owl:ObjectProperty rdf:ID="fuelBurner">
		<rdfs:type rdf:resource="av7#TranslationProp"/>
	</owl:ObjectProperty>
	<owl:ObjectProperty rdf:ID="jacket">
		<rdfs:type rdf:resource="av7#TranslationProp"/>
	</owl:ObjectProperty>
	<owl:ObjectProperty rdf:ID="magnification">
		<rdfs:type rdf:resource="av7#TranslationProp"/>
	</owl:ObjectProperty>
	<owl:ObjectProperty rdf:ID="memory">
		<rdfs:type rdf:resource="av7#TranslationProp"/>
	</owl:ObjectProperty>
	<owl:ObjectProperty rdf:ID="partialPack">
		<rdfs:type rdf:resource="av7#TranslationProp"/>
	</owl:ObjectProperty>
	<owl:ObjectProperty rdf:ID="recycling">
		<rdfs:type rdf:resource="av7#TranslationProp"/>
	</owl:ObjectProperty>
	<owl:ObjectProperty rdf:ID="screenDisplay">
		<rdfs:type rdf:resource="av7#TranslationProp"/>
	</owl:ObjectProperty>
	<owl:ObjectProperty rdf:ID="seasonality">
		<rdfs:type rdf:resource="av7#TranslationProp"/>
	</owl:ObjectProperty>
	<owl:ObjectProperty rdf:ID="shaft">
		<rdfs:type rdf:resource="av7#TranslationProp"/>
	</owl:ObjectProperty>
	<owl:ObjectProperty rdf:ID="smallPackageCarrier">
		<rdfs:type rdf:resource="av7#TranslationProp"/>
	</owl:ObjectProperty>
	<owl:ObjectProperty rdf:ID="spreadRate">
		<rdfs:type rdf:resource="av7#TranslationProp"/>
	</owl:ObjectProperty>
	<owl:ObjectProperty rdf:ID="storageTemperature">
		<rdfs:type rdf:resource="av7#TranslationProp"/>
	</owl:ObjectProperty>
	<owl:ObjectProperty rdf:ID="usState">
		<rdfs:type rdf:resource="av7#TranslationProp"/>
	</owl:ObjectProperty>
	<owl:ObjectProperty rdf:ID="variant">
		<rdfs:type rdf:resource="av7#TranslationProp"/>
	</owl:ObjectProperty>
	<owl:ObjectProperty rdf:ID="warning">
		<rdfs:type rdf:resource="av7#TranslationProp"/>
	</owl:ObjectProperty>
	<owl:ObjectProperty rdf:ID="warranty">
		<rdfs:type rdf:resource="av7#TranslationProp"/>
	</owl:ObjectProperty>
	<owl:ObjectProperty rdf:ID="waterproof">
		<rdfs:type rdf:resource="av7#TranslationProp"/>
	</owl:ObjectProperty>
	<owl:ObjectProperty rdf:ID="wood">
		<rdfs:type rdf:resource="av7#TranslationProp"/>
	</owl:ObjectProperty>
	<owl:AnnotationProperty rdf:ID="maintainenceTypeCode">
		<rdfs:type rdf:resource="av7#TranslationProp"/>
	</owl:AnnotationProperty>
	<owl:ObjectProperty rdf:ID="directShipCost">
		<rdfs:label>Direct Ship Price</rdfs:label>
		<rdfs:range>
			<owl:Restriction>
				<owl:onProperty rdf:resource="av7#directShipCost"/>
				<owl:allValuesFrom rdf:resource="xsd#float"/>
			</owl:Restriction>
		</rdfs:range>
		<rdfs:range>
			<owl:Restriction>
				<owl:onProperty rdf:resource="av7#directShipCost"/>
				<owl:allValuesFrom rdf:resource="wmlo#PriceUOM"/>
			</owl:Restriction>
		</rdfs:range>
	</owl:ObjectProperty>
	<owl:ObjectProperty rdf:ID="dropShipCost">
		<rdfs:label>Drop Ship Price</rdfs:label>
		<rdfs:range>
			<owl:Restriction>
				<owl:onProperty rdf:resource="av7#dropShipCost"/>
				<owl:allValuesFrom rdf:resource="xsd#float"/>
			</owl:Restriction>
		</rdfs:range>
		<rdfs:range>
			<owl:Restriction>
				<owl:onProperty rdf:resource="av7#dropShipCost"/>
				<owl:allValuesFrom rdf:resource="wmlo#PriceUOM"/>
			</owl:Restriction>
		</rdfs:range>
	</owl:ObjectProperty>
	<owl:ObjectProperty rdf:ID="internetMinimumAdvertisedCost">
		<rdfs:label>Internet Minimum Advertised Price</rdfs:label>
		<rdfs:range>
			<owl:Restriction>
				<owl:onProperty rdf:resource="av7#internetMinimumAdvertisedCost"/>
				<owl:allValuesFrom rdf:resource="xsd#float"/>
			</owl:Restriction>
		</rdfs:range>
		<rdfs:range>
			<owl:Restriction>
				<owl:onProperty rdf:resource="av7#internetMinimumAdvertisedCost"/>
				<owl:allValuesFrom rdf:resource="wmlo#PriceUOM"/>
			</owl:Restriction>
		</rdfs:range>
	</owl:ObjectProperty>
	<owl:ObjectProperty rdf:ID="listCost">
		<rdfs:label>List Price</rdfs:label>
		<rdfs:range>
			<owl:Restriction>
				<owl:onProperty rdf:resource="av7#listPrice"/>
				<owl:allValuesFrom rdf:resource="xsd#float"/>
			</owl:Restriction>
		</rdfs:range>
		<rdfs:range>
			<owl:Restriction>
				<owl:onProperty rdf:resource="av7#listpCost"/>
				<owl:allValuesFrom rdf:resource="wmlo#PriceUOM"/>
			</owl:Restriction>
		</rdfs:range>
	</owl:ObjectProperty>
	<owl:ObjectProperty rdf:ID="manufacturerSuggestedRetailCost">
		<rdfs:label>Manufacturer Suggested Retail Price</rdfs:label>
		<rdfs:range>
			<owl:Restriction>
				<owl:onProperty rdf:resource="av7#manufacturerSuggestedRetailCost"/>
				<owl:allValuesFrom rdf:resource="xsd#float"/>
			</owl:Restriction>
		</rdfs:range>
		<rdfs:range>
			<owl:Restriction>
				<owl:onProperty rdf:resource="av7#manufacturerSuggestedRetailCost"/>
				<owl:allValuesFrom rdf:resource="wmlo#PriceUOM"/>
			</owl:Restriction>
		</rdfs:range>
	</owl:ObjectProperty>
	<owl:ObjectProperty rdf:ID="marketRetailCost">
		<rdfs:label>Market Retail Price</rdfs:label>
		<rdfs:range>
			<owl:Restriction>
				<owl:onProperty rdf:resource="av7#marketRetailCost"/>
				<owl:allValuesFrom rdf:resource="xsd#float"/>
			</owl:Restriction>
		</rdfs:range>
		<rdfs:range>
			<owl:Restriction>
				<owl:onProperty rdf:resource="av7#marketRetailCost"/>
				<owl:allValuesFrom rdf:resource="wmlo#PriceUOM"/>
			</owl:Restriction>
		</rdfs:range>
	</owl:ObjectProperty>
	<owl:ObjectProperty rdf:ID="unilateralMinimumAdvertisedCost">
		<rdfs:label>Unilateral Minimum Advertised Price</rdfs:label>
		<rdfs:range>
			<owl:Restriction>
				<owl:onProperty rdf:resource="av7#unilateralMinimumAdvertisedCost"/>
				<owl:allValuesFrom rdf:resource="xsd#float"/>
			</owl:Restriction>
		</rdfs:range>
		<rdfs:range>
			<owl:Restriction>
				<owl:onProperty rdf:resource="av7#unilateralMinimumAdvertisedCost"/>
				<owl:allValuesFrom rdf:resource="wmlo#PriceUOM"/>
			</owl:Restriction>
		</rdfs:range>
	</owl:ObjectProperty>
	<owl:ObjectProperty rdf:ID="unitCostCost">
		<rdfs:label>Unit Cost Price</rdfs:label>
		<rdfs:range>
			<owl:Restriction>
				<owl:onProperty rdf:resource="av7#unitCostCost"/>
				<owl:allValuesFrom rdf:resource="xsd#float"/>
			</owl:Restriction>
		</rdfs:range>
		<rdfs:range>
			<owl:Restriction>
				<owl:onProperty rdf:resource="av7#unitCostCost"/>
				<owl:allValuesFrom rdf:resource="wmlo#PriceUOM"/>
			</owl:Restriction>
		</rdfs:range>
	</owl:ObjectProperty>
	<owl:ObjectProperty rdf:ID="wholesaleCost">
		<rdfs:label>Wholesale Price</rdfs:label>
		<rdfs:range>
			<owl:Restriction>
				<owl:onProperty rdf:resource="av7#wholesaleCost"/>
				<owl:allValuesFrom rdf:resource="xsd#float"/>
			</owl:Restriction>
		</rdfs:range>
		<rdfs:range>
			<owl:Restriction>
				<owl:onProperty rdf:resource="av7#wholesaleCost"/>
				<owl:allValuesFrom rdf:resource="wmlo#PriceUOM"/>
			</owl:Restriction>
		</rdfs:range>
	</owl:ObjectProperty>
</rdf:RDF>
